%
% Copyright © 2013 Peeter Joot.  All Rights Reserved.
% Licenced as described in the file LICENSE under the root directory of this GIT repository.
%
%\input{../blogpost.tex}
%\renewcommand{\basename}{nonIntegralBinomialSeries}
%\renewcommand{\dirname}{notes/phy452/}
%\newcommand{\keywords}{binomial coefficient, factorial, gamma function, Taylor expansion, binomial series}
%
%\input{../peeter_prologue_print2.tex}
%
%\beginArtNoToc
%
%\generatetitle{Non integral binomial coefficient}
\label{chap:nonIntegralBinomialSeries}

In \citep{pathriastatistical} appendix \S F was the use of binomial coefficients in a non-integral binomial expansion.  This surprised me, since I'd never seen that before.  However, on reflection, this is a very sensible notation, provided the binomial coefficients are defined in terms of the gamma function.  Let's explore this little detail explicitly, starting with a Taylor expansion of

\begin{dmath}\label{eqn:nonIntegralBinomialSeries:20}
f(x) = (a + x)^b.
\end{dmath}

Our derivatives are

\begin{equation}\label{eqn:nonIntegralBinomialSeries:40}
\begin{aligned}
f'(x) &= b (a + x)^{b-1} \\
f''(x) &= b(b-1) (a + x)^{b-2} \\
f^3(x) &= b(b-1)(b-(3-1)) (a + x)^{b-3} \\
\vdots & \\
f^k(x) &= b(b-1)\cdots (b-(k-1)) (a + x)^{b-k}.
\end{aligned}
\end{equation}

Our Taylor series is then

\begin{dmath}\label{eqn:nonIntegralBinomialSeries:60}
(a + x)^b = \sum_{k = 0}^\infty \inv{k!} b(b-1)\cdots (b-(k-1)) a^{b-k} x^k.
\end{dmath}

If $b$ is integral, then all the elements of this series become zero at $b = k - 1$, or

\begin{dmath}\label{eqn:nonIntegralBinomialSeries:80}
(a + x)^b = \sum_{k = 0}^k \inv{k!} b(b-1)\cdots (b-(k-1)) a^{b-k} x^k.
\end{dmath}

Let's now relate this to the gamma function.  From \citep{abramowitz1964handbook} \S 6.1.1 we have

\begin{dmath}\label{eqn:nonIntegralBinomialSeries:100}
\Gamma(z) = \int_0^\infty t^{z-1} e^{-t} dt.
\end{dmath}

Iteratively integrating by parts, we find the usual relation between gamma functions of integral separation

\begin{dmath}\label{eqn:nonIntegralBinomialSeries:120}
\Gamma(z + 1) 
= \int_0^\infty t^{z} e^{-t} dt
= \int_0^\infty t^{z} d \lr{ \frac{ e^{-t}}{-1} }
= 
\evalrange{
t^z \frac{e^{-t}}{-1}
}{0}{\infty}
- \int_0^\infty z t^{z-1} \frac{e^{-t}}{-1} dt
=
z \int_0^\infty t^{z-1} e^{-t} dt
=
z (z - 1)\int_0^\infty t^{z-2} e^{-t} dt
=
z (z - 1)(z - (3-1))\int_0^\infty t^{z-3} e^{-t} dt
=
z (z - 1) \cdots (z - (k-1))\int_0^\infty t^{z-k} e^{-t} dt
=
z (z - 1) \cdots (z - (k-1))\int_0^\infty t^{(z + 1 - k) - 1} e^{-t} dt,
\end{dmath}

or

\begin{dmath}\label{eqn:nonIntegralBinomialSeries:140}
\Gamma(z + 1) = z (z - 1) \cdots (z - (k-1)) \Gamma( z - (k-1) ).
\end{dmath}

Flipping this gives us a nice closed form expression for the products of a number of unit separated values, integer or otherwise

\begin{dmath}\label{eqn:nonIntegralBinomialSeries:160}
z (z - 1) \cdots (z - k)
=
\frac{\Gamma(z + 1)}{\Gamma( z - (k-1) )}.
\end{dmath}

We can now use this in our Taylor expansion \eqnref{eqn:nonIntegralBinomialSeries:60}

\begin{dmath}\label{eqn:nonIntegralBinomialSeries:180}
(a + x)^b 
= \sum_{k = 0}^\infty \inv{k!} \frac{\Gamma(b+1)}{\Gamma{b - k + 1}}
a^{b-k} x^k
= \sum_{k = 0}^\infty \frac{\Gamma(b + 1)}{\Gamma(k + 1)\Gamma{b - k + 1}}
a^{b-k} x^k.
\end{dmath}

Observe that when $b$ is integral we have

\begin{equation}\label{eqn:nonIntegralBinomialSeries:200}
\frac{\Gamma(b + 1)}{\Gamma(k + 1)\Gamma{b - k + 1}}
=
\frac{b!}{k!(b-k)!}
= \binom{b}{k}.
\end{equation}

We see that is then very reasonable to define the binomial coefficient \index{binomial coefficient} explicitly in terms of the gamma function

\begin{equation}\label{eqn:nonIntegralBinomialSeries:220}
\binom{b}{k} \equiv
\frac{\Gamma(b + 1)}{\Gamma(k + 1)\Gamma(b - k + 1)}.
\end{equation}

If we do that, then the binomial expansion for non-integral values of $b$ is simply

\begin{dmath}\label{eqn:nonIntegralBinomialSeries:240}
(a + x)^b = \sum_{k = 0}^\infty \binom{b}{k} a^{b-k} x^k.
\end{dmath}

%\EndArticle
