\input{../peeter_prologue_print.tex}
%\input{../peeter_prologue_widescreen.tex}

\chapter{PHY454H1S\\Continuum Mechanics.  Lecture 8: Phasor description of elastic waves.  Fluid dynamics.  Taught by Prof. K. Das.}
\label{chap:continuumL8}
%\useCCL
\blogpage{http://sites.google.com/site/peeterjoot2/math2012/continuumL8.pdf}
\date{Feb 3, 2012}
\revisionInfo{continuumL8.tex}

\beginArtWithToc
%\beginArtNoToc

\section{Disclaimer.}

Peeter's lecture notes from class.  May not be entirely coherent.

\section{Review.  Elastic wave equation}

Starting with

\begin{equation}\label{eqn:continuumL8:n}
\rho \PDSq{t}{\Be} = (\lambda + \mu) \spacegrad (\spacegrad \cdot \Be) + \mu \spacegrad^2 \Be
\end{equation}

and applying a divergence operation we find

\begin{align}\label{eqn:continuumL8:n}
\rho \PDSq{t}{\theta} &= C_L^2 \spacegrad^2 \theta \\
\theta &= \spacegrad \cdot \Be \\
C_L^2 &= \frac{\lambda + 2\mu}{\rho}.
\end{align}

This is the P-wave equation.  Applying a curl operation we find

\begin{align}\label{eqn:continuumL8:n}
\rho \PDSq{t}{\Bomega} &= C_T^2 \spacegrad^2 \Bomega \\
\Bomega &= \spacegrad \cross \Be \\
C_T^2 &= \frac{\lambda + 2\mu}{\rho}.
\end{align}

This is the S-wave equation.  We also found that

\begin{equation}\label{eqn:continuumL8:n}
\frac{C_L}{C_T} > 1,
\end{equation}

and concluded that P waves are faster than S waves.  What we haven't shown is that the P waves are longitudinal, and that the S waves are transverse.

Assuming a gradient and curl description of our displacement

\begin{equation}\label{eqn:continuumL8:n}
\Be = \spacegrad \phi + \spacegrad \cross \BH = \BP + \BS,
\end{equation}

we found

\begin{align}\label{eqn:continuumL8:n}
(\lambda + 2 \mu) \spacegrad^2 \phi - \rho \PDSq{t}{\phi} &= 0 \\
\mu \spacegrad^2 \BH - \rho \PDSq{t}{\BH} &= 0,
\end{align}

allowing us to separately solve for the P and the S wave solutions respectively.  Now, let's introduce a phasor representation (again following \S 22 of the text \cite{landau1960theory})

\begin{align}\label{eqn:continuumL8:n}
\phi &= A \exp\left( i ( \Bk \cdot \Bx - \omega t) \right) \\
\BH &= \BB \exp\left( i ( \Bk \cdot \Bx - \omega t) \right)
\end{align}

Operating with the gradient we find

\begin{align*}
\BP
&= \spacegrad \phi \\
&= \Be_k \partial_k A \exp\left( i ( \Bk \cdot \Bx - \omega t) \right) \\
&= \Be_k \partial_k A \exp\left( i ( k_m x_m - \omega t) \right) \\
&= \Be_k i k_k A \exp\left( i ( k_m x_m - \omega t) \right) \\
&= i \Bk A \exp\left( i ( \Bk \cdot \Bx - \omega t) \right) \\
&= i \Bk \phi
\end{align*}

We can also write

\begin{equation}\label{eqn:continuumL8:n}
\BP = \Bk \phi'
\end{equation}

where $\phi'$ is the derivative of $\phi$ ``with respect to its argument''.   Here argument must mean the entire phase $\Bk \cdot \Bx - \omega t$

\begin{equation}\label{eqn:continuumL8:n}
\phi' = \frac{ d\phi( \Bk \cdot \Bx - \omega t )}{ d(\Bk \cdot \Bx - \omega t) } = i \phi
\end{equation}

For the curl term we find

\begin{align*}
\BS
&= \spacegrad \cross \BH \\
&= \Be_a \partial_b H_c \epsilon_{a b c} \\
&= \Be_a \partial_b \epsilon_{a b c} B_c \exp\left( i ( \Bk \cdot \Bx - \omega t) \right) \\
&= \Be_a \partial_b \epsilon_{a b c} B_c \exp\left( i ( k_m x_m - \omega t) \right) \\
&= \Be_a i k_b \epsilon_{a b c} B_c \exp\left( i ( \Bk \cdot \Bx - \omega t) \right) \\
&= i \Bk \cross \BH
\end{align*}

Again writing
\begin{equation}\label{eqn:continuumL8:n}
\BH' = \frac{ d\BH( \Bk \cdot \Bx - \omega t )}{ d(\Bk \cdot \Bx - \omega t) } = i \BH
\end{equation}

we can write the S wave as

\begin{equation}\label{eqn:continuumL8:n}
\BS = \Bk \cross \BH'
\end{equation}

\subsection{Some waves illustrated.}

The following wave types were noted, but not defined:

\begin{itemize}
\item Love wave
\item Rayleigh wave
\end{itemize}

Some illustrations from the class notes were also shown.

\section{Fluid dynamics.}

%FIXME: Reading: \S XX from \cite{landau1960theory}.

In fluid dynamics we look at displacements with respect to time as illustrated in

FIXME: F1.

\begin{equation}\label{eqn:continuumL8:n}
d\Bx' = d\Bx + d\Bu \delta t
\end{equation}

In index notation

\begin{align*}
dx_i'
&= dx_i + du_i \delta t \\
&= dx_i + \PD{x_j}{u_i} dx_j \delta t
\end{align*}

We define

\begin{equation}\label{eqn:continuumL8:n}
e_{ij} = \inv{2} \left(
\PD{x_j}{u_i} +
\PD{x_i}{u_j} \right)
\end{equation}

a symmetric tensor.  We also define

\begin{equation}\label{eqn:continuumL8:n}
\omega_{ij} = \inv{2} \left(
\PD{x_j}{u_i}
-\PD{x_i}{u_j} \right)
\end{equation}

Effect of $e_{ij}$ when diagonalized

\begin{equation}\label{eqn:continuumL8:n}
e_{ij} =
=
\begin{bmatrix}
e_{11} & 0 & 0 \\
0 & e_{22} & 0 \\
0 & 0 & e_{33}
\end{bmatrix}
\end{equation}

FIXME: check:
\begin{align}\label{eqn:continuumL8:n}
dx_1' &= ( 1 + u_1 \delta t) dx_1 \\
dx_2' &= ( 1 + u_2 \delta t) dx_2 \\
dx_3' &= ( 1 + u_3 \delta t) dx_3
\end{align}

Let's find the matrix form of the antisymmetric tensor.  We find

\begin{equation}\label{eqn:continuumL8:n}
\omega_{11} = \omega_{22} = \omega_{33} = 0
\end{equation}

Introducing a vorticity vector

\begin{equation}\label{eqn:continuumL8:n}
\Bomega = \spacegrad \cross \Bu
\end{equation}

we find

\begin{align}\label{eqn:continuumL8:n}
\omega_{12} &= \inv{2}\left( \PD{x_2}{u_1} -\PD{x_1}{u_2} \right) = - \inv{2} (\spacegrad \cross \Bu)_3 \\
\omega_{23} &= \inv{2}\left( \PD{x_3}{u_2} -\PD{x_2}{u_3} \right) = - \inv{2} (\spacegrad \cross \Bu)_1 \\
\omega_{31} &= \inv{2}\left( \PD{x_1}{u_3} -\PD{x_3}{u_1} \right) = - \inv{2} (\spacegrad \cross \Bu)_2
\end{align}

Writing

\begin{equation}\label{eqn:continuumL8:n}
\Omega_i = \inv{2} \omega_i
\end{equation}

we find the matrix form of this antisymmetric tensor

\begin{equation}\label{eqn:continuumL8:n}
\omega_{ij}
=
\begin{bmatrix}
0 & -\Omega_3 & \Omega_2 \\
\Omega_3 & 0 & -\Omega_1 \\
-\Omega_2 & \Omega_1 & 0 \\
\end{bmatrix}
\end{equation}

\begin{align*}
dx_1'
&= dx_1 + \left( \cancel{\omega_{11}} dx_1 + \omega_{12} dx_2 + \omega_{13} dx_3 \right) \delta t \\
&= dx_1 + \left( \omega_{12} dx_2 + \omega_{13} dx_3 \right) \delta t \\
&= dx_1 + \left( \Omega_2 dx_3 - \Omega_3 dx_2 \right) \delta t
\end{align*}

Doing this for all components we find

\begin{equation}\label{eqn:continuumL8:n}
d\Bx' = d\Bx + (\BOmega \cross d\Bx) \delta t.
\end{equation}

The tensor $\omega_{ij}$ implies rotation of a control volume with an angular velocity $\BOmega = \Bomega/2$ (half the vorticity vector).

In general we have

\begin{equation}\label{eqn:continuumL8:n}
dx_i' = dx_i + e_{ij} dx_j \delta t + \omega_{ij} dx_j \delta t
\end{equation}

\EndArticle
%\EndNoBibArticle
