\makeproblem{description}{modernOptics:problemSet4:4}{ 

Using the M\"obius transform $q' = (A q + B)/(C q + D)$, show that transformation using $\{A_1, B_1, C_1, D_1 \}$ followed by $\{A_2, B_2, C_2, D_2 \}$ is equivalent to transformation using the elements of the single matrix $M = M_2 M_1$, where 
$$M_1 = \left( \begin{array}{cc} A_1 & B_1 \\ C_1 & D_1  \end{array} \right) 
\quad  \mbox{and} \quad
M_2 = \left( \begin{array}{cc} A_2 & B_2 \\ C_2 & D_2  \end{array} \right) .$$
}
\makeanswer{modernOptics:problemSet4:4}{ 

TODO.
}

