\makeproblem{Gaussian beam and lens}{modernOptics:problemSet4:1}{ 

%\cref{fig::FigQ1}.
\imageFigure{FigQ1}{}{fig:modernOpticsProblemSet4:FigQ1}{0.3}
%\begin{center}
%{\resizebox{3.5in}{!}{\includegraphics{FigQ1.eps} } }
%\end{center}

Consider a Gaussian beam whose waist is $w_{01}$ and placed at a lens of focal length $f$. This lens makes a focus some distance $\ell$ away. 

\makesubproblem{Find the distance}{modernOptics:problemSet4:1a}
%{\bf (a)} 
Find the distance $\ell$, in terms of $w_{01}$, $f$, and $\lambda$. In what limit does the lens create a focus at $\ell = f$, as geometric optics would have predicted? Interpret this physically.

\makesubproblem{new beam waist}{modernOptics:problemSet4:1b}
%{\bf (b)} 
Find the new beam waist $w_{03}$. In the same limit where $\ell \approx f$, show that the waist is $w_{03} \approx {\lambda f}/{\pi w_{01}}.$
}
\makeanswer{modernOptics:problemSet4:1}{ 
\makeSubAnswer{The distance}{modernOptics:problemSet4:1a}
TODO.

\makeSubAnswer{The waist}{modernOptics:problemSet4:1b}

Observe that the we can write the waist function as a function of $q$

\begin{dmath}\label{eqn:problemSet4Problem1:20}
w^2(z) 
= w_0^2 \left( 1 + \frac{z^2}{z_0^2} \right)
= \frac{w_0^2}{z_0^2} ( z_0^2 + z^2 )
= \frac{w_0^2}{z_0^2} \Abs{ q(z) }^2.
\end{dmath}

Also observe that $w(0) = w(0)$, so if we are looking for the beam waist after a geometric (M\"obius) transformation on $q$, we can find the new beam waist, looking at the $z = 0$ value.  

\paragraph{After just the lens}

After transmission through the lens, with ABCD matrix

\begin{dmath}\label{eqn:problemSet4Problem1:40}
M = 
\begin{bmatrix}
1 & 0 \\
-1/f & 1
\end{bmatrix}
\end{dmath}

\begin{dmath}\label{eqn:problemSet4Problem1:60}
q' = 
\frac{q + 0}{-q/f + 1},
\end{dmath}

or

\begin{dmath}\label{eqn:problemSet4Problem1:80}
\inv{q'} 
= 
\frac
{-q/f + 1}
{q}
= 
\inv{q} -\inv{f}.
\end{dmath}

At $z = 0$ we have

\begin{dmath}\label{eqn:problemSet4Problem1:100}
\Abs{\inv{q'}}^2 
= \Abs{ \inv{-i z_0} - \inv{f} } 
= \inv{z_0^2} + \inv{f^2} 
\end{dmath}

So that 

\begin{dmath}\label{eqn:problemSet4Problem1:120}
w^2(0) 
\rightarrow 
\frac{w_{01}^2}{z_0^2} 
\left( \inv{z_0^2} + \inv{f^2}  \right)^{-1}
=
\frac{w_{01}^2}{z_0^2} 
\frac{ f^2 z_0^2}{
f^2 + z_0^2
}
=
\frac{w_{01}^2}{ 1 + z_0^2/f^2}.
\end{dmath}

We see that the beam waste after transmission through the lens is reduced by a factor of

\begin{dmath}\label{eqn:problemSet4Problem1:140}
\frac
{w_{02}}
{w_{01}}
=
\frac{1}{ \sqrt{1 + z_0^2/f^2} }.
\end{dmath}

\paragraph{After the lens and the free propagation}

With both transmission through the air and the lens, where our free propagation matrix is

\begin{dmath}\label{eqn:problemSet4Problem1:160}
M_2 = 
\begin{bmatrix}
1 & l \\
0 & 1
\end{bmatrix}
\end{dmath}

\begin{dmath}\label{eqn:problemSet4Problem1:180}
q 
\rightarrow \frac{q' + l}{0 q' + 1} 
= q' + l 
= \frac{q}{-q/f + 1} + l,
\end{dmath}

so that the waste function is transformed as

\begin{dmath}\label{eqn:problemSet4Problem1:200}
w^2(z) \rightarrow \frac{w_{01}^2}{z_0^2} \Abs{ 
\frac{q}{-q/f + 1} + l
}^2,
\end{dmath}

and our waist goes as
\begin{dmath}\label{eqn:problemSet4Problem1:220}
w_{01}^2 
\rightarrow \frac{w_{01}^2}{z_0^2} \Abs{ 
\frac{-i z_0 f }{i z_0 + f} + l
}^2
= \frac{w_{01}^2}{z_0^2} \Abs{ 
\frac{-i z_0 f \left(-i z_0 + f\right)}{z_0^2 + f^2} + l
}^2
= \frac{w_{01}^2}{z_0^2} \Abs{ 
-\frac{z_0^2 f}{z_0^2 + f^2} + l
-\frac{i z_0 f^2 }{z_0^2 + f^2} 
}^2.
\end{dmath}

This gives us

\begin{dmath}\label{eqn:problemSet4Problem1:240}
\boxed{
\frac{w_{03}^2}{w_{01}^2} 
= \frac{
\left(z_0^2 \left(l - f\right) + f^2 l\right)^2
+ \left( f^2 z_0  \right)^2
}{z_0^2 \left(z_0^2 + f^2\right)^2 }.
}
\end{dmath}

When $l = f$ the square root simplifies nicely, leaving

\begin{dmath}\label{eqn:problemSet4Problem1:260}
\frac{w_{03}^2}{w_{01}^2} 
= \frac{
f^6 + f^4 z_0^2
}{z_0^2 \left(z_0^2 + f^2\right)^2 }
= 
\frac{f^4}{z_0^2\left(z_0^2 + f^2\right) },
\end{dmath}

or
\begin{dmath}\label{eqn:problemSet4Problem1:280}
w_{03}
= 
\frac{w_{01} f^2}{z_0 \sqrt{z_0^2 + f^2} }
= 
\frac{w_{01} f}{z_0 \sqrt{z_0^2/f^2 + 1} }
=
\frac{w_{01} f \lambda}{\pi w_{01}^2 \sqrt{z_0^2/f^2 + 1} }
=
\frac{f \lambda}{\pi w_{01}} \inv{\sqrt{z_0^2/f^2 + 1} }.
\end{dmath}

When $f \gg z_0$ we have the desired result
\begin{dmath}\label{eqn:problemSet4Problem1:300}
\boxed{
w_{03}
\approx
\frac{f \lambda}{\pi w_{01}} 
}
\end{dmath}

}

