%
% Copyright © 2012 Peeter Joot.  All Rights Reserved.
% Licenced as described in the file LICENSE under the root directory of this GIT repository.
%
% pick one:
%\input{../assignment.tex}
\input{../blogpost.tex}
\renewcommand{\basename}{modernOpticsCheatsheet}
\renewcommand{\dirname}{notes/phy485/}
%\newcommand{\dateintitle}{}
%\newcommand{\keywords}{}

\input{../peeter_prologue_print2.tex}

\beginArtNoToc

\generatetitle{Possible content for formula sheet}

Rules: No text, or figures allowed.

\section{Geometric optics}

\begin{dmath}
n \sin\alpha = n' \sin\alpha'
\end{dmath}

\begin{equation}
\inv{f} = \inv{s} + \inv{s'}
\end{equation}

\begin{dmath}
\begin{bmatrix}
y_f \\
\alpha_f
\end{bmatrix}
=
\begin{bmatrix}
1 & L \\
0 & 1
\end{bmatrix}
\begin{bmatrix}
y_i \\
\alpha_i
\end{bmatrix}
\end{dmath}

\begin{dmath}
\begin{bmatrix}
y_f \\
\alpha_f
\end{bmatrix}
=
\begin{bmatrix}
1 & 0 \\
0 & \frac{n'}{n}
\end{bmatrix}
\begin{bmatrix}
y_i \\
\alpha_i
\end{bmatrix}
\end{dmath}

\begin{dmath}
\begin{bmatrix}
y_f \\
\alpha_f
\end{bmatrix}
=
\begin{bmatrix}
1 & 0 \\
\inv{R}\left( \frac{n}{n'} -1 \right) & \frac{n}{n'}
\end{bmatrix}
\begin{bmatrix}
y_i \\
\alpha_i
\end{bmatrix}
\end{dmath}

\begin{dmath}
M =
\begin{bmatrix}
1 & 0 \\
- 1/f & 1
\end{bmatrix}
\end{dmath}

\begin{dmath}
\inv{f} = \frac{n' - n}{n} \left( \inv{R_1} - \inv{R_2} \right), \qquad R_1 > 0, R_2 < 0
\end{dmath}

\begin{equation}
x x' = f^2, x + f = s, x' + f = s'
\end{equation}

\begin{equation}
m = -\frac{s'}{s} = \frac{x'}{f}
\end{equation}

\section{Misc trig}

\begin{equation}
\sin(\pi - \theta) = \sin\theta
\end{equation}

\begin{equation}
\sin( \alpha + \beta) = \sin \alpha \cos \beta + \cos \alpha \sin \beta
\end{equation}

\begin{equation}
\cos(\alpha + \beta) = cos(\alpha)cos(\beta) - sin(\alpha)sin(\beta) 
\end{equation}

\begin{equation}
\sin 2\theta = 2 \sin \theta \cos \theta
\end{equation}

\begin{equation}
\cos 2\theta = 2 \cos^2 \theta - 1
\end{equation}

\begin{equation}
\cos\Atan x = \inv{\sqrt{1 + x^2}}
\end{equation}
\begin{equation}
\sin\Atan x = \frac{x}{\sqrt{1 + x^2}}
\end{equation}

\section{Eikonal}

\begin{equation}
\begin{bmatrix}
\BE \\
\BB \\
\end{bmatrix}
=
\begin{bmatrix}
\BE_0(\Br) \\
\BB_0(\Br) \\
\end{bmatrix}
e^{i \phi(\Br) - i \omega t}
\end{equation}


\begin{equation}
n = \frac{c}{v} = \sqrt{\epsilon \mu}
\end{equation}

\begin{equation}
\begin{bmatrix}
\BE \\
\BB \\
\end{bmatrix}
=
\begin{bmatrix}
\BE_0(\Br) \\
\BB_0(\Br) \\
\end{bmatrix}
e^{i \phi(\Br) - i \omega t}
\end{equation}


\begin{equation}
\spacegrad \cdot \BE = 
e^{-i \omega t}
\left(
\cancel{
e^{i \phi(\Br)}
\spacegrad \cdot \BE_0(\Br) 
}
+
\BE_0(\Br) \cdot \left( \spacegrad e^{i \phi(\Br)} \right)
\right)
\end{equation}

and
\begin{equation}
\spacegrad \cross \BE = 
e^{-i \omega t}
\left(
\cancel{
e^{i \phi(\Br)}
\spacegrad \cross \BE_0(\Br) 
}
-
\BE_0(\Br) \cross \left( \spacegrad e^{i \phi(\Br)} \right)
\right)
\end{equation}

\begin{subequations}

\begin{equation}
\BE_0 \cdot \spacegrad \phi = 0
\end{equation}
\begin{equation}
\BB_0 \cdot \spacegrad \phi = 0
\end{equation}
\begin{equation}
\spacegrad \phi \cross \BE_0 = k_0 \BB_0
\end{equation}
\begin{equation}
\spacegrad \phi \cross \BB_0 = - \epsilon k_0 \BE_0
\end{equation}
\end{subequations}

\begin{equation}
\Abs{\spacegrad \phi}^2 = k_0^2 \epsilon(\Br)
\end{equation}

\begin{equation}
\Abs{\spacegrad \phi} = k_0 n(\Br)
\end{equation}

\begin{equation}
\expectation{\BS} = \frac{c}{8 \pi k_0} \Abs{\BE_0}^2 \spacegrad \phi
\end{equation}

\begin{equation}
\Bt = \frac{d\Br(s)}{ds}
= \frac{\spacegrad \phi}{\Abs{\spacegrad \phi}} \\
= \frac{\spacegrad \phi}{ n(\Br) k_0}
\end{equation}

\begin{equation}
n(\Br) \frac{d\Br}{ds} = \inv{k_0} \spacegrad \phi
\end{equation}

\begin{equation}
\frac{d}{ds} \left( n(\Br) \frac{d\Br}{ds} \right) = \spacegrad n(\Br)
\end{equation}

\section{Wave relations}

\begin{equation}
k = \frac{2 \pi}{\lambda}
\end{equation}

\begin{equation}
\omega = 2 \pi \nu
\end{equation}

FIXME: relation between $k$ and $\omega$
%\begin{equation}
%k v = \omega \lambda \nu
%\end{equation}

\section{Electrodynamics}

\begin{align}
\spacegrad \cdot \BD &= 0 \\
\spacegrad \cdot \BB &= 0 \\
\spacegrad \cross \BE &= - \inv{c} \PD{t}{\BB} \\
\spacegrad \cross \BB &= \inv{c} \PD{t}{\BD}
\end{align}

\begin{equation}
\BD = \epsilon \BE
\end{equation}

\begin{equation}
\BS = \frac{c}{4 \pi} \Real{\BE} \cross \Real{\BB}
\end{equation}

\begin{dmath}
\LL_{\text{EM}} = \inv{c} \rho \phi + \inv{c} \Bj \cdot \BA + \inv{8 \pi} \BE^2 - \inv{8 \pi} \BB^2
\end{dmath}

\begin{align}
\BE &= \Real\left( \BE_0 e^{i \Bk \cdot \Bx - \omega t} \right) \\
\BB &= \Real\left( \BB_0 e^{i \Bk \cdot \Bx - \omega t} \right)
\end{align}

\begin{dmath}
\expectation{ \BE \cross \BB } = \inv{2} \Real( \BE_0 \cross \BB_0^\conj )
\end{dmath}

\section{Misc calculus results}

\begin{dmath}
\left(\spacegrad \phi \cdot \spacegrad \right) \spacegrad \phi
=
\inv{2} \spacegrad \left( \spacegrad \phi \right)^2
\end{dmath}

\begin{equation}
\spacegrad e^{i\phi} = i (\spacegrad \phi) e^{i \phi}
\end{equation}

\begin{dmath}
\spacegrad 
=
\rcap \PD{r}{} 
+\frac{\thetacap}{r} \PD{\theta}{} 
+\zcap \PD{z}{} 
\end{dmath}

\section{Diffraction}

\begin{align}
\BR &= \Br - \Br' \\
\BR_s &= \Br_s - \Br' \\
R &= \Abs{\BR} \\
R_s &= \Abs{\BR_s}
\end{align}

\begin{dmath}
\left( \spacegrad^2 + \Bk^2 \right) \Psi(\Br) = 0
\end{dmath}

\begin{dmath}
\Psi(\Br) = \iint da' \left( \Psi(\Br') \spacegrad' G - G \spacegrad' \Psi(\Br') \right) \cdot \ncap
\end{dmath}

\begin{dmath}
G(\Br, \Br') = -\frac{e^{i k R}}{4 \pi R} = -\frac{e^{i k \Abs{\Br - \Br'}}}{4 \pi \Abs{\Br - \Br'}},
\end{dmath}

\begin{dmath}
\spacegrad \left( 
\frac{ e^{i k r} }{r}
\right) = \rcap \left( i k - \inv{r} \right) 
\frac{e^{i k r}}{r}
\end{dmath}

\begin{dmath}
\Psi(\Br) = -\inv{4 \pi} \iint \frac{e^{i k R}}{R} 
\ncap \cdot 
\left( 
\spacegrad' \Psi(\Br') + \left( i k - \inv{R} \right) \frac{\BR}{R} \Psi(\Br') \right) 
da'
\end{dmath}

\begin{dmath}
\Psi(\Br) = \frac{A}{\lambda i} \iint da' \frac{e^{i k ( r + r_s)}}{r r_s} k(\theta)
\end{dmath}

\begin{dmath}
k(\theta) = \inv{2} \left( 1 + \cos \theta \right)
\end{dmath}

\begin{dmath}
k R = \underbrace{k r}_{O(r\lambda)} - \underbrace{k \rcap \cdot \Br'}_{O(d/\lambda)} + \underbrace{\frac{k}{2r} \left( {\Br'}^2 - \left( \rcap \cdot \Br' \right)^2 \right)}_{O(d^2/\lambda r)} + \underbrace{\cdots}_{O(d^3/\lambda r^2)}
\end{dmath}

\begin{dmath}
\Psi(\Br) 
= \frac{ A }{\lambda i} \frac{ e^{i k (r_s + r)}}{r_s r} \iint_{A} da' e^{i k f(\Br')}
\end{dmath}

\begin{dmath}
f(\Br') = - \left(\rcap + \rcap_s \right) \cdot \Br' + \inv{2r} \left( {\Br'}^2 - (\rcap \cdot \Br')^2 \right) + \inv{2 r_s} \left( (\Br')^2 - (\rcap_s \cdot \Br')^2 \right)
\end{dmath}

\begin{equation}
\rcap \sim (\alpha, \beta, 1)
\end{equation}

\begin{equation}
\Psi(\Br) = \frac{\Psi_s}{i \lambda} \frac{e^{i k f}}{f} \iint_A e^{-i k ( \alpha x' + \beta y' ) } da'.
\end{equation}

\begin{equation}
k f = \frac{k}{2} \left( 
r_s^{-1}
+r^{-1} \right) \left({x'}^2 + {y'}^2 \right) = \frac{\pi}{2} \left( u^2 + v^2 \right),
\end{equation}

\begin{dmath}
\Psi(\Br) 
= 
\frac{A}{2 i} e^{ik (r_s + r)} 
\frac{1}{r_s + r}
\int_{A} e^{i \frac{\pi}{2} (u^2 + v^2)} du dv
\end{dmath}

\begin{equation}
\int_{-\infty}^\infty dv e^{i \frac{\pi}{2} v^2 } = 1 + i = \sqrt{2} e^{i \pi/4}
\end{equation}

\begin{subequations}
\begin{equation}
S(w) = \int_0^w \sin \left( \frac{\pi}{2} u^2 \right) du
\end{equation}
\begin{equation}
C(w) = \int_0^w \cos \left( \frac{\pi}{2} u^2 \right) du
\end{equation}
\end{subequations}

\begin{equation}
1 = \left(\frac{dS}{dw}\right)^2 + \left(\frac{dC}{dw}\right)^2
\end{equation}

\begin{dmath}
\tan 
\left( \frac{\pi}{2} w^2 \right)
= \frac{dy}{dx}
\end{dmath}

\section{Coherence}

\begin{equation}
\expectation{ f(t) } = \lim_{T \rightarrow \infty } \inv{T} \int_0^T dt' f(t').
\end{equation}

\begin{align}
\Psi_1 &= \sqrt{I_1(\Br)} e^{i \phi_1(\Br, t)} \\
\Psi_2 &= \sqrt{I_2(\Br)} e^{i \phi_2(\Br, t)}.
\end{align}

\begin{dmath}
I 
= \Abs{\Psi_1 + \Psi_2}^2
= \Abs{\Psi_1}^2
+ \Abs{\Psi_2}^2
+ 2 \Real \expectation{ \Psi_1 \Psi_2^\conj}
\end{dmath}

\begin{equation}
V \equiv \frac
{
I_{\text{max}}
- I_{\text{min}}}
{
I_{\text{max}}
+ I_{\text{min}}
}
\end{equation}

\begin{dmath}
I 
= \expectation{ \Abs{\Psi}^2 }
= 
I(\Br_1) + 
I(\Br_2) + 
2 \Real \expectation{ \Psi(\Br_1, t) \Psi^\conj(\Br_2, t) }
\end{dmath}

\begin{dmath}
\Gamma_{12} \equiv
\expectation{ \Psi(\Br_1, t) \Psi^\conj(\Br_2, t) }
\end{dmath}

\begin{dmath}
\tau_{\text{coh}} = \inv{\Delta w}
\end{dmath}

\begin{dmath}
\gamma_{12} = \frac{\Gamma_{12}}{\sqrt{I_1} \sqrt{I_2}}
\end{dmath}

\section{Temporal coherence}

\begin{dmath}
I = I_1 + I_2 + 2 \sqrt{I_1 I_2} \Real \gamma_{12}
\end{dmath}

\begin{dmath}
\gamma(\tau) = \gamma_{12} = \FF \{ I(\omega) \}
\end{dmath}

\begin{dmath}
\tau = \frac{s_2 - s_1}{c}
\end{dmath}

\begin{dmath}
I = 
\Abs{\gamma_{12}} 
\left(
I_1 + I_2 + 2 \sqrt{I_1 I_2} \cos \left( \alpha_{12}(\tau) - \delta \right)
\right)
+ 
\left( 1 - \Abs{\gamma_{12}} \right) 
\left( I_1 + I_2 \right)
=
\Abs{\gamma_{12}} 
I_{\text{coh}}
+
(1 - \Abs{\gamma_{12}})
I_{\text{incoh}}
\end{dmath}

\begin{dmath}
\tau_a - \tau_b = \frac{
r_{1a}
-r_{2a}
-r_{1b}
+r_{2b}
}{c}
= 
\frac{l \theta_s}{c }
\end{dmath}

\begin{dmath}
k \left( R_1 - R_2 \right) \approx k \left( \Br_{\text{av}} - \Br_s \right) \cdot \frac{ \Delta \Br}{r_{\text{av}}}
\end{dmath}

\begin{equation}
\sum_{\Bk} I_{\Bk} e^{i \Bk \cdot \Bl} = \Gamma_{12} = \FF( I_{\Bk} )
\end{equation}

\begin{dmath}
I = \sum_{\Bk}
\Abs{
\Psi_k(\Br_1, t) + e^{i \Bk \cdot \Bl} \Psi_k(\Br_1, t) 
}^2
=
\sum \left( 
2 I_{\Bk} + 2 \Real \left( \Psi_k^\conj e^{i \Bk \cdot \Bl} \Psi_k \right)
     \right)
= 2 \sum I_\Bk + 2 \Real \left( 
\sum_{\Bk} I_{\Bk} e^{i \Bk \cdot \Bl}
\right)
\end{dmath}

\begin{equation}
\Gamma_{12} 
= 
e^{ i \Bk_{\text{av}} \cdot \Delta \Br }
\inv{ \lambda^2 \bar{R_1} \bar{R_2} }
\iint d^2 r_s e^{-i \Bk_s \cdot \Delta \Br } I( \Bk_s )
\end{equation}

where

\begin{subequations}
\begin{equation}
\Bk_s = k \frac{\Br_s}{r_{\text{av}}}
\end{equation}
\begin{equation}
\Bk_{\text{av}} = k \rcap_{\text{av}}
\end{equation}
\begin{equation}
\Delta \Br = \Br_1 - \Br_2
\end{equation}
\end{subequations}

\begin{dmath}\label{eqn:modernOptics:ProblemSet2:P3:490}
V = \frac
{
I_{\text{max}}
- I_{\text{max}}
}
{
I_{\text{max}}
+ I_{\text{max}}
}
= \Abs{\gamma_{12}}
=
2 \Abs{\frac{J_1(\pi \theta_s d/\lambda)}{\pi \theta_s d/\lambda}}.
\end{dmath}

\section{Fourier transforms}

\begin{dmath}
f(x) = g * h = \int_{-\infty}^\infty dx' g(x') h(x - x')
\end{dmath}

\begin{dmath}
F(k) = G(k) H(k)
\end{dmath}

\EndNoBibArticle
