\input{../peeter_prologue_print.tex}
%\input{../peeter_prologue_widescreen.tex}

\chapter{PHY450H1F: Quantum Mechanics II.  Lecture 4 (Taught by Prof J.E. Sipe).  Time independent pertubation theory (continued)}
\label{chap:qmTwoL4}
%\useCCL
\blogpage{http://sites.google.com/site/peeterjoot/math2011/qmTwoL4.pdf}
\date{Sept 21, 2011}
\revisionInfo{qmTwoL4.tex}

% subst: \Esn => {E_s}^{(n)}
% subst: \kpsi_s^n => \ket{{\psi_s}^{(n)}}
% subst: \kpsi_s => \ket{\psi_s}
% subst: \cns\d => {c_{ns}}^{(d)}
% subst: \cns => c_{ns}
%:,$ s/\\E\(.\)\(.\)/E_\1^{(\2)}/cg
%:,$ s/\\kpsi_\(.\)^\(.\)/\\ket{\\psi_\1^{(\2)}}/cg
%:,$ s/\\kpsi_\(.\)/\\ket{\\psi_\1}/cg
%:,$ s/\\cns\([0-9]\)/{c_{ns}}^{(\1)}/cg
%:,$ s/\\cns\>/c_{ns}/cg
\beginArtWithToc
%\beginArtNoToc

\section{Disclaimer.}

Peeter's lecture notes from class.  May not be entirely coherent.

\section{Time independent pertubation.}
\subsection{The setup}

To recap, we were covering the time independent pertubation methods from \S 16.1 of the text \cite{desai2009quantum}.  We start with a known Hamiltonian $H_0$, and alter it with the addition of a ``small'' pertubation

\begin{equation}\label{eqn:qmTwoL4:10}
H = H_0 + \lambda H', \qquad \lambda \in [0,1]
\end{equation}

For the original operator, we assume that a complete set of eigenvectors and eigenkets is known

\begin{equation}\label{eqn:qmTwoL4:30}
H_0 \ket{{\psi_0}^{(0)}} = {E_s}^{(0)} \ket{{\psi_s}^{(0)}}
\end{equation}

We seek the perturbed eigensolution

\begin{equation}\label{eqn:qmTwoL4:50}
H \ket{\psi_s} = E_s \ket{\psi_s}
\end{equation}

and assumed a pertubative series representation for the energy eigenvalues in the new system

\begin{equation}\label{eqn:qmTwoL4:70}
E_s = {E_s}^{(0)} + \lambda {E_s}^{(1)} + \lambda^2 {E_s}^{(2)} + \cdots
\end{equation}

Given an assumed representation for the new eigenkets in terms of the known basis

\begin{equation}\label{eqn:qmTwoL4:90}
\ket{\psi_s} = \sum_n c_{ns} \ket{{\psi_n}^{(0)}} 
\end{equation}

and a pertubative series representation for the probability coeffecients

\begin{equation}\label{eqn:qmTwoL4:110}
c_{ns} = {c_{ns}}^{(0)} + \lambda {c_{ns}}^{(1)} + \lambda^2 {c_{ns}}^{(2)},
\end{equation}

so that 

\begin{equation}\label{eqn:qmTwoL4:130}
\ket{\psi_s} = 
\sum_n {c_{ns}}^{(0)} \ket{{\psi_n}^{(0)}} 
+
\lambda
\sum_n {c_{ns}}^{(1)} \ket{{\psi_n}^{(0)}} 
+ 
\lambda^2
\sum_n {c_{ns}}^{(2)} \ket{{\psi_n}^{(0)}} 
+ \cdots
\end{equation}

Setting $\lambda = 0$ requires 

\begin{equation}\label{eqn:qmTwoL4:150}
{c_{ns}}^{(0)} = \delta_{ns},
\end{equation}

for

\begin{equation}\label{eqn:qmTwoL4:170}
\begin{aligned}
\ket{\psi_s} 
&= 
\ket{{\psi_s}^{(0)}} 
+
\lambda
\sum_n {c_{ns}}^{(1)} \ket{{\psi_n}^{(0)}} 
+ 
\lambda^2
\sum_n {c_{ns}}^{(2)} \ket{{\psi_n}^{(0)}} 
+ \cdots \\
&=
\left(
1 
+ \lambda {c_{ns}}^{(1)} 
+ \lambda^2 {c_{ns}}^{(2)} 
+ \cdots
\right)
\ket{{\psi_s}^{(0)}} 
+ 
\lambda
\sum_{n \ne s} {c_{ns}}^{(1)} \ket{{\psi_n}^{(0)}} 
+
\lambda^2
\sum_{n \ne s} {c_{ns}}^{(2)} \ket{{\psi_n}^{(0)}} 
+ \cdots
\end{aligned}
\end{equation}

We rescaled our kets 

\begin{equation}\label{eqn:qmTwoL4:190}
\ket{\bar{\psi}_s} 
=
\ket{{\psi_s}^{(0)}} 
+ 
\lambda
\sum_{n \ne s} {\bar{c}_{ns}}^{(1)} \ket{{\psi_n}^{(0)}} 
+
\lambda^2
\sum_{n \ne s} {\bar{c}_{ns}}^{(2)} \ket{{\psi_n}^{(0)}} 
+ \cdots
\end{equation}

where
\begin{equation}\label{eqn:qmTwoL4:210}
{\bar{c}_{ns}}^{(j)} = 
\frac{{c_{ns}}^{(j)}}
{
1 
+ \lambda {c_{ns}}^{(1)} 
+ \lambda^2 {c_{ns}}^{(2)} 
+ \cdots
}
\end{equation}

The normalization of the rescaled kets is then

\begin{equation}\label{eqn:qmTwoL4:230}
\braket{\bar{\psi}_s}{\bar{\psi}_s} 
=
1
+ 
\lambda^2
\sum_{n \ne s} \Abs{{\bar{c}_{ns}}^{(1)}}^2
+
\cdots
\equiv \inv{Z_s},
\end{equation}

One can then construct a renormalized ket if desired

\begin{equation}\label{eqn:qmTwoL4:250}
\ket{\bar{\psi}_s}_R = Z_s^{1/2} \ket{\bar{\psi}_s},
\end{equation}

so that
\begin{equation}\label{eqn:qmTwoL4:270}
(\ket{\bar{\psi}_s}_R)^\dagger \ket{\bar{\psi}_s}_R = Z_s \braket{\bar{\psi}_s}{\bar{\psi}_s} = 1.
\end{equation}

\subsection{The meat.}

That's as far as we got last time.  We continue by renaming terms in \ref{eqn:qmTwoL4:190}

\begin{equation}\label{eqn:qmTwoL4:300}
\ket{\bar{\psi}_s} 
=
\ket{{\psi_s}^{(0)}} 
+ 
\lambda \ket{{\psi_s}^{(1)}} 
+ 
\lambda^2 \ket{{\psi_s}^{(2)}} 
+ \cdots
\end{equation}

where

\begin{equation}\label{eqn:qmTwoL4:320}
\ket{{\psi_n}^{(j)}} = \sum_{n \ne s} {\bar{c}_{ns}}^{(j)} \ket{{\psi_s}^{(0)}}.
\end{equation}

Now we act on this with the Hamiltonian

\begin{equation}\label{eqn:qmTwoL4:340}
H \ket{\bar{\psi}_s} = E_s \ket{\bar{\psi}_s},
\end{equation}

or

\begin{equation}\label{eqn:qmTwoL4:360}
H \ket{\bar{\psi}_s} - E_s \ket{\bar{\psi}_s} = 0.
\end{equation}

Expanding this, we have
\begin{equation}\label{eqn:qmTwoL4:380}
\begin{aligned}
&(H_0 + \lambda H') 
\left(
\ket{{\psi_s}^{(0)}} 
+ 
\lambda \ket{{\psi_s}^{(1)}} 
+ 
\lambda^2 \ket{{\psi_s}^{(2)}} 
+ \cdots
\right) \\
&\quad - 
\left( {E_s}^{(0)} + \lambda {E_s}^{(1)} + \lambda^2 {E_s}^{(2)} + \cdots \right)
\left(
\ket{{\psi_s}^{(0)}} 
+ 
\lambda \ket{{\psi_s}^{(1)}} 
+ 
\lambda^2 \ket{{\psi_s}^{(2)}} 
+ \cdots
\right)
= 0.
\end{aligned}
\end{equation}

We want to write this as

\begin{equation}\label{eqn:qmTwoL4:400}
\ket{A} + \lambda \ket{B} + \lambda^2 \ket{C} + \cdots = 0.
\end{equation}

This is

\begin{equation}\label{eqn:qmTwoL4:420}
\begin{aligned}
0 &=
\lambda^0
(H_0 - E_s^{(0)}) \ket{{\psi_s}^{(0)}}  \\
&+ \lambda
\left(
(H_0 - E_s^{(0)}) \ket{{\psi_s}^{(1)}} 
+(H' - E_s^{(1)}) \ket{{\psi_s}^{(0)}} 
\right) \\
&+ \lambda^2
\left(
(H_0 - E_s^{(0)}) \ket{{\psi_s}^{(2)}} 
+(H' - E_s^{(1)}) \ket{{\psi_s}^{(1)}} 
-E_s^{(2)} \ket{{\psi_s}^{(0)}} 
\right) \\
&\cdots
\end{aligned}
\end{equation}

So we form

\begin{align}\label{eqn:qmTwoL4:440}
\ket{A} &=
(H_0 - E_s^{(0)}) \ket{{\psi_s}^{(0)}} \\
\ket{B} &=
(H_0 - E_s^{(0)}) \ket{{\psi_s}^{(1)}} 
+(H' - E_s^{(1)}) \ket{{\psi_s}^{(0)}} \\
\ket{C} &=
(H_0 - E_s^{(0)}) \ket{{\psi_s}^{(2)}} 
+(H' - E_s^{(1)}) \ket{{\psi_s}^{(1)}} 
-E_s^{(2)} \ket{{\psi_s}^{(0)}}  \\
&\vdots
\end{align}

\paragraph{Zeroth order in $\lambda$}

Since $H_0 \ket{{\psi_s}^{(0)}} = E_s^{(0)} \ket{{\psi_s}^{(0)}}$, this first condition on $\ket{A}$ is not much more than a statement that $0 - 0 = 0$.  

\paragraph{First order in $\lambda$}

How about $\ket{B} = 0$?  For this to be zero we require that both of the following are simulataneously zero

\begin{align}\label{eqn:qmTwoL4:460}
\braket{{\psi_s}^{(0)}}{B} &= 0 \\
\braket{{\psi_m}^{(0)}}{B} &= 0, \qquad m \ne s
\end{align}

This first condition is
\begin{equation}\label{eqn:qmTwoL4:480}
\bra{{\psi_s}^{(0)}} (H' - E_s^{(1)}) \ket{{\psi_s}^{(0)}} = 0.
\end{equation}

With
\begin{equation}\label{eqn:qmTwoL4:500}
\bra{{\psi_m}^{(0)}} H' \ket{{\psi_s}^{(0)}} \equiv {H_{ms}}',
\end{equation}

or
\begin{equation}\label{eqn:qmTwoL4:520}
{H_{ss}}' = E_s^{(1)}.
\end{equation}

From the second condition we have
\begin{equation}\label{eqn:qmTwoL4:540}
0 = \bra{{\psi_m}^{(0)}} 
(H_0 - E_s^{(0)}) \ket{{\psi_s}^{(1)}} 
+\bra{{\psi_m}^{(0)}} 
(H' - E_s^{(1)}) \ket{{\psi_s}^{(0)}} 
\end{equation}

Utilizing the Hermitian nature of $H_0$ we can act backwards on $\bra{{\psi_m}^{(0)}}$ 

\begin{equation}\label{eqn:qmTwoL4:560}
\bra{{\psi_m}^{(0)}} H_0
=
E_m^{(0)} \bra{{\psi_m}^{(0)}}.
\end{equation}

We note that $\braket{{\psi_m}^{(0)}}{{\psi_s}^{(0)}} = 0, m \ne s$.  We can also expand the $\braket{{\psi_m}^{(0)}}{{\psi_s}^{(1)}}$, which is

\begin{align*}
\braket{{\psi_m}^{(0)}}{{\psi_s}^{(1)}} 
&=
\bra{{\psi_m}^{(0)}}
\left(
\sum_{n \ne s} {\bar{c}_{ns}}^{(1)} \ket{{\psi_n}^{(0)}}
\right) \\
\end{align*}

I found that reducing this sum wasn't obvious until some actual integers were plugged in.  Suppose that $s = 3$, and $m = 5$, then this is

\begin{align*}
\braket{{\psi_5}^{(0)}}{{\psi_3}^{(1)}} 
&=
\bra{{\psi_5}^{(0)}}
\left(
\sum_{n = 0, 1, 2, 4, 5, \cdots} {\bar{c}_{n3}}^{(1)} \ket{{\psi_n}^{(0)}}
\right) \\
&=
\bra{{\psi_5}^{(0)}}
{\bar{c}_{53}}^{(1)} \braket{{\psi_5}^{(0)}}{{\psi_5}^{(0)}} \\
&=
{\bar{c}_{53}}^{(1)}.
\end{align*}

More generally that is
\begin{equation}\label{eqn:qmTwoL4:580}
\braket{{\psi_m}^{(0)}}{{\psi_s}^{(1)}} 
=
{\bar{c}_{ms}}^{(1)}.
\end{equation}

Utilizing this gives us
\begin{equation}\label{eqn:qmTwoL4:600}
0 = 
( E_m^{(0)} - E_s^{(0)}) 
{\bar{c}_{ms}}^{(1)}
+
{H_{ms}}' 
\end{equation}

And summarizing what we learn from our $\ket{B} = 0$ conditions we have

\begin{align}\label{eqn:qmTwoL4:620}
E_s^{(1)} &= {H_{ss}}' \\
{\bar{c}_{ms}}^{(1)}
&=
\frac{{H_{ms}}' }
{ E_s^{(0)} - E_m^{(0)} }
\end{align}

\paragraph{Second order in $\lambda$}

Doing the same thing for $\ket{C} = 0$ we form (or assume)

\begin{align}\label{eqn:qmTwoL4:640}
\braket{{\psi_s}^{(0)}}{C} &= 0 \\
\braket{{\psi_m}^{(0)}}{C} &= 0, \qquad m \ne s
\end{align}

\begin{align*}
0 
&= \braket{{\psi_s}^{(0)}}{C}  \\
&=
\bra{{\psi_s}^{(0)}}
\left(
(H_0 - E_s^{(0)}) \ket{{\psi_s}^{(2)}} 
+(H' - E_s^{(1)}) \ket{{\psi_s}^{(1)}} 
-E_s^{(2)} \ket{{\psi_s}^{(0)}}  
\right) \\
&=
(E_s^{(0)} - E_s^{(0)}) 
\braket{{\psi_s}^{(0)}}{{\psi_s}^{(2)}} 
+
\bra{{\psi_s}^{(0)}}
(H' - E_s^{(1)}) \ket{{\psi_s}^{(1)}} 
-E_s^{(2)} \braket{{\psi_s}^{(0)}}{{\psi_s}^{(0)}} 
\end{align*}

We need to know what the $\braket{{\psi_s}^{(0)}}{{\psi_s}^{(1)}}$ is, and find that it is zero

\begin{equation}\label{eqn:qmTwoL4:660}
\braket{{\psi_s}^{(0)}}{{\psi_s}^{(1)}}
=
\bra{{\psi_s}^{(0)}}
\sum_{n \ne s} {\bar{c}_{ns}}^{(1)} \ket{{\psi_n}^{(0)}}
\end{equation}

Again, suppose that $s = 3$.  Our sum ranges over all $n \ne 3$, so all the brakets are zero.  Utilizing that we have

\begin{align*}
E_s^{(2)} 
&=
\bra{{\psi_s}^{(0)}} H' \ket{{\psi_s}^{(1)}}  \\
&=
\bra{{\psi_s}^{(0)}} H' \sum_{m \ne s} {\bar{c}_{ms}}^{(1)} \ket{{\psi_m}^{(0)}} \\
&=
\sum_{m \ne s} {\bar{c}_{ms}}^{(1)} {H_{sm}}'
\end{align*}

From \ref{eqn:qmTwoL4:620} we have

\begin{equation}\label{eqn:qmTwoL4:n}
E_s^{(2)} 
=
\sum_{m \ne s} 
\frac{{H_{ms}}' }
{ E_s^{(0)} - E_m^{(0)} }
{H_{sm}}'
=
\sum_{m \ne s} 
\frac{\Abs{{H_{ms}}'}^2 }
{ E_s^{(0)} - E_m^{(0)} }
\end{equation}

\EndArticle
