\input{../peeter_prologue_print.tex}
%\input{../peeter_prologue_widescreen.tex}

\chapter{PHY450H1S.  Relativistic Electrodynamics Tutorial 4 (TA: Simon Freedman).  Waveguides: confined EM waves.}
\label{chap:relativisticElectrodynamicsT4}
%\useCCL
\blogpage{http://sites.google.com/site/peeterjoot/math2011/relativisticElectrodynamicsT4.pdf}
\date{Mar 3, 2011}
\revisionInfo{relativisticElectrodynamicsT4.tex}

\beginArtWithToc
%\beginArtNoToc

\section{Motivation}

While this isn't part of the course, the topic of waveguides is one of so many applications that it is worth a mention, and that will be done in this tutorial.

We will setup our system with a waveguide (conducting surface that confines the radiation) oriented in the $\zcap$ direction.  The shape can be arbitrary

PICTURE: cross section of wacky shape.

\subsection{At the surface of a conductor.}

At the surface of the conductor (I presume this means the interior surface where there is no charge or current enclosed) we have

\begin{align}\label{eqn:relativisticElectrodynamicsT4:10}
\spacegrad \cross \BE &= - \inv{c} \PD{t}{\BB} \\
\spacegrad \cross \BB &= \inv{c} \PD{t}{\BE} \\
\spacegrad \cdot \BB &= 0 \\
\spacegrad \cdot \BE &= 0
\end{align}

If we are talking about the exterior surface, do we need to make any other assumptions (perfect conductors, or constant potentials)?

\subsection{Wave equations.}

For electric and magnetic fields in vacuum, we can show easily that these, like the potentials, separately satisfy the wave equation

Taking curls of the Maxwell curl equations above we have

\begin{align}\label{eqn:relativisticElectrodynamicsT4:30}
\spacegrad \cross (\spacegrad \cross \BE) &= - \inv{c^2} \PDSq{t}{\BE} \\
\spacegrad \cross (\spacegrad \cross \BB) &= - \inv{c^2} \PDSq{t}{\BB},
\end{align}

but we have for vector $\BM$

\begin{equation}\label{eqn:relativisticElectrodynamicsT4:50}
\spacegrad \cross (\spacegrad \cross \BM)
=
\spacegrad (\spacegrad \cdot \BM) - \Delta \BM,
\end{equation}

which gives us a pair of wave equations

\begin{align}\label{eqn:relativisticElectrodynamicsT4:70}
\square \BE &= 0 \\
\square \BB &= 0.
\end{align}

We still have the original constraints of Maxwell's equations to deal with, but we are free now to pick the complex exponentials as fundamental solutions, as our starting point

\begin{align}\label{eqn:relativisticElectrodynamicsT4:90}
\BE &= \BE_0 e^{i k^a x_a} = \BE_0 e^{ i (k^0 x_0 - \Bk \cdot \Bx) } \\
\BB &= \BB_0 e^{i k^a x_a} = \BB_0 e^{ i (k^0 x_0 - \Bk \cdot \Bx) },
\end{align}

With $k_0 = \omega/c$ and $x_0 = c t$ this is

\begin{align}\label{eqn:relativisticElectrodynamicsT4:110}
\BE &= \BE_0 e^{ i (\omega t - \Bk \cdot \Bx) } \\
\BB &= \BB_0 e^{ i (\omega t - \Bk \cdot \Bx) }.
\end{align}

For the vacuum case, with monochromatic light, we treated the amplitudes as constants.  Let's see what happens if we relax this assumption, and allow for spatial dependence (but no time dependence) of $\BE_0$ and $\BB_0$.  For the LHS of the electric field curl equation we have

\begin{align*}
0 
&= \spacegrad \cross \BE_0 e^{i k_a x^a} \\
&= (\spacegrad \cross \BE_0 - \BE_0 \cross \spacegrad) e^{i k_a x^a} \\
&= (\spacegrad \cross \BE_0 - \BE_0 \cross \Be^\alpha i k_a \partial_\alpha x^a) e^{i k_a x^a} \\
&= (\spacegrad \cross \BE_0 + \BE_0 \cross \Be^\alpha i k^a {\delta_\alpha}^a ) e^{i k_a x^a} \\
&= (\spacegrad \cross \BE_0 + i \BE_0 \cross \Bk ) e^{i k_a x^a}.
\end{align*}

Similarly for the divergence we have

\begin{align*}
0 
&= \spacegrad \cdot \BE_0 e^{i k_a x^a} \\
&= (\spacegrad \cdot \BE_0 + \BE_0 \cdot \spacegrad) e^{i k_a x^a} \\
&= (\spacegrad \cdot \BE_0 + \BE_0 \cdot \Be^\alpha i k_a \partial_\alpha x^a) e^{i k_a x^a} \\
&= (\spacegrad \cdot \BE_0 - \BE_0 \cdot \Be^\alpha i k^a {\delta_\alpha}^a ) e^{i k_a x^a} \\
&= (\spacegrad \cdot \BE_0 - i \Bk \cdot \BE_0 ) e^{i k_a x^a}.
\end{align*}

This provides constraints on the amplitudes

\begin{align}\label{eqn:relativisticElectrodynamicsT4:130}
\spacegrad \cross \BE_0 - i \Bk \cross \BE_0 &= -i \frac{\omega}{c} \BB_0 \\
\spacegrad \cross \BB_0 - i \Bk \cross \BB_0 &= i \frac{\omega}{c} \BE_0 \\
\spacegrad \cdot \BE_0 - i \Bk \cdot \BE_0 &= 0 \\
\spacegrad \cdot \BB_0 - i \Bk \cdot \BB_0 &= 0
\end{align}

%Having seen that taking curls of the curl equations gave us the wave equation, let's see what happens when we do so in momentum space.  It is worth recalling that
%
%\begin{equation}\label{eqn:relativisticElectrodynamicsT4:150}
%\spacegrad \cross (\Bk \cross \BM) = \Bk (\spacegrad \cdot \BM) - (\Bk \cdot \spacegrad) \BM,
%\end{equation}
%
%where $\Bk$ is a constant, and $\BM$ is not.  We have
%
%\begin{align*}
%\spacegrad (\spacegrad \cdot \BE_0) - \Delta \BE_0 - i (
%\Bk (\spacegrad \cdot \BE_0) - (\Bk \cdot \spacegrad) \BE_0
%) &= -i \frac{\omega}{c} \spacegrad \cross \BB_0.
%\end{align*}
%
%This doesn't look like it will be terribly helpful.  Backing up, and 
Applying the wave equation operator to our phasor we get

\begin{align*}
0 &=
\left(\inv{c^2} \partial_{tt} - \spacegrad^2 \right) \BE_0 e^{i (\omega t - \Bk \cdot \Bx)} \\
&=
\left(-\frac{\omega^2}{c^2} - \spacegrad^2 + \Bk^2 \right) \BE_0 e^{i (\omega t - \Bk \cdot \Bx)}
\end{align*}

So the momentum space equivalents of the wave equations are

\begin{align}\label{eqn:relativisticElectrodynamicsT4:170}
\left( \spacegrad^2 +\frac{\omega^2}{c^2} - \Bk^2 \right) \BE_0 &= 0 \\
\left( \spacegrad^2 +\frac{\omega^2}{c^2} - \Bk^2 \right) \BB_0 &= 0.
\end{align}

Observe that if $c^2 \Bk^2 = \omega^2$, then these amplitudes are harmonic functions (solutions to the Laplacian equation).  However, it doesn't appear that we require such a light like relation for the four vector $k^a = (\omega/c, \Bk)$.

\section{Back to the tutorial notes.}

In class we went straight to an assumed solution of the form

\begin{align}\label{eqn:relativisticElectrodynamicsT4:190}
\BE &= \BE_0(x, y) e^{ i(\omega t - k z) } \\
\BB &= \BB_0(x, y) e^{ i(\omega t - k z) },
\end{align}

where $\Bk = k \zcap$.  Our Laplacian was also written as the sum of components in the propagation and perpendicular directions

\begin{equation}\label{eqn:relativisticElectrodynamicsT4:210}
\spacegrad^2 = \PDSq{x_\perp}{} + \PDSq{z}{}.
\end{equation}

With no $z$ dependence in the amplitudes we have

\begin{align}\label{eqn:relativisticElectrodynamicsT4:170}
\left( \PDSq{x_\perp} +\frac{\omega^2}{c^2} - \Bk^2 \right) \BE_0 &= 0 \\
\left( \PDSq{x_\perp} +\frac{\omega^2}{c^2} - \Bk^2 \right) \BB_0 &= 0.
\end{align}

Splitting $\BE_0$, $\BB_0$ in components $\BE_0 = \BE_\perp + \BE_z$ and $\BB_0 = \BB_\perp + \BB_z$ in the propagation direction, and components in the perpendicular direction we have 

\begin{align*}
\spacegrad \cross \BE_0 
&=
(\spacegrad_\perp + \zcap\partial_z) \cross \BE_0 \\
&=
\spacegrad_\perp \cross \BE_0 \\
&=
\spacegrad_\perp \cross (\BE_\perp + \BE_z) \\
&=
\spacegrad_\perp \cross \BE_\perp 
+\spacegrad_\perp \cross \BE_z \\
&=
( \xcap \partial_x +\ycap \partial_y ) \cross ( \xcap E_x +\ycap E_y ) 
+\spacegrad_\perp \cross \BE_z \\
&=
\zcap (\partial_x E_y - \partial_z E_z) 
+\spacegrad_\perp \cross \BE_z.
\end{align*}

We can do something similar for $\BB_0$.  This allows for a split of \ref{eqn:relativisticElectrodynamicsT4:130} into $\zcap$ and perpendicular components

\begin{align}\label{eqn:relativisticElectrodynamicsT4:130}
% zcap terms
\spacegrad_\perp \cross \BE_\perp &= -i \frac{\omega}{c} \BB_z \\
\spacegrad_\perp \cross \BB_\perp &= i \frac{\omega}{c} \BE_z \\
% perp terms
\spacegrad_\perp \cross \BE_z - i \Bk \cross \BE_\perp &= -i \frac{\omega}{c} \BB_\perp \\
\spacegrad_\perp \cross \BB_z - i \Bk \cross \BB_\perp &= i \frac{\omega}{c} \BE_\perp \\
\spacegrad_\perp \cdot \BE_\perp &= i k E_z - \partial_z E_z \\
\spacegrad_\perp \cdot \BB_\perp &= i k B_z - \partial_z B_z
\end{align}

%where $k^0 x_0 = \Bk \cdot \Bx$.  

%\EndArticle
\EndNoBibArticle
