\input{../peeter_prologue_print.tex}
%\input{../peeter_prologue_widescreen.tex}

\chapter{PHY450H1S.  Relativistic Electrodynamics Lecture 15 (Taught by Prof. Erich Poppitz).  FIXME.}
\label{chap:relativisticElectrodynamicsL15}
%\useCCL
\blogpage{http://sites.google.com/site/peeterjoot/math2011/relativisticElectrodynamicsL15.pdf}
\date{Feb 16, 2011}
\revisionInfo{relativisticElectrodynamicsL15.tex}

%\beginArtWithToc
\beginArtNoToc

\section{Reading.}

Covering chapter 4 material from the text \cite{landau1980classical}.

Covering \href{http://www.physics.utoronto.ca/~poppitz/e-poppitz/PHY450_files/RelEMpp115-127.pdf}{lecture notes pp. 115-127}: reminder on wave equations (115); reminder on Fourier series and integral (115-117); Fourier expansion of the EM potential in Coulomb gauge and equation of motion for the spatial Fourier components (118-119); the general solution of Maxwell's equations in vacuum (120-121) [Tuesday, Mar. 1]; properties of monochromatic plane EM waves (122-124); energy and energy flux of the EM field and energy conservation from the equations of motion (125-127)  [Wednesday, Mar. 2]

\section{Review of wave equation results obtained.}

Maxwell's equations in vacuum lead to Coulomb gauge and the Lorentz gauge.

Coulomb gauge

\begin{align}\label{eqn:relativisticElectrodynamicsL15:n}
A^0 &= 0 \\
\spacegrad \cdot \BA &= 0
\left( \inv{c^2} \PDSq{t}{} - \Delta \right) \BA &= 0
\end{align}

Lorentz gauge

\begin{align}\label{eqn:relativisticElectrodynamicsL15:n}
\partial_i A^i &= 0 \\
\left( \inv{c^2} \PDSq{t}{} - \Delta \right) A^i &= 0
\end{align}

Note that $\partial_i A^i = 0$ is invariant under gauge transformations

\begin{equation}\label{eqn:relativisticElectrodynamicsL15:n}
A^i \rightarrow A^i + \partial^i \chi
\end{equation}

where 

\begin{equation}\label{eqn:relativisticElectrodynamicsL15:n}
\partial_i \partial^i \chi = 0
\end{equation}

i.e.  If one uses the Lorentz gauge, this has to be fixed.

However, in both cases we have 

\begin{equation}\label{eqn:relativisticElectrodynamicsL15:n}
\left( \inv{c^2} \PDSq{t}{} - \Delta \right) f = 0
\end{equation}

where 

\begin{equation}\label{eqn:relativisticElectrodynamicsL15:n}
\inv{c^2} \PDSq{t}{} - \Delta 
\end{equation}

is the wave operator.

Consider 

\begin{equation}\label{eqn:relativisticElectrodynamicsL15:n}
\Delta = \PDSq{x}{}
\end{equation}

where we are looking for a solution that is independent of $y, z$.  Recall that the general solution for this equation has the form

\begin{equation}\label{eqn:relativisticElectrodynamicsL15:n}
f(t, x) = 
F_1 \left(t - \frac{x}{c}\right)
+F_2 \left(t + \frac{x}{c}\right)
\end{equation}

PICTURE: superposition of two waves with $F_1$ moving along the x-axis in the positive direction, and $F_2$ in the negative x direction.

\section{Review of Fourier methods.}

It is often convienent to impose periodic boundary conditions

\begin{equation}\label{eqn:relativisticElectrodynamicsL15:n}
\BA(\Bx + \Be_i L) = \BA(\Bx), i = 1,2,3
\end{equation}

\subsection{In one dimension}

\begin{equation}\label{eqn:relativisticElectrodynamicsL15:n}
f(x + L) = f(x)
\end{equation}

\begin{equation}\label{eqn:relativisticElectrodynamicsL15:n}
f(x) = \sum_{n=-\infty}^\infty e^{i \frac{2 \pi n}{L} x} \tilde{f}_n
\end{equation}

When $f(x)$ is real we also have

\begin{equation}\label{eqn:relativisticElectrodynamicsL15:n}
f^\conj(x) = \sum_{n = -\infty}^\infty e^{-i \frac{2 \pi n}{L} x} (\tilde{f}_n)^\conj
\end{equation}

which implies

FIXME: DIY: 

\begin{equation}\label{eqn:relativisticElectrodynamicsL15:n}
{\tilde{f}^\conj}_{n} = \tilde{f}_{-n}
\end{equation}

Write 

\begin{equation}\label{eqn:relativisticElectrodynamicsL15:n}
k_n = \frac{2 \pi n}{L}
\end{equation}

This is the wave number, giving us

\begin{equation}\label{eqn:relativisticElectrodynamicsL15:n}
f(x) = \sum_{n=-\infty}^\infty e^{i k_n x} \tilde{f}_{k_n}
\end{equation}

The inverse transform is obtained by integration

\begin{equation}\label{eqn:relativisticElectrodynamicsL15:n}
f_{k_n} = \inv{L} \int_{-L/2}^{L/2} dx e^{-i k_n x} f(x)
\end{equation}

Verify: 
\begin{align*}
f_{k_n} 
&= \inv{L} \int_{-L/2}^{L/2} dx e^{-i k_n x} \sum_{m=-\infty}^\infty e^{i k_m x} \tilde{f}_{k_m} \\
&= ...  \\
&DIY: \\
&= \sum_{m = -\infty}^\infty \tilde{f}_{k_m} \delta_{mn} = \tilde{f}_{k_m}
\end{align*}

It is conventional to absorb $\tilde{f}_{k_n} = \tilde{f}(k_n)$ for

\begin{equation}\label{eqn:relativisticElectrodynamicsL15:n}
f(x) = \inv{L} \sum_n \tilde{f}(k_n) e^{i k_n x}
\tilde{f}(k_n) = \int_{-L/2}^{L/2} dx f(x) e^{-i k_n x}
\end{equation}

To take $L -> \infty$ notice

\begin{equation}\label{eqn:relativisticElectrodynamicsL15:n}
k_n = \frac{2 \pi}{L} n
\end{equation}

when $n$ changes by $\Delta n = 1$, $k_n$ changes by $\Delta k_n = \frac{2 \pi}{L} \Delta n$

Using this 

\begin{equation}\label{eqn:relativisticElectrodynamicsL15:n}
f(x) = \inv{2\pi} \sum_n \left( \frac{2\pi}{L} \delta n \right) \tilde{f}(k_n) e^{i k_n x}
\end{equation}

With $L -> \infty$, and $\Delta k_n \rightarrow 0$

\begin{equation}\label{eqn:relativisticElectrodynamicsL15:n}
f(x) = \frac{dk}{2\pi} \tilde{f}(k_n) e^{i k_n x}
\end{equation}

Verify:

\begin{equation}\label{eqn:relativisticElectrodynamicsL15:n}
f(x) = \int \frac{dk}{2\pi} \tilde{f}(k_n) e^{i k x}
\end{equation}

\begin{equation}\label{eqn:relativisticElectrodynamicsL15:n}
\tilde{f}(k) = \int dx f(x) e^{-i k x}
\end{equation}

With
\begin{equation}\label{eqn:relativisticElectrodynamicsL15:n}
\int dk e^{i k (x - y)} = 2 \pi \delta(x - y)
\end{equation}

we verify the inverse relation.

=> FIXME:DIY:

\subsection{In three dimensions}

\begin{align}\label{eqn:relativisticElectrodynamicsL15:n}
\BA(\Bx, t) &= \iiint_{-\infty}^\infty \tilde{\BA}(\Bk, t) e^{i \Bk \cdot \Bx} \\
\tilde{\BA}(\Bx, t) &= \iiint_{-\infty}^\infty \BA(\Bx, t) e^{-i \Bk \cdot \Bx}
\end{align}

\subsection{Application to the wave equation}

\begin{align*}
0 &= 
\left( \inv{c^2} \PDSq{t}{} - \Delta \right) \BA(\Bx, t) \\
&=
\left( \inv{c^2} \PDSq{t}{} - \Delta \right) \BA(\Bx, t)
\int \tilde{\BA}(\Bk, t) e^{i \Bk \cdot \Bx} \\
&=
\int 
\left( 
\inv{c^2} \partial_{tt} \tilde{\BA}(\Bk, t) + \Bk^2 \BA(\Bk, t)
\right)
e^{i \Bk \cdot \Bx} 
\end{align*}

Now operate with $\int d^3 \Bx e^{-i \Bp \cdot \Bx }$

\begin{align*}
0 &=
\int d^3 \Bx e^{-i \Bp \cdot \Bx }
\int 
\left( 
\inv{c^2} \partial_{tt} \tilde{\BA}(\Bk, t) + \Bk^2 \BA(\Bk, t)
\right)
e^{i \Bk \cdot \Bx}  \\
&=
\int \frac{d^3 \Bk}{2\pi} (2\pi)^3 \delta^3(\Bp -\Bk) 
\left( 
\inv{c^2} \partial_{tt} \tilde{\BA}(\Bk, t) + \Bk^2 \BA(\Bk, t)
\right)
\end{align*}

Since this is true for all $\Bp$ we have

\begin{equation}\label{eqn:relativisticElectrodynamicsL15:n}
\partial_{tt} \tilde{\BA}(\Bp, t) = -c^2 \Bp^2 \tilde{\BA}(\Bp, t) 
\end{equation}

For every value of momentum we have a harmonic osciallator!

\begin{equation}\label{eqn:relativisticElectrodynamicsL15:n}
\ddot{x} = -\omega^2 x
\end{equation}

Fourier modes of EM potential in vacuum obey

\partial_{tt} \tilde{\BA}(\Bk, t) = -c^2 \Bk^2 \tilde{\BA}(\Bk, t)

FIXME: DIY:

\spacegrad \cdot \BA(\Bx, t) = 0

=> 

\begin{align*}
0 
&= \int \frac{d^3 \Bk }{(2 \pi)^3} \spacegrad e^{i \Bk \cdot \Bx} \cdot \TBA(\Bk, t)
\end{align*}

e^{i \Bk \cdot \Bx} i \Bk \cdot \BA(\Bk, t)

=> 

\begin{align}\label{eqn:relativisticElectrodynamicsL15:n}
\TBA(-\Bk, t) &= \TBA^\conj(\Bk, t)
\Bk \cdot \TBA(\Bk, t) &= 0
\end{align}

\BA(\Bx, t) = \int d3k/2p^3 e^{i \Bk \cdot \Bx} \left( \inv{2} \TBA(\Bk, t) + \inv{2} \TBA^\conj(- \Bk, t) \right)

Since we have

\partial_{tt} \TBA(\Bk, t) = - \omega_k^2 \TBA(\Bk, t)

gives general solution 

\TBA(\Bk, t) = e^{i \omega_k t} \Ba_{+}(\Bk) +e^{-i \omega_k t} \Ba_{-}(\Bk)
\TBA^\conj(\Bk, t) = e^{-i \omega_k t} \Ba_{+}^\conj(\Bk) +e^{i \omega_k t} \Ba_{-}^\conj(\Bk)


\BA(\Bx, t) 
= \int d3k/2pi^3 e^{i \Bk \cdot \Bx} 
\inv{2} \left( 
e^{i \omega_k t} (\Ba_p(\Bk) + \Ba_m^\conj(-\Bk)) 
+e^{-i \omega_k t} (\Ba_m(\Bk) + \Ba_p^\conj(-\Bk)) 
\right)

Define

\Bbeta(\Bk) \equiv \Ba_m(\Bk) + \Ba_p^\conj(-\Bk) 

so that

\Bbeta(-\Bk) = \Ba_p(\Bk) + \Ba_p^\conj(-\Bk)

This is now manifestly real

\begin{equation}\label{eqn:relativisticElectrodynamicsL15:n}
\BA(\Bx, t) = \int d3k/2pi^3 \left( 
e^{i (\Bk \cdot \Bx + \omega_k t) \Bbeta^\conj(-\Bk)
+e^{i (\Bk \cdot \Bx - \omega_k t) \Bbeta(\Bk)
\end{equation}

With $\Bk \cdot \Bbeta(\Bk)  = 0$

CHANGE: EXAM: 7-9 MONDAY!!!

\EndArticle
