\input{../peeter_prologue_print.tex}
%\input{../peeter_prologue_widescreen.tex}

\chapter{PHY450H1S.  Relativistic Electrodynamics Tutorial 3 (TA: Simon Freedman).  XXX FIXME TITLE XXX.}
\label{chap:relativisticElectrodynamicsT3}
%\useCCL
\blogpage{http://sites.google.com/site/peeterjoot/math2011/relativisticElectrodynamicsT3.pdf}
\date{Feb 3, 2011}
\revisionInfo{relativisticElectrodynamicsT3.tex}

\beginArtWithToc
%\beginArtNoToc

\section{Motion in an constant uniform Electric field.}

\begin{equation}\label{eqn:relativisticElectrodynamicsT3:n}
\BE = E \xcap
\end{equation}

\begin{equation}\label{eqn:relativisticElectrodynamicsT3:n}
\BF = e ( \BE + \frac{\Bv}{c} \cross \BH ) = e ( \BE )
\end{equation}

Our force is the rate of change of momentum, but we will want the relativistic momentum

\begin{equation}\label{eqn:relativisticElectrodynamicsT3:n}
\frac{d\Bp}{dt} = \frac{d m \gamma \Bv}{dt} = e \BE 
\end{equation}

Or 

pdot_x = e E
pdot_y = \text{constant}

e E t + p_x(0)
&=
m xdot/SQR = e E t
&= 

m^2/(e E t)^2 \xdot^2 =\left( 1 - \frac{xdot^2 - ydot^2}{c^2}

where we let p_x(0) = 0

\xdot^2 = \frac{c^2 - ydot^2}{1 + (mc/eEt)^2}


Or

p_y = p_0

m ydot/SQR = p_y(0)

c^2 m^2/p_y(0)^2 \ydot^2 = c^2 - \xdot^2 - ydot^2

ydot^2 = \frac{ p_y(0)^2 (c^2 - xdot^2)}{1 + m^2 c^2/p_y(0)^2

Observe that 

\Epsilon^2 = p_0^2 c^2 + m^2 c^4

so we can write

ydot^2 = \frac{ c^2 p_0^2 (c^2 - xdot^2)}{ \Epsilon_0^2 }


Subst

\xdot = \frac{c^2 e \Epsilon t}{\sqrt{ \Epsilon_0^2 + (e c \Epsilon t)^2 }
\ydot = \frac{c p_0^2 }{\sqrt{ \Epsilon_0^2 + (e c \Epsilon t)^2 }

Tricky way also possible (as in the text)

\Bp = m \gamma \Bv 
\Epsilon = \gamma m c^2 

Solve for $\Bp$ and get

\Bp = \frac{\Epsilon \Bv}{c^2}

implies

\xdot = \frac{c^2 p_x}{\Epsilon}

Solving for $x$ we have

x(t) = c^2 e E \int \frac{dt' t'}{\sqrt{ \Epsilon_0^2 + (e c E t)^2 }}

Can solve with hyperbolic subst or

x(t) = c^2 e E \int \frac{dt' t'}{\sqrt{ \Epsilon_0^2 + (e c E t)^2 }}

du^2 = 2 u du \implies u du = \inv{2} d(u^2)

x(t) = \frac{c^2 e E}{2 \Epsilon_0} \int \frac{d (u^2)}{\sqrt{ 1 + \left(\frac{e c E}{\Epsilon_0}\right)^2 u^2 }}

Solving this we get

x(t) = \inv{e E} \sqrt{ \Epsilon_0^2 + (e c E t)^2 }

or

x^2 - c^2 t^2 = \frac{E_0^2}{ e^2 E^2 } = a^{-2}

y(t) = c^2 p_0^2 \int \frac{dt}{\sqrt{\Epsilon_0^2 + (e c E t)^2 }

t = \frac{E_0}{ e c E} \sinh(u) 

dt = \frac{E_0}{ e c E} \cosh(u) du

y(t) 
&= \frac{c^2 p_0^2}{\Epsilon_0} \int \frac{dt}{\sqrt{1 + (\frac{e c E}{\Epsilon_0)})^2 t^2 }
&= \frac{c^2 p_0^2}{\Epsilon_0} 
\frac{E_0}{ e c E} \cosh(u) du
\int \frac{ du \cosh u }{\sqrt{1 + (\sinh u)^2 }
&= \frac{c p_0}{ e E} u \\

for

boxed:
y(t) &= \frac{c p_0}{ e E} \sinh^{-1} \left( \frac{e c E t}{\Epsilon_0} \right) \\
x(y) &= \frac{\Epsilon_0}{c E} \cosh( y e E / c p_0 )

v \rightarrow c, t \rightarrow \infty

v << c, t \rightarrow 0

m v_x = e E t + ...
x \similar t^2 

m v_y = p_0 -> y \similar t

x(y) \similar y^2

(a parabola)

\section{Motion in an constant uniform Magnetic field.}

Note that the magnetic field does no work

\BF = e/c \Bv \cross \BH

dW = 
\BF \cdot d\Bl
&=
e/c (\Bv \cross \BH) \cdot d\Bl
&= 0

(perpendicular)

So our energy is only the initial time value

\E = .... + e A^0

\E(t) = \E_0

\BH = H \zcap

\delta_{\alpha 3} H = H_\alpha

\Bp = \E \Bv/c^2 = \E_0 \Bv/c^2 

=> 

\Bv = \Bp c^2/\E_0

\dot{\Bv} = \dot{\Bp} c^2/\E_0

\vdot_\alpha = \frac{e c}{\E_0} \epsilon_{\alpha \beta \gamma} v^\beta H_\gamma

write

\omega = e c H /\E_0

for (eval delta -> show)
\vdot_\alpha = \omega \epsilon_{\alpha \beta 3} v_\beta 

\vdot_1 = \omega \epsilon_{1 \beta 3} v_\beta = \omega v_2
\vdot_2 = \omega \epsilon_{2 \beta 3} v_\beta = - \omega v_1
\vdot_3 = \omega \epsilon_{3 \beta 3} v_\beta = 0

show:
ddt ( v_1 + i v_2 ) = -i \omega ( v_1 + i v_2 )
z = v_1 + i v_2 

=> 

z = V_0 e^{-i \omega z t + i \alpha}

=> 
v_1(t) = V_0 \cos( \omega z t + \alpha)
v_2(t) = -V_0 \sin( \omega z t + \alpha)

x_1(t) = x_1(0) + V_0 \sin( \omega z t + \alpha)
x_2(t) = x_2(0) + V_0 \cos( \omega z t + \alpha)

=> A helix.

%\EndArticle
\EndNoBibArticle
