%
% Copyright © 2015 Peeter Joot.  All Rights Reserved.
% Licenced as described in the file LICENSE under the root directory of this GIT repository.
%
\input{../blogpost.tex}
\renewcommand{\basename}{simplestTwoByTwoPerturbation}
\renewcommand{\dirname}{notes/phy1520/}
%\newcommand{\dateintitle}{}
%\newcommand{\keywords}{}

\input{../peeter_prologue_print2.tex}

\usepackage{peeters_layout_exercise}
\usepackage{peeters_braket}
\usepackage{peeters_figures}
\usepackage{enumerate}

\beginArtNoToc

\generatetitle{Simplest perturbation two by two Hamiltonian}
%\chapter{Simplest perturbation two by two Hamiltonian}
%\label{chap:simplestTwoByTwoPerturbation}

%\makeoproblem{}{problem:simplestTwoByTwoPerturbation:1}{\citep{sakurai2014modern} pr. 5.11}{
%
%\makesubproblem{}{problem:simplestTwoByTwoPerturbation:1:a}
%\makesubproblem{}{problem:simplestTwoByTwoPerturbation:1:b}
%\makesubproblem{}{problem:simplestTwoByTwoPerturbation:1:c}
%
%} % problem
%
%\makeanswer{problem:simplestTwoByTwoPerturbation:1}{
%
%\makeSubAnswer{}{problem:simplestTwoByTwoPerturbation:1:a}
%\makeSubAnswer{}{problem:simplestTwoByTwoPerturbation:1:b}
%\makeSubAnswer{}{problem:simplestTwoByTwoPerturbation:1:c}
%
%} % answer

\paragraph{Q: two state Hamiltonian.} 

Given a two-state system

\begin{dmath}\label{eqn:simplestTwoByTwoPerturbation:20}
H = H_0 + \lambda V
=
\begin{bmatrix}
E_1 & \lambda \Delta \\
\lambda \Delta & E_2
\end{bmatrix}
\end{dmath}

\begin{enumerate}[a]
\item Solve the system exactly.
\item Find the first order perturbed states and second order energy shifts, and compare to the exact solution.
\item Solve the degenerate case for \( E_1 = E_2 \), and compare to the exact solution.
\end{enumerate}

\paragraph{A: part (a)}

The energy eigenvalues \( \epsilon \) are given by

\begin{dmath}\label{eqn:simplestTwoByTwoPerturbation:40}
0
=
\lr{ E_1 - \epsilon }
\lr{ E_2 - \epsilon }
- (\lambda \Delta)^2,
\end{dmath}

or

\begin{dmath}\label{eqn:simplestTwoByTwoPerturbation:60}
\epsilon^2 - \epsilon\lr{ E_1 + E_2 } + E_1 E_2 = (\lambda \Delta)^2.
\end{dmath}

After rearranging this is
\begin{dmath}\label{eqn:simplestTwoByTwoPerturbation:80}
\epsilon = \frac{ E_1 + E_2 }{2} \pm \sqrt{ \lr{ \frac{ E_1 - E_2 }{2} }^2 + (\lambda \Delta)^2 }.
\end{dmath}

Notice that for \( E_2 = E_1 \) we have

\begin{dmath}\label{eqn:simplestTwoByTwoPerturbation:100}
\epsilon = E_1 \pm \lambda \Delta.
\end{dmath}

Since a change of basis can always put the problem in a form so that \( E_1 > E_2 \), let's assume that to make an approximation of the energy eigenvalues for \( \Abs{\lambda \Delta} \ll \ifrac{ (E_1 - E_2) }{2} \)

\begin{dmath}\label{eqn:simplestTwoByTwoPerturbation:120}
\epsilon 
=
\frac{ E_1 + E_2 }{2} \pm \frac{ E_1 - E_2 }{2} \sqrt{ 1 + \frac{(2 \lambda \Delta)^2}{(E_1 - E_2)^2} }
\approx 
\frac{ E_1 + E_2 }{2} \pm \frac{ E_1 - E_2 }{2} \lr{ 1 + 2 \frac{(\lambda \Delta)^2}{(E_1 - E_2)^2} }
=
\frac{ E_1 + E_2 }{2} \pm \frac{ E_1 - E_2 }{2} 
\pm
\frac{(\lambda \Delta)^2}{E_1 - E_2}
=
E_1 + \frac{(\lambda \Delta)^2}{E_1 - E_2}, E_2 + \frac{(\lambda \Delta)^2}{E_2 - E_1}.
\end{dmath}

For the perturbed states, starting with the plus case, if 

\begin{dmath}\label{eqn:simplestTwoByTwoPerturbation:140}
\ket{+} \propto 
\begin{bmatrix}
a \\
b
\end{bmatrix},
\end{dmath}

we must have
\begin{dmath}\label{eqn:simplestTwoByTwoPerturbation:160}
0 
=
\biglr{ E_1 - \lr{ E_1 + \frac{(\lambda \Delta)^2}{E_1 - E_2} } } a + \lambda \Delta b
=
\biglr{ - \frac{(\lambda \Delta)^2}{E_1 - E_2} } a + \lambda \Delta b,
\end{dmath}

so

\begin{dmath}\label{eqn:simplestTwoByTwoPerturbation:180}
\ket{+} \rightarrow 
\begin{bmatrix}
1 \\
\frac{\lambda \Delta}{E_1 - E_2}
\end{bmatrix}
= \ket{+} + \frac{\lambda \Delta}{E_1 - E_2} \ket{-}.
\end{dmath}

Similarily for the minus case we must have

\begin{dmath}\label{eqn:simplestTwoByTwoPerturbation:200}
0 
=
\lambda \Delta a + \biglr{ E_2 - \lr{ E_2 + \frac{(\lambda \Delta)^2}{E_2 - E_1} } } b 
=
\lambda \Delta b + \biglr{ - \frac{(\lambda \Delta)^2}{E_2 - E_1} } b,
\end{dmath}

for
\begin{dmath}\label{eqn:simplestTwoByTwoPerturbation:220}
\ket{-} \rightarrow 
\ket{-} + \frac{\lambda \Delta}{E_2 - E_1} \ket{+}.
\end{dmath}

\paragraph{A: part (b)}

For the pertubation the first energy shift for pertubation of the \( \ket{+} \) state is

\begin{dmath}\label{eqn:simplestTwoByTwoPerturbation:240}
E_{+}^{(1)} 
= \ket{+} V \ket{+}
= 
\lambda \Delta 
\begin{bmatrix}
1 & 0
\end{bmatrix}
\begin{bmatrix}
0 & 1 \\
1 & 0
\end{bmatrix}
\begin{bmatrix}
1 \\
0
\end{bmatrix}
=\lambda \Delta
\begin{bmatrix}
1 & 0
\end{bmatrix}
\begin{bmatrix}
0 \\
1 
\end{bmatrix}
=
0.
\end{dmath}

The first order energy shift for the pertubation of the \( \ket{-} \) state is also zero.  The perturbed \( \ket{+} \) state is

\begin{dmath}\label{eqn:simplestTwoByTwoPerturbation:260}
\ket{+}^{(1)} 
= \frac{\overbar{P}_{+}}{E_1 - H_0} V \ket{+}
= \frac{\ket{-}\bra{-}}{E_1 - E_2} V \ket{+}
\end{dmath}

The numerator matrix element is

\begin{dmath}\label{eqn:simplestTwoByTwoPerturbation:280}
\bra{-} V \ket{+}
=
\begin{bmatrix}
0 & 1
\end{bmatrix}
\begin{bmatrix}
0 & \Delta \\
\Delta & 0
\end{bmatrix}
\begin{bmatrix}
1 \\
0
\end{bmatrix}
=
\begin{bmatrix}
0 & 1
\end{bmatrix}
\begin{bmatrix}
0 \\
\Delta
\end{bmatrix}
=
\Delta,
\end{dmath}

so

\begin{dmath}\label{eqn:simplestTwoByTwoPerturbation:300}
\ket{+} \rightarrow \ket{+} + \ket{-} \frac{\Delta}{E_1 - E_2}.
\end{dmath}

Observe that this matches the first order series expansion of the exact value above.

For the perturbation of \( \ket{-} \) we need the matrix element

\begin{dmath}\label{eqn:simplestTwoByTwoPerturbation:320}
\bra{+} V \ket{-}
=
\begin{bmatrix}
1 & 0
\end{bmatrix}
\begin{bmatrix}
0 & \Delta \\
\Delta & 0
\end{bmatrix}
\begin{bmatrix}
0 \\
1
\end{bmatrix}
=
\begin{bmatrix}
1 & 0
\end{bmatrix}
\begin{bmatrix}
\Delta
0 \\
\end{bmatrix}
=
\Delta,
\end{dmath}

so it's clear that the perturbed ket is

\begin{dmath}\label{eqn:simplestTwoByTwoPerturbation:340}
\ket{-} \rightarrow \ket{-} + \ket{+} \frac{\Delta}{E_2 - E_1},
\end{dmath}

also matching the approximation found from the exact computation.  The second order energy shifts can now be calculated

\begin{dmath}\label{eqn:simplestTwoByTwoPerturbation:360}
\bra{+} V \ket{+}'
=
\begin{bmatrix}
1 & 0
\end{bmatrix}
\begin{bmatrix}
0 & \Delta \\
\Delta & 0
\end{bmatrix}
\begin{bmatrix}
1 \\
\frac{\Delta}{E_1 - E_2}
\end{bmatrix}
=
\begin{bmatrix}
1 & 0
\end{bmatrix}
\begin{bmatrix}
\frac{\Delta^2}{E_1 - E_2} \\
\Delta
\end{bmatrix}
=
\frac{\Delta^2}{E_1 - E_2},
\end{dmath}

and

\begin{dmath}\label{eqn:simplestTwoByTwoPerturbation:380}
\bra{-} V \ket{-}'
=
\begin{bmatrix}
0 & 1
\end{bmatrix}
\begin{bmatrix}
0 & \Delta \\
\Delta & 0
\end{bmatrix}
\begin{bmatrix}
\frac{\Delta}{E_2 - E_1}
1 \\
\end{bmatrix}
=
\begin{bmatrix}
0 & 1
\end{bmatrix}
\begin{bmatrix}
\Delta \\
\frac{\Delta^2}{E_2 - E_1} \\
\end{bmatrix}
=
\frac{\Delta^2}{E_2 - E_1},
\end{dmath}

The energy perturbations are therefore
\begin{dmath}\label{eqn:simplestTwoByTwoPerturbation:400}
\begin{aligned}
E_1 &\rightarrow E_1 + \frac{(\lambda \Delta)^2}{E_1 - E_2} \\
E_2 &\rightarrow E_2 + \frac{(\lambda \Delta)^2}{E_2 - E_1}.
\end{aligned}
\end{dmath}

This is what we had by approximating the exact case.

\paragraph{A: part (c)}

\EndArticle
