\input{../peeter_prologue_print.tex}
%\input{../peeter_prologue_widescreen.tex}

\chapter{24.77 notes.}
%\label{chap:template}
%\useCCL
%\blogpage{http://sites.google.com/site/peeterjoot/math2011/template.pdf}
%\date{Sept 1, 2011}
%\revisionInfo{template.tex}

\beginArtWithToc
%\beginArtNoToc

%\section{Motivation.}
%
%\section{Guts}

We start with

\begin{align*}
\expectation{\frac{e^2}{\Abs{\Br_1 - \Br_2}}}
&=
\left( \frac{Z^3}{\pi a_0^3}\right)^2 e^2
\int d^3 k d^3 r_1 d^3 r_2 \inv{2 \pi^2 k^2} e^{i \Bk \cdot (\Br_1 - \Br_2) } e^{ -2 Z (r_1 + r_2)/a_0} \\
&= 
\left( \frac{Z^3}{\pi a_0^3}\right)^2 e^2
\inv{2 \pi^2} 
\int d^3 k \inv{k^2}
d^3 r_1 
e^{i \Bk \cdot \Br_1 } e^{ -2 Z r_1 /a_0} 
\int 
d^3 r_2 
e^{-i \Bk \cdot \Br_2 } e^{ -2 Z r_2/a_0} \\
\end{align*}

To evaluate the two last integrals, I figure the author has aligned the axis for the $d^3 r_1$ volume elements to make the integrals easier.  Specifically, for the first so that $\Bk \cdot \Br_1 = k r_1 \cos\theta$, so the integral takes the form

\begin{align*}
\int 
d^3 r_1 
e^{i \Bk \cdot \Br_1 } e^{ -2 Z r_1 /a_0} 
&=
-\int 
r_1^2 d r_1 d\phi d(\cos\theta)
e^{i k r_1 \cos\theta } e^{ -2 Z r_1 /a_0} \\
&=
- 2 \pi \int_{r=0}^\infty \int_{u=1}^{-1}
r^2 dr du
e^{i k r u } e^{ -2 Z r /a_0} \\
&=
- 2 \pi \int_{r=0}^\infty 
r^2 dr 
\inv{i k r} \left( e^{-i k r } - e^{i k r} \right) e^{ -2 Z r /a_0} \\
&=
\frac{4 \pi}{k } \int_{r=0}^\infty 
r dr 
\inv{2i} \left( e^{i k r } - e^{-i k r} \right) e^{ -2 Z r /a_0} \\
&=
\frac{4 \pi}{k } \int_{r=0}^\infty r dr \sin(k r) e^{ -2 Z r /a_0} \\
\end{align*}

For this last, mathematica gives me (24.75) from the text

\begin{equation}\label{eqn:qmTwoL6:n}
\int 
d^3 r_1 
e^{i \Bk \cdot \Br_1 } e^{ -2 Z r_1 /a_0} 
=
\frac{ 16 \pi Z a_0^3 }{(k^2 a_0^2 + 4 Z^2)^2}
\end{equation}

For the second integral, if we align the axis so that $-\Bk \cdot \Br_2 = k r \cos\theta$ and repeat, then we have

\begin{align*}
\expectation{\frac{e^2}{\Abs{\Br_1 - \Br_2}}}
&=
\left( \frac{Z^3}{\pi a_0^3}\right)^2 e^2
\inv{2 \pi^2} 
16^2 \pi^2 Z^2 a_0^6 
\int d^3 k \inv{k^2}
\frac{ 1 }{(k^2 a_0^2 + 4 Z^2)^4} \\
&=
\frac{128 Z^8}{\pi^2 } e^2
\int dk d\Omega 
\frac{ 1 }{(k^2 a_0^2 + 4 Z^2)^4} \\
&=
\frac{512 Z^8}{\pi} e^2
\int dk 
\frac{ 1 }{(k^2 a_0^2 + 4 Z^2)^4} \\
&=
\frac{512 Z^8}{\pi} e^2
\int dk 
\frac{ 1 }{(k^2 a_0^2 + 4 Z^2)^4} \\
\end{align*}

With $k a_0 = 2 Z \kappa$ this is

\begin{align*}
\expectation{\frac{e^2}{\Abs{\Br_1 - \Br_2}}}
&=
\frac{512 Z^8}{\pi} e^2
\int d\kappa 
\frac{ 2 Z }{a_0}
\frac{ 1 }{(2 Z)^8 (\kappa^2 + 1)^4} \\
&=
\frac{4 Z}{\pi a_0} e^2
\int d\kappa 
\frac{ 1 }{(\kappa^2 + 1)^4} \\
\end{align*}

Here I note that 

\begin{align*}
\frac{d}{d\kappa}
\frac{-1}{ 3 (1+x)^3 }
=
\inv{ (1+x)^4 }
\end{align*}

so the definite integral has the value
\begin{align*}
\int_0^\infty d\kappa 
\frac{ 1 }{ (\kappa^2 + 1)^4} 
=
\frac{-1}{ 3 (1+\infty)^3 }
-
\frac{-1}{ 3 (1+0)^3 }
= \inv{3}
\end{align*}

(not $5 \pi/3$ as claimed in the text).  This gives us

\begin{align*}
\expectation{\frac{e^2}{\Abs{\Br_1 - \Br_2}}}
&=
\frac{4 Z e^2} { \pi a_0 } 
\int d\kappa 
\frac{ 1 }{(\kappa^2 + 1)^4} \\
&=
\frac{4 Z e^2} { 3 \pi a_0 }  \\
&\approx 0.424 \frac{Z e^2 }{a_0} \ne \frac{5}{8} \frac{Z e^2 }{a_0}
\end{align*}

%\EndArticle
\EndNoBibArticle
