\documentclass{article}      % Specifies the document class

\input{../peeters_macros.tex}
\newcommand{\gpgrade}[2] {{\left\langle{{#1}}\right\rangle}_{#2}}

%
% The real thing:
%

                             % The preamble begins here.
\title{ Notes on shear transformation. } % Declares the document's title.
\author{Peeter Joot}         % Declares the author's name.
%\date{}        % Deleting this command produces today's date.

\begin{document}             % End of preamble and beginning of text.

\maketitle{}

\section{}

GASC and GAFP both give examples of shear transformations of the following
form:

\[
F(a) = a + \alpha(a \cdot f) e.
\]

Geometric Algebra for Physicists uses this to compute the determinant without putting the operator in matrix form.  They end up stating that 

\begin{equation}\label{eqn:shearblade}
F(A) = A + \alpha e \wedge (f \cdot A).
\end{equation}

holds for any grade blade $A$.  For grade 1 that is true since

\begin{align*}
(a \cdot f) e 
&= \gpgrade{(a \cdot f) e \rangle}{1} \\
&= (a \cdot f) \wedge e.
\end{align*}

They demonstrate equation \ref{eqn:shearblade}
holds for the grade 2 case.  To me it seems
like an induction is required to make their statement for any grade.

Question: Is there some other principle that I didn't notice in my reading that allows assertion of 
equation \ref{eqn:shearblade}
for any grade blade without the induction.

\subsection{ Proof for any grade blade. }

For $A \in {\bigwedge}^r$

\begin{align*}
F(A) \wedge F(b)
&= \left(A + \alpha e \wedge (f \cdot A)\right) \wedge
   \left(b + \alpha(b \cdot f) e \right) \\
&= A \wedge b
 + \alpha 
\left(
e \wedge (f \cdot A) \wedge b
+ (b \cdot f) A \wedge e 
\right) \\
&= A \wedge b
 + \alpha e \wedge
\underbrace{
\left(
(f \cdot A) \wedge b
+ (-1)^r (b \cdot f) A 
\right)
}_{(*)} \\
&= A \wedge b + \alpha e \wedge (f \cdot (A \wedge b))
\end{align*}

QED.

Verification below of $(*) = f \cdot (A \wedge b)$ is required to complete the proof (can probably find that in one of the books or papers but it is derivable
easily enough).

Do I have a sign mixup here somewhere?  Now that I look again I see that GAFP
has the result in different order $(A \cdot f) \wedge e$, and I get negation
reconciling the two.

\subsection{ Dot product reduction of blade by one. }

\begin{align*}
f \cdot (A \wedge b)
&= \inv{2} \gpgrade{f (A \wedge b)}{r} \\
&= \inv{2} \gpgrade{f (A b + (-1)^r b A)}{r} \\
&= \inv{2} \gpgrade{(f A) b + (-1)^r f b A}{r} \\
&= \inv{2} \gpgrade{((-1)^r A f + 2 f \cdot A) b + (-1)^r f b A}{r} \\
&= (f \cdot A) \wedge b + \frac{(-1)^r}{2} \gpgrade{A f b + f b A}{r} \\
&= (f \cdot A) \wedge b + (-1)^r (f \cdot b) A
+ \frac{(-1)^r}{2} \gpgrade{A f \wedge b + f \wedge b A}{r} \\
\end{align*}

This last term, the symmetric product of a bivector with a blade is zero.
The grades $r-2, r+4, \ldots$ terms are symmetric, and the other grades
$r, r+4, \ldots$ are antisymmetric.

Thus we have

\begin{equation}
f \cdot (A \wedge b)
= (f \cdot A) \wedge b - (-1)^r (f \cdot b) A
\end{equation}

This generalizes the familiar vector reduction formula to higher grades.
Observe that for the vector case we need the most general definition
of the wedge product for the scalar-vector wedge product (grade $1-0$ part of the product).

\end{document}               % End of document.
