%
% Copyright © 2012 Peeter Joot.  All Rights Reserved.
% Licenced as described in the file LICENSE under the root directory of this GIT repository.
%
\makeproblem{Convolution theorem}{pr:convolution:1}{

Find the form of the Fourier transform

\begin{dmath}\label{eqn:convolution:10}
\tilde{f}(\omega) = \int f(y) e^{-i \omega y} dy
\end{dmath}

of a convolution integral

\begin{dmath}\label{eqn:convolution:30}
f(y) = \int dy' g(y') h(y - y') = g(y) \conj h(y).
\end{dmath}

} % makeproblem

\makeanswer{pr:convolution:1}{ 

This is basically just an application of change of variables

\begin{dmath}\label{eqn:convolution:50}
\FF f(y) 
= 
\int dy e^{-i \omega y}
dy' g(y') h(y - y')
= 
\int dy' g(y') 
\int dy e^{-i \omega y} \mathWithDescription{h(y - y')}{
$y - y' = u$
}{1}
= 
\int dy' g(y') 
\int du e^{-i \omega (u + y')} h(u)
= 
\tilde{h}(\omega)
\int dy' g(y') e^{-i \omega y'} 
= 
\tilde{h}(\omega)
\tilde{g}(\omega)
\end{dmath}

} % makeanswer
