%
% Copyright © 2012 Peeter Joot.  All Rights Reserved.
% Licenced as described in the file LICENSE under the root directory of this GIT repository.
%
%\input{../blogpost.tex}
%\renewcommand{\basename}{modernOpticsLecture15}
%\renewcommand{\dirname}{notes/phy485/}
%\newcommand{\keywords}{Optics, PHY485H1F}
%\input{../peeter_prologue_print2.tex}
%
%\usepackage[draft]{fixme}
%\fxusetheme{color}
%
%\beginArtNoToc
%\generatetitle{PHY485H1F Modern Optics.  Lecture 15: Multiple interference (cont.).  Taught by Prof.\ Joseph Thywissen}
%%\chapter{Multiple interference (cont.)}
%\label{chap:modernOpticsLecture15}
%
%\section{Disclaimer}
%
%Peeter's lecture notes from class.  May not be entirely coherent.

\fxwarning{review lecture 15}{work through this lecture in detail.}

We are going to look at the far field of a diffraction grating with $N$ illuminated slits \cref{fig:modernOpticsLecture15:modernOpticsLecture15Fig1}.  Let's review this, writing out the Fraunhofer approximation for an image plane set at the back plane of a lens at the aperture as in \cref{fig:modernOpticsLecture15:modernOpticsLecture15Fig6}.

\imageFigure{figures/modernOpticsLecture15Fig1}{Diffraction grating interferometry}{fig:modernOpticsLecture15:modernOpticsLecture15Fig1}{0.3}
\imageFigure{figures/modernOpticsLecture15Fig6}{Fraunhofer diffraction}{fig:modernOpticsLecture15:modernOpticsLecture15Fig6}{0.3}

Our transfer matrix is

\begin{dmath}\label{eqn:modernOpticsLecture15:620}
M_{x,y} = 
\begin{bmatrix}
1 & f \\
0 & 1
\end{bmatrix}
\begin{bmatrix}
1 & 0 \\
-1/f & 1
\end{bmatrix}
=
\begin{bmatrix}
0 & f \\
-1/f & 1
\end{bmatrix}
\end{dmath}

so that if $\alpha, \beta$ are the output angles at the lens, our image positions are $f \alpha, f \beta$ respectively.  Our geometry is

\begin{dmath}\label{eqn:modernOpticsLecture15:640}
\BR + \Br' = \Br = f(\alpha, \beta, 1),
\end{dmath}

for which our path length from $\Br'$ is

\begin{dmath}\label{eqn:modernOpticsLecture15:660}
\Abs{\BR} 
= r \left( 1 + \frac{{r'}^2}{r^2} - 2 \frac{\Br \cdot \Br'}{r^2} \right)^{1/2}
\sim r + \frac{{r'}^2}{2 r^2} - \rcap \cdot \Br',
\end{dmath}

and to first order

\begin{dmath}\label{eqn:modernOpticsLecture15:680}
k\Abs{\BR} 
\sim k f - k \rcap \cdot \Br'
= k f - k (x', y') \cdot (\alpha, \beta)
= k f - k x' \alpha - k y' \beta
= k f - \Bk \cdot \Br'.
\end{dmath}

Our diffraction integral therefore takes the form

\begin{dmath}\label{eqn:modernOpticsLecture15:700}
\Psi(\Br) \sim \frac{e^{i k f}}{f} \int e^{-i \Bk \cdot \Br' } d^2 \Br'.
\end{dmath}

Dealing with only one direction ($y$), and writing $\Bk = (k_x, k_y) = (2 \pi/\lambda) (\cos\theta, \sin\theta)$, and dropping the propagation term we have

\begin{dmath}\label{eqn:modernOpticsLecture15:720}
\Psi(\Br) \sim \int e^{-i k_y y' } dy',
\end{dmath}

which is the Fourier transform of the aperture, say $g(y)$ evaluated at $k_y = (2 \pi/\lambda) \sin\theta$.

We will use the convolution theorem \ref{pr:convolution:1}, constructing the complete aperture as a convolution, with transmission \cref{fig:modernOpticsLecture15:modernOpticsLecture15Fig2}.

\imageFigure{figures/modernOpticsLecture15Fig2}{Convolution of box with comb}{fig:modernOpticsLecture15:modernOpticsLecture15Fig2}{0.2}

\begin{dmath}\label{eqn:modernOpticsLecture15:20}
f(y) = \int dy' g(y') h(y - y') = g(y) \conj h(y)
\end{dmath}

Consider the convolution with the delta function comb

\begin{dmath}\label{eqn:modernOpticsLecture15:40}
h(y) = \sum_{n=0}^{N-1} \delta (y - n a)
\end{dmath}

So that the convolution is

\begin{dmath}\label{eqn:modernOpticsLecture15:60}
f(y) 
= \int dy' g(y') \sum_{n = 0}^{N-1} \delta(y - y' - n a)
= 
\sum_{n = 0}^{N-1} 
\int dy' g(y') 
\delta(y - y' - n a)
= 
\sum_{n = 0}^{N-1} 
g(y - n a) 
\end{dmath}

Convolution theorem

\begin{dmath}\label{eqn:modernOpticsLecture15:80}
F( k_y ) = H( k_y ) G( k_y ).
\end{dmath}

As mentioned, here we write

\begin{dmath}\label{eqn:modernOpticsLecture15:100}
k_y = \frac{2 \pi}{\lambda} \sin\theta.
\end{dmath}

(to distinguish from our normal writing of $k = 2 \pi /\lambda$)

For a single slit, in the Fraunhofer limit, we compute

\begin{dmath}\label{eqn:modernOpticsLecture15:120}
G(k_y) 
= 
\int_{-b/2}^{b/2} e^{-i k_y y} dy
= \evalrange{\frac{e^{-i k_y y}}{-i k_y}}{-b/2}{b/2}
= \frac{
e^{i k_y b/2}
-e^{-i k_y b/2}
}
{
2 (i k_y) /2 
}
= 
\frac{\sin(b k_y/2)}{b k_y/2}
\end{dmath}

as illustrated in \cref{fig:lecture15figuresSincCrossings:lecture15figuresSincCrossingsFig7}.
% hand drawn:
%\cref{fig:modernOpticsLecture15:modernOpticsLecture15Fig3}.
%\imageFigure{figures/modernOpticsLecture15Fig3}{Zero of diffraction intensity}{fig:modernOpticsLecture15:modernOpticsLecture15Fig3}{0.2}
% mathematica:
\imageFigure{figures/lecture15figuresSincCrossingsFig7}{Zero of diffraction wavefunction}{fig:lecture15figuresSincCrossings:lecture15figuresSincCrossingsFig7}{0.3}

For the Fourier transform of the delta comb, we have

\begin{dmath}\label{eqn:modernOpticsLecture15:140}
H(k_y) 
= 
\int_{-\infty}^\infty 
e^{i k_y y} 
\sum_{n = 0}^{N-1} 
\delta(y - n a)
=
\sum_{n = 0}^{N-1} 
\int_{-\infty}^\infty 
e^{i k_y y} 
\delta(y - n a)
=
\sum_{n = 0}^{N-1} 
e^{i k_y n a} 
=
\sum_{n = 0}^{N-1} 
\left( e^{i k_y a}  \right)^n
\end{dmath}

Recall that we can sum a finite geometric series, by taking the difference of

\begin{subequations}
\begin{dmath}\label{eqn:modernOpticsLecture15:160}
a S_N = a + a^2 + \cdots a^{N}
\end{dmath}
\begin{dmath}\label{eqn:modernOpticsLecture15:180}
S_N = 1 + a + \cdots a^{N-1}
\end{dmath}
\end{subequations}

so that 

\begin{dmath}\label{eqn:modernOpticsLecture15:200}
(a - 1)S_N = a^N - 1
\end{dmath}

or
\begin{dmath}\label{eqn:modernOpticsLecture15:220}
S_N = \frac{a^N - 1}{a-1},
\end{dmath}

and we have for our Fourier transform we have

\begin{dmath}\label{eqn:modernOpticsLecture15:240}
H(k_y) 
= 
\frac{1 - e^{i k_y a N }}{1 - e^{i k_y a}}
=
\frac{e^{i k_y a N/2}}{e^{i k_y a/2}}
\frac{e^{-i k_y a N/2} - e^{i k_y a N/2 }}{e^{-i k_y a/2} - e^{i k_y a/2}}
=
e^{i \gamma (N-1)}
\frac{\sin (N\gamma)}{ \sin \gamma}
\end{dmath}

where
\begin{equation}\label{eqn:modernOpticsLecture15:260}
\gamma = \inv{2} k_y a = \inv{2} k a \sin\theta.
\end{equation}

We want

\begin{dmath}\label{eqn:modernOpticsLecture15:280}
I 
= \Abs{F(k_y)}^2
= 
\Abs{H(k_y)}^2
\Abs{G(k_y)}^2
= I_0 \left( \frac{\sin\beta}{\beta} \right)^2 \left( 
\frac
{\sin N\gamma}
{\sin \gamma}
\right)^2
\end{dmath}

where 

\begin{subequations}
\begin{equation}\label{eqn:modernOpticsLecture15:300}
\beta = \inv{2} b k_y = \inv{2} b k \sin\theta
\end{equation}
\begin{equation}\label{eqn:modernOpticsLecture15:320}
\gamma = \inv{2} k_y a = \inv{2} k a \sin\theta.
\end{equation}
\end{subequations}

\paragraph{Check: $N = 2$}

\begin{dmath}\label{eqn:modernOpticsLecture15:340}
\left( \frac{\sin 2 \gamma}{2 \sin\gamma} \right)^2 = 
\left( \frac{2 \sin \gamma \cos\gamma}{2 \sin\gamma} \right)^2 = \cos^2\gamma
\end{dmath}

(Good).

To get a bit of a feeling for what this looks like we can check out a plot, as in \cref{fig:lecture15figures5aperaturesIntensityPlot:lecture15figures5aperaturesIntensityPlotFig8}, plotting $n = 5, a = 0.869, b = 0.172, \lambda = 1$ (generated from \nbref{lecture15figures.nb}.)

\imageFigure{figures/lecture15figures5aperaturesIntensityPlotFig8}{A sample intensity pattern for a multiple aperature diffraction grating}{fig:lecture15figures5aperaturesIntensityPlot:lecture15figures5aperaturesIntensityPlotFig8}{0.3}

Our far field view was \cref{fig:modernOpticsLecture15:modernOpticsLecture15Fig4}.

\imageFigure{figures/modernOpticsLecture15Fig4}{Far field view}{fig:modernOpticsLecture15:modernOpticsLecture15Fig4}{0.2}

How well can we resolve frequency?

We will write out $\gamma$ in terms of angular frequency

\begin{dmath}\label{eqn:modernOpticsLecture15:360}
\gamma 
= \inv{2} a \frac{\omega}{c} \sin\theta
= \pi \frac{\omega}{\omega_0} \sin\theta
\end{dmath}

where

\begin{dmath}\label{eqn:modernOpticsLecture15:380}
\omega_0 = \frac{2 \pi c}{a}
\end{dmath}

(where $a$ is the period of the diffraction grating).

The peak is at $\gamma = m \pi$, or

\begin{dmath}\label{eqn:modernOpticsLecture15:400}
\gamma_{\mathrm{peak}} 
= m \pi
= \pi \frac{\omega}{\omega_0} \sin\theta,
\end{dmath}

or
\begin{dmath}\label{eqn:modernOpticsLecture15:420}
m = \frac{\omega}{\omega_0} \sin\theta,
\end{dmath}

Zeros are at $N \gamma = l \pi$ (provided $l \ne N m$)

\fxwarning{verify zeros location claim}{verify this zeros result}

Closest zero

\begin{dmath}\label{eqn:modernOpticsLecture15:440}
l = N m + 1
\end{dmath}

\begin{dmath}\label{eqn:modernOpticsLecture15:460}
\Delta \gamma 
= \gamma_{\mathrm{zero}} - \gamma_{\mathrm{peak}} 
= \frac{l}{N} \pi - m \pi
= \frac{N m + 1}{N} \pi - m \pi
\end{dmath}

or

\begin{dmath}\label{eqn:modernOpticsLecture15:480}
\Delta \gamma 
= \frac{\pi}{N} 
= \frac{\pi \sin\theta}{\omega_0} \Delta \omega
\end{dmath}

\paragraph{Rework after question:}

Peaks for $\omega_{1,2}$ are

\begin{dmath}\label{eqn:modernOpticsLecture15:500}
\gamma_{\mathrm{peak}, 1} = \pi \frac{\omega_1}{\omega_0} \sin\theta = m \pi
\end{dmath}
\begin{dmath}\label{eqn:modernOpticsLecture15:520}
\gamma_{\mathrm{peak}, 2} = \pi \frac{\omega_2}{\omega_0} \sin\theta = m \pi
\end{dmath}

so that
\begin{dmath}\label{eqn:modernOpticsLecture15:540}
\Delta \gamma 
= 
\Delta \omega
\frac{\pi}{\omega_0} \sin\theta.
\end{dmath}

The peak is resolved when

\begin{dmath}\label{eqn:modernOpticsLecture15:560}
\Delta \gamma = \frac{m \pi}{\omega_1} \Delta \omega = \frac{\pi}{N},
\end{dmath}

as shown in \cref{fig:modernOpticsLecture15:modernOpticsLecture15Fig5}.

\imageFigure{figures/modernOpticsLecture15Fig5}{Resolution}{fig:modernOpticsLecture15:modernOpticsLecture15Fig5}{0.2}

That is

\begin{dmath}\label{eqn:modernOpticsLecture15:580}
\boxed{
\frac{\Delta \omega}{\overbar{\omega}} = \inv{N m}
}
\end{dmath}

Observe that this looks 

\begin{dmath}\label{eqn:modernOpticsLecture15:600}
\frac{\Delta \omega}{\omega} = \inv{m \FF},
\end{dmath}

because $\FF \sim \text{number of bounces in the Etalon}$.

But $m \approx 1,2,3$, not $m \gg 1$.

%\EndNoBibArticle
