\documentclass{article}

\input{../peeters_macros.tex}
\input{../peeters_macros2.tex}

\DeclareMathOperator{\sgn}{sgn}
\newcommand{\expectation}[1]{\langle{#1}\rangle}

%\usepackage{listings}
%\usepackage{txfonts} % for ointctr... (also appears to make "prettier" \int and \sum's)
\usepackage[bookmarks=true]{hyperref}

\usepackage{color,cite,graphicx}
   % use colour in the document, put your citations as [1-4]
   % rather than [1,2,3,4] (it looks nicer, and the extended LaTeX2e
   % graphics package. 
\usepackage{latexsym,amssymb,epsf} % don't remember if these are
   % needed, but their inclusion can't do any damage


\title{ Bohm Chapter 10 problems. }
\author{Peeter Joot \quad peeter.joot@gmail.com }
\date{ April 2d, 2009.  Last Revision: $Date: 2009/04/24 18:27:05 $ }

\begin{document}

\maketitle{}
\tableofcontents
\section{ Bohm Chapter 10 problems. }

Problems and additional details from reading of \cite{bohm1989qt}, chapter 10.

Differing from the text, the notation $\expectation{O}$ has been used instead $\bar{O}$ mostly due to not knowing how to format the a wide overbar, and getting peculilar looking results.

\subsection{ P1. Uncertainty calculations. }

Calculate $\Delta x \Delta p$ for a few wave functions

\subsubsection{ Gaussian wave function. }

\begin{align*}
\psi = \alpha_1 e^{-\alpha x^2/2}
\end{align*}

Normalization

\begin{align*}
1 
&= \alpha_1^2 \int e^{-\alpha x^2} dx \\
&= \alpha_1^2 \sqrt{\pi/\alpha}
\end{align*}

\begin{align*}
\expectation{x} \propto \int x e^{-\alpha x^2} dx = 0
\end{align*}

(odd)

\begin{align*}
\expectation{x^2} 
&= \alpha_1^2 \int x^2 e^{-\alpha x^2} dx \\
&= \alpha_1^2 \int x (e^{-\alpha x^2}/-2\alpha)' dx \\
&= \alpha_1^2 \int (e^{-\alpha x^2}/2\alpha) dx \\
&= \alpha_1^2 \inv{2\alpha} \sqrt{\pi/\alpha}
\end{align*}

\begin{align*}
\expectation{p} 
&= -i \hbar \alpha_1^2 \int e^{-\alpha x^2 /2} d/dx e^{-\alpha x^2 /2} dx
&= -i \hbar \alpha_1^2 \int e^{-\alpha x^2 /2} (-\alpha x) e^{-\alpha x^2 /2} dx
&= 0
\end{align*}

(odd).

\begin{align*}
\expectation{p^2} 
&= - \hbar^2 \alpha_1^2 \int e^{-\alpha x^2 /2} d/dx ((-\alpha x) e^{-\alpha x^2 /2}) dx \\
&= \hbar^2 \alpha_1^2 \alpha \int e^{-\alpha x^2 /2} d/dx (x e^{-\alpha x^2 /2}) dx \\
&= \hbar^2 \alpha_1^2 \alpha \int e^{-\alpha x^2 } ( 1 - \alpha x) dx \\
&= \hbar^2 \alpha_1^2 \alpha \sqrt{\pi/\alpha}
\end{align*}

Assembling results

\begin{align*}
\frac{(\Delta x \Delta p)^2}{\hbar^2} 
&= \alpha_1^4 \alpha {\pi/\alpha} \inv{2\alpha} \\
&= \alpha_1^4 {\pi/\alpha} \inv{2} \\
&= (1)^2 \inv{2} \\
&= \inv{2} \\
\end{align*}
%1 &= \alpha_1^2 \sqrt{\pi/\alpha}

For
\begin{align*}
\Delta x \Delta p \approx 0.7 \hbar > \hbar/2
\end{align*}

\subsubsection{ Absolute valued exponential wave function. }

\begin{align*}
\psi &= \alpha_2 e^{-\alpha\Abs{x}}
\end{align*}

Normalization

\begin{align*}
1 
&= 2 \alpha_2^2 \int_0^\infty e^{-2 \alpha{x}} dx \\
&= 2 \alpha_2^2 \left. \frac{e^{-2 \alpha{x}}}{-2\alpha} \right\vert_0^\infty \\
&= 2 \alpha_2^2 \inv{2\alpha}
\end{align*}

\begin{align*}
\expectation{x} = 0
\end{align*}

(odd).

\begin{align*}
\expectation{x^2} 
&= 2 \alpha_2^2 \int_0^\infty x^2 e^{-2\alpha x} dx \\
&= \alpha_2^2 \inv{2 \alpha^3}
\end{align*}

For the momentum we need derivatives

\begin{align*}
\frac{d}{dx} e^{-\alpha \Abs{x}} 
&=
\left\{
\begin{array}{l l}
d/dx(e^{-\alpha x} & \quad \mbox{$x>0$} \\
d/dx(e^{\alpha x} & \quad \mbox{$x<0$} \\
\end{array}
\right. \\
&=
\left\{
\begin{array}{l l}
-\alpha (e^{-\alpha x} & \quad \mbox{$x>0$} \\
\alpha (e^{\alpha x} & \quad \mbox{$x<0$} \\
\end{array}
\right. \\
&=
-\alpha \sgn(x) e^{-\alpha \Abs{x}}
\end{align*}

\begin{align*}
\expectation{p} 
&= i \hbar \alpha_2^2 \alpha \int \sgn(x) e^{-2\alpha\Abs{x}} dx  \\
&= 0
\end{align*}

(odd)

\begin{align*}
\expectation{p^2} 
&= (-i \hbar)^2 \alpha_2^2 \alpha^2 \int (\sgn(x))^2 e^{-2\alpha\Abs{x}} dx  \\
&= - 2(\hbar)^2 \alpha_2^2 \alpha^2 \int_0^\infty e^{-2\alpha\Abs{x}} dx  \\
&= 2(\hbar)^2 \alpha_2^2 \alpha^2 \inv{2\alpha} \\
&= (\hbar)^2 \alpha_2^2 \alpha \\
\end{align*}

Putting results together we have

\begin{align*}
\expectation{p^2} \expectation{x^2} 
&= (\hbar)^2 \alpha_2^4 \inv{2 \alpha^2} \\
&= (\hbar)^2/2
\end{align*}

Same as in the Gaussian.

\subsubsection{ Squared polynomial. }

\begin{align*}
\psi = \frac{\alpha_3}{(\alpha^2 + x^2)^2}
\end{align*}

For this one, the integrals were evaluated with Mathematica online integrator, where the contributions at $\infty$ were scaled $\arctan(x/\alpha)$ values.

\begin{align*}
1 
&= \alpha_3^2 \int \frac{dx}{(\alpha^2 + x^2)^4} \\
&= \alpha_3^2 \frac{15 \pi}{48 \alpha^7}
\end{align*}

\begin{align*}
\expectation{x} &= 0
\end{align*}

\begin{align*}
\expectation{x^2} 
&= \alpha_3^2 \int \frac{x^2 dx}{(\alpha^2 + x^2)^4} \\
&= \alpha_3^2 \frac{3 \pi}{48 \alpha^5}
\end{align*}

\begin{align*}
\expectation{p} 
&= -i \hbar \alpha_3^2 \int \frac{dx}{(\alpha^2 + x^2)^2} \frac{d}{dx} \frac{1}{(\alpha^2 + x^2)^2}  \\
&= -i \hbar \alpha_3^2 \int \frac{dx}{(\alpha^2 + x^2)^2} \frac{-4x}{(\alpha^2 + x^2)^2} \\
&= 0
\end{align*}

\begin{align*}
\expectation{p^2} 
&= (-i \hbar)^2 \alpha_3^2 \int \frac{dx}{(\alpha^2 + x^2)^2} \frac{d^2}{dx^2} \frac{1}{(\alpha^2 + x^2)^2}  \\
&= 4 \hbar^2 \alpha_3^2 \int \frac{dx}{(\alpha^2 + x^2)^2} \frac{d}{dx} \frac{x}{(\alpha^2 + x^2)^3} \\
&= 4 \hbar^2 \alpha_3^2 \int dx
\left( \frac{1}{(\alpha^2 + x^2)^5} \frac{x(-3)(2x)}{(\alpha^2 + x^2)^6} \right)
\\
&= 4 \hbar^2 \alpha_3^2 \int dx \frac{\alpha^2 - 5x^2}{(\alpha^2 + x^2)^6} 
\\
&= 4 \hbar^2 \alpha_3^2 \frac{105 \pi}{960 \alpha^9}
\\
\end{align*}

Assembling

\begin{align*}
\expectation{p^2} \expectation{x^2} 
&= 4 \hbar^2 \alpha_3^4 \frac{105 \pi}{960 \alpha^9} \frac{3 \pi}{48 \alpha^5} \\
&= \hbar^2 \frac{7}{25}
\end{align*}

For
\begin{align*}
\Delta{p} \Delta{x} 
&= \hbar \frac{\sqrt{7}}{5} \\
&\approx 0.52 \hbar  \\
&> \hbar/2
\end{align*}

\subsection{ P2. Correlation coefficients. }

It is noted that a classical correlation coefficient for random variables $x$, and $p$ has the form

\begin{align*}
C_{n,m}
&= \expectation{x^n p^m} - \expectation{x^n}\expectation{p^m}
\end{align*}

However, for operator expectation values and average of both orderings is more reasonable

\begin{align*}
C_{n,m}
&= \inv{2} \left( 
\expectation{x^n p^m} - \expectation{x^n}\expectation{p^m} 
+ \expectation{p^m x^n} - \expectation{p^m}\expectation{x^n} 
\right) \\
&= \inv{2} \left( \expectation{x^n p^m} + \expectation{p^m x^n} \right) - \expectation{x^n}\expectation{p^m} 
\end{align*}

With the operator substitution $p \rightarrow -i \hbar d/dx$ this provides equation (7) in the text.

\subsubsection{ first correlations. }

Calculate $C_{1,1}$, and $C_{2,2}$ for 

\begin{align*}
\psi = \alpha e^{-\alpha x^2/2}
\end{align*}

First the normalization and first and second order expectations.

\begin{align*}
1 
&= \alpha^2 \int e^{-\alpha x^2} dx \\
&= \alpha^2 \sqrt{\pi/\alpha} \\
\implies \\
\alpha &= \pi^{1/3}
\end{align*}

\begin{align*}
\expectation{x} &= 0
\end{align*}

\begin{align*}
\expectation{p} &= 0
\end{align*}

And in particular

\begin{align*}
\expectation{p} \expectation{x} &= 0 \\
\end{align*}

\subsubsection{ second correlations. }

\begin{align*}
\expectation{x^2} 
&= \alpha^2 \int x^2 e^{-\alpha x^2} dx \\
&= \alpha^2 \int x x e^{-\alpha x^2} dx \\
&= \alpha^2 \int x (e^{-\alpha x^2}/-\alpha)' dx \\
&= \alpha^2 \int e^{-\alpha x^2}/\alpha dx \\
&= \alpha \int e^{-\alpha x^2} dx \\
&= \alpha \sqrt{\pi/\alpha} \\
&= \sqrt{\alpha \pi} \\
&= \pi^{2/3} \\
\end{align*}

\begin{align*}
\expectation{p^2} 
&= -\alpha^2 \hbar^2 \int e^{-\alpha x^2/2} \frac{d^2}{dx^2} e^{-\alpha x^2/2} dx \\
&= \alpha^2 \hbar^2 \int \frac{d}{dx} e^{-\alpha x^2/2} \frac{d}{dx} e^{-\alpha x^2/2} dx \\
&= \alpha^2 \hbar^2 \int (-\alpha x)^2 e^{-\alpha x^2} dx \\
&= \alpha^4 \hbar^2 \int x^2 e^{-\alpha x^2} dx \\
&= \alpha^4 \hbar^2 \int x x e^{-\alpha x^2} dx \\
&= \alpha^4 \hbar^2 \int x (e^{-\alpha x^2}/-\alpha)' dx \\
&= \alpha^3 \hbar^2 \int e^{-\alpha x^2} dx \\
&= \alpha^3 \hbar^2 \inv{2\alpha} \\
&= \alpha^2 \hbar^2  \\
&= \pi^{2/3} \hbar^2 
\end{align*}

\begin{align*}
\expectation{p^2} \expectation{x^2} &= \hbar^2 \pi^{4/3}
\end{align*}

For the first terms we want

\begin{align*}
\inv{2} \left( \expectation{x^2 p^2} + \expectation{p^2 x^2} \right)
&=
\frac{-\hbar^2 \alpha^2}{2} \int \left( 
e^{-\alpha x^2/2} x^2 \frac{d^2}{dx^2} (e^{-\alpha x^2/2} )
+ e^{-\alpha x^2/2} \frac{d^2}{dx^2} ( x^2 e^{-\alpha x^2/2} ) \right) dx \\
&=
\frac{-\hbar^2 \alpha^2}{2} \int \left( 
 \frac{d^2}{dx^2} ( e^{-\alpha x^2/2} x^2 ) e^{-\alpha x^2/2} 
+ e^{-\alpha x^2/2} \frac{d^2}{dx^2} ( x^2 e^{-\alpha x^2/2} ) \right) dx \\
&=
{-\hbar^2 \alpha^2} \int e^{-\alpha x^2/2} \frac{d^2}{dx^2} ( e^{-\alpha x^2/2} x^2 ) dx \\
&=
{\hbar^2 \alpha^2} \int \left( \frac{d}{dx} e^{-\alpha x^2/2} \right) \left( \frac{d}{dx} ( e^{-\alpha x^2/2} x^2 ) \right) dx \\
&=
{\hbar^2 \alpha^2} \int (-\alpha x) e^{-\alpha x^2} (2x + x^2(-\alpha x)) dx \\
&=
{\hbar^2 \alpha^3} \int x^2 e^{-\alpha x^2} (-2 + x^2 \alpha ) dx \\
&=
{-\hbar^2 \alpha^2} \sqrt{\pi/\alpha}  \\
&=
-\hbar^2 \pi
\end{align*}

This leaves 

\begin{align*}
C_{2,2} &=
-\hbar^2 \left( \pi + \pi^{2/3} \right)
\end{align*}

\subsection{ P3. First correlations zero for real wave function. }

Show that the first correlation coefficient is zero for any real wave function.

\begin{align*}
C_{1,1} &= \inv{2}\left( \expectation{x p} + \expectation{p x} \right) - \expectation{x}\expectation{p}
\end{align*}

Calculate instead the equivalent problem

\begin{align*}
2 C_{1,1}/(-i\hbar) &= \left( \expectation{x d/dx} + \expectation{d/dx x} \right) - 2 \expectation{x}\expectation{d/dx}
\end{align*}

For the anti-commutator part we have

\begin{align*}
\expectation{x d/dx} + \expectation{d/dx x} 
&=
\int \psi x \psi' + \psi (x \psi)' \\
&=
\int \psi x \psi' - \psi' x \psi \\
&= 0
\end{align*}

and for the remainder if one is zero then the sum is.  In particular

\begin{align*}
\expectation{d/dx} 
&= \int_{-\infty}^\infty dx \psi \psi' \\
&= \inv{2} \int_{-\infty}^\infty dx (\psi^2)' \\
&= \inv{2} \left. \psi^2 \right\vert_{-\infty}^\infty
\end{align*}

Provided the wave function vanishes in the square at $\pm \infty$, then we are done.

\subsection{ P4. }
\subsection{ P5. }
\subsection{ P6. }

The phase space text on this page is not clear to me.  Revisit after study
of phase space, Poisson brackets, and Liouville's theorem in a classical
context.

\subsection{ P7. wave function for the position and momentum operators for the equality uncertaintly case. }

Note that in the definitions of $\alpha$ and $\beta$ right before equation (25) in the text, the symbols are reversed.  For consistency with condition (1)
this should be

\begin{align*}
\beta &= (x - \bar{x}) \\
\alpha &= (p - \bar{p})
\end{align*}

Where condition (1) for equality in the Schwartz inequality for this 
generalized uncertainty principle is

\begin{align*}
\alpha \psi &= C \beta \psi
\end{align*}

Putting the two together for this problem one has

\begin{align*}
(p - \bar{p}) \psi &= C (x - \bar{x}) \psi \\
\implies \\
p \psi &= \bar{p} \psi + C (x - \bar{x}) \psi \\
\end{align*}

or
\begin{align*}
\frac{\hbar}{i} \frac{d\psi}{dx} &= \bar{p} \psi + C (x - \bar{x}) \psi \\
\end{align*}

Integrating, as was done in the $\bar{x} = \bar{p} = 0$ case in the text, 
one has

\begin{align*}
\ln \psi &= \frac{i}{\hbar}( \bar{p} x + C (x - \bar{x})^2/2 ) + \ln D \\
\end{align*}

or
\begin{align*}
\psi &= D e^{i\bar{p} x/\hbar} e^{ i C (x - \bar{x})^2/2\hbar } \\
\end{align*}

Note that this shows there is a typo in equation (26) in the text too ($i\bar{p} x$ needs the $1/\hbar$ factor).  References to $C$ in the text preceding this should be $C/\hbar$ in a few cases too.

It was shown above that real wave functions have the vanishing $C_{1,1}$ coefficient required for uncorrelated operators, and if that's the case $i C/\hbar$, must be a real negative constant.  Denoting that as $-a$ as in the text one has

\begin{align*}
\psi \propto e^{i\bar{p} x/\hbar} e^{ -a(x - \bar{x})^2/2} \\
\end{align*}

\subsection{ P8. Calculate uncertainty for the initially Gaussian wave function. }

Wave function for the problem is

\begin{align*}
\psi &= \alpha \exp\left( -(A - iB) \frac{x^2}{2} \right) \\
A &= \frac{(\Delta k)^2}{ 1 + \frac{\hbar^2 t^2}{m^2}(\Delta k)^4 } \\
B &= (\Delta k)^4 \frac{\hbar t}{m} \frac{1}{ 1 + \frac{\hbar^2 t^2}{m^2}(\Delta k)^4 } \\
\end{align*}

The normalization is

\begin{align*}
1 
&= \Abs{\alpha}^2 \int \exp\left( -A {x^2} \right) \\
&= \Abs{\alpha}^2 \sqrt{\frac{\pi}{A}}
\end{align*}

First moment
\begin{align*}
\expectation{x} = 0
\end{align*}

Second moment
\begin{align*}
\expectation{x^2} 
&= 
\Abs{\alpha}^2 \int x^2 \exp\left( -A x^2 \right) \\
&= 
\Abs{\alpha}^2 \int x (\exp\left( -A x^2 \right)/(-A))' \\
&= 
\Abs{\alpha}^2 \int \exp\left( -A x^2 \right)/A \\
&= 
\Abs{\alpha}^2 \inv{A} \sqrt{ \frac{\pi}{A}} \\
&= 
\inv{A} \\
&=
\frac{ 1 + \frac{\hbar^2 t^2}{m^2}(\Delta k)^4 }{(\Delta k)^2}
 \\
&=
\inv{(\Delta k)^2} + \frac{\hbar^2 t^2}{m^2}(\Delta k)^2 \\
\end{align*}

\bibliographystyle{plainnat}
\bibliography{myrefs}

\end{document}
