%\input{../peeter_prologue_print.tex}
%\input{../peeter_prologue_widescreen.tex}

\chapter{More problems from Liboff chapter 4}
\label{chap:liboff43}
%\useCCL
\blogpage{http://sites.google.com/site/peeterjoot/math2010/liboff43.pdf}
\date{June 25, 2010}
\revisionInfo{liboff43.tex}

%\beginArtWithToc
\beginArtNoToc

\section{Motivation.}

Some more problems from \citep{liboff2003iqm}.

\section{Problem 4.11}

Some problems on Hermitian adjoints.  The starting point is the definition of the adjoint $A^\dagger$ of $A$ in terms of the inner product

\begin{align*}
\braket{\hatA^\dagger \phi}{\psi} = \braket{\phi}{\hatA \psi}
\end{align*}

\subsection{4.11 a}

\begin{align*}
\braket{ \phi }{ (a \hatA + b \hatB) \psi } 
&=
a \braket{ \phi }{ \hatA \psi } + b \braket{ \phi }{ \hatB \psi }  \\
&=
a \braket{ \hatA^\dagger \phi }{ \psi } + b \braket{ \hatB^\dagger \phi }{ \psi }  \\
&=
\braket{ a^\conj \hatA^\dagger \phi }{ \psi } + \braket{ b^\conj \hatB^\dagger \phi }{ \psi }  \\
&=
\braket{ (a^\conj \hatA^\dagger + b^\conj \hatB^\dagger ) \phi }{ \psi }  \\
&\implies \\
(a \hatA + b \hatB)^\dagger = (a^\conj \hatA^\dagger + b^\conj \hatB^\dagger)
\end{align*}

\subsection{4.11 b}
\begin{align*}
\braket{ \phi }{ \hatA \hatB \psi } 
&=
\braket{ \hatA^\dagger \phi }{ \hatB \psi }  \\
&=
\braket{ \hatB^\dagger \hatA^\dagger \phi }{ \psi }  \\
&\implies \\
(\hatA \hatB )^\dagger &=
\hatB^\dagger \hatA^\dagger 
\end{align*}

%\subsection{4.11 c}
\subsection{4.11 d}

Hermitian adjoint of $D^2$, where $D = \PDi{x}{}$.  Here we need the integral form of the inner product

\begin{align*}
\braket{\phi}{D^2 \psi} 
&=
\int \phi^\conj \PD{x}{}\PD{x}{\psi} \\
&=
-\int \PD{x}{\phi^\conj} \PD{x}{\psi} \\
&=
\int \psi \PD{x}{}\PD{x}{\phi^\conj} \\
&\implies \\
(D^2)^\dagger &= D^2
\end{align*}

Since the text shows that the square of a Hermitian operator is Hermitian, one perhaps wonders if $D$ is (but we expect not since $\hatp = -i \hbar D$ is Hermitian).

Suppose $\hatA = aD$, we have 

\begin{align*}
\hatA^\dagger = -a^\conj D,
\end{align*}

so for this to be Hermitian ($\hatA = \hatA^\dagger$) we must have $- a^\conj = a$.  If $a = r e^{i\theta}$, we have

\begin{align*}
-1 = e^{2 i\theta}
\end{align*}

So $\theta = \pi (1/2 + n)$, and $a = \pm i r$.  This fixes the scalar multiples of $D$ that are required to form a Hermitian operator

\begin{align*}
\hatA &= \pm i r D
\end{align*}

where $r$ is any real positive constant.

\subsection{4.11 e}

\begin{align*}
(\hatA \hatB - \hatB \hatA)^\dagger &= - (\hatA^\dagger \hatB^\dagger - \hatB^\dagger \hatA^\dagger)
\end{align*}

\subsection{4.11 f}

\begin{align*}
(\hatA \hatB + \hatB \hatA)^\dagger &= \hatA^\dagger \hatB^\dagger + \hatB^\dagger \hatA^\dagger
\end{align*}

\subsection{4.11 g}

\begin{align*}
i (\hatA \hatB - \hatB \hatA)^\dagger &= i ( \hatA^\dagger \hatB^\dagger - \hatB^\dagger \hatA^\dagger)
\end{align*}

\subsection{4.11 h}

This one was to calculate $(\hatA^\dagger)^\dagger$.  Intuitively I'd expect that $(\hatA^\dagger)^\dagger = \hatA$.  How could one show this?

Trying to show this with Dirac notation, I got all mixed up initially.

Using the more straightforward and old fashioned integral notation (as in \citep{bohm1989qt}), this is more straightforward.  We have the Hermitian conjugate defined by

\begin{align*}
\int \psi_2^\conj (\hatA \psi_1) = \int (\hatA^\dagger \psi_2^\conj) \psi_1,
\end{align*}

Or, more symmetrically, using braces to indicate operator direction

\begin{align*}
\int \psi_2^\conj (\hatA \psi_1) = \int (\psi_2^\conj \hatA^\dagger) \psi_1.
\end{align*}

Introduce a couple of variable substitutions for clarity

\begin{align*}
\phi_1 &= \psi_1^\conj \\
\phi_2 &= \psi_2^\conj \\
\hatB &= \hatA^\dagger.
\end{align*}

We then have

\begin{align*}
\int \psi_2^\conj (\hatA \psi_1)
&=
\int (\psi_2^\conj \hatA^\dagger) \psi_1 \\
&=
\int (\phi_2 \hatB) \phi_1^\conj \\
&=
\int \phi_1^\conj (\hatB \phi_2) \\
&=
\int (\phi_1^\conj \hatB^\dagger) \phi_2 \\
&=
\int \phi_2 (\hatB^\dagger \phi_1^\conj) \\
&=
\int \psi_2^\conj (\hatA^{\dagger \dagger} \psi_1) \\
\end{align*}

Since this is true for all $\psi_k$, we have $\hatA = \hatA^{\dagger \dagger}$ as expected.

Having figured out the problem in the simpleton way, it's now simple to go back and translate this into the Dirac inner product notation without getting muddled.  We have

\begin{align*}
\braket{ \psi_2 }{ \hatA \psi_1 } 
&=
\braket{ \hatA^\dagger \psi_2 }{ \psi_1 }  \\
&=
\braket{ \hatB \phi_2^\conj }{ \phi_1^\conj }  \\
&=
{\braket{ \phi_1 }{ \hatB^\conj \phi_2}}^\conj  \\
&=
{\braket{ (\hatB^\conj)^\dagger \phi_1 }{ \phi_2}}^\conj  \\
&=
\braket{\phi_2^\conj }{ \hatB^\dagger \phi_1^\conj } \\
&=
\braket{\psi_2 }{ \hatA^{\dagger \dagger} \psi_1 } \\
\end{align*}

\subsection{4.11 i}

\begin{align*}
(\hatA \hatA^\dagger)^\dagger &= (\hatA^\dagger)^\dagger \hatA^\dagger 
\end{align*}

since $(\hatA^\dagger) ^\dagger = \hatA$

\begin{align*}
(\hatA \hatA^\dagger)^\dagger &= \hatA \hatA^\dagger.
\end{align*}

\section{Problem 4.12 d}

If $\hatA$ is not Hermitian, is the product $\hatA^\dagger \hatA$ Hermitian?  To start we need to verify that $\braket{\psi}{\hatA^\dagger \phi} = \braket{\hatA \psi}{\phi}$.

\begin{align*}
\braket{ \psi }{ \hatA^\dagger \phi } 
&=
{\braket{ (\hatA^\dagger)^\conj \phi^\conj }{ \psi^\conj }}^\conj \\
&=
{\braket{ \phi^\conj }{ \hatA^\conj \psi^\conj }}^\conj \\
&=
\braket{ \psi }{ \hatA \psi }.
\end{align*}

With that verified we have

\begin{align*}
\braket{ \psi }{ \hatA^\dagger \hatA \phi } 
&=
\braket{ \hatA \psi }{ \hatA \phi }  \\
&=
\braket{ \hatA^\dagger \hatA \psi }{ \phi },
\end{align*}

so, the answer is yes.  Provided the adjoint exists, that product will be Hermitian.

\section{Problem 4.14}

Show that $\Expectation{\hatA} = \Expectation{\hatA}^\conj$ (that it is real), if $\hatA$ is Hermitian.  This follows by expansion of that conjugate

\begin{align*}
\Expectation{\hatA}^\conj 
&= \left(\int \psi^\conj \hatA \psi \right)^\conj \\
&= \int \psi \hatA^\conj \psi^\conj \\
&= \int (\hatA \psi)^\conj \psi \\
&= \braket{ \hatA \psi }{ \psi } \\
&= \braket{ \psi }{ \hatA^\dagger \psi } \\
&= \braket{ \psi }{ \hatA \psi } \\
&= \Expectation{\hatA}
\end{align*}

\EndArticle
