\documentclass{article}

\input{../peeters_macros.tex}
\input{../peeters_macros2.tex}

%\usepackage{listings}
\usepackage{txfonts} % for ointctr... (also appears to make "prettier" \int and \sum's)
\usepackage[bookmarks=true]{hyperref}

\usepackage{color,cite,graphicx}
   % use colour in the document, put your citations as [1-4]
   % rather than [1,2,3,4] (it looks nicer, and the extended LaTeX2e
   % graphics package. 
\usepackage{latexsym,amssymb,epsf} % don't remember if these are
   % needed, but their inclusion can't do any damage


\title{ Four vector velocity addition notes. }
\author{Peeter Joot \quad peeter.joot@gmail.com }
\date{ April 8, 2009.  Last Revision: $Date: 2009/04/10 02:42:18 $ }

\begin{document}

\maketitle{}
\tableofcontents
\section{ Motivation. }

Reconcile four vector transformed velocity coordinates with non-covariant form.
Specifically, equations (10) and (191) in \cite{pauli1981tr} look considerably
different on the surface, but must have the same content.

Equations (10) were also derived in a bit more detail than in Pauli's book in
\cite{PJpauliVelocityAddition} and are

\begin{align}\label{eqn:eqn10}
u_x &= \frac{ {u_x}' + v  }{ 1 + v {u_x}'} \\
u_y &= \frac{{u_y}'}{\gamma (1 + v {u_x}'/c^2)} \\
u_z &= \frac{{u_z}'}{\gamma (1 + v {u_x}'/c^2)} \\
\gamma^{-1} &= \sqrt{ 1 - v^2/c^2}
\end{align}

whereas equations (191) are given as

\begin{align}\label{eqn:eqn191}
{u^1}' &= \gamma ( u^1 + i (v/c) u^4) \\
{u^2}' &= {u^2} \\
{u^3}' &= {u^3} \\
{u^4}' &= \gamma ( u^4 - i (v/c) u^1)
\end{align}

\section{ Derive the transformed velocity equations. }

Pauli uses a $(+,+,+,-)$ metric, with $ct = x^4 = - x_4$.  For much of his SR treatment he also uses the Minkowski representation $x^4 = x_4 = ict$. In the first representation we have

\begin{align*}
-c^2 
&= \frac{dx^\mu}{d\tau} \frac{dx_\mu}{d\tau} \\
&= \frac{dx^k}{d\tau} \frac{dx_k}{d\tau} + \frac{dx^4}{d\tau} \frac{dx_4}{d\tau} \\
&= \left(\frac{dt}{d\tau}\right)^2 \left( \sum_{k=1}^3 \left(\frac{dx^k}{dt}\right)^2 - \left(\frac{dx^4}{dt}\right)^2 \right) \\
&= \left(\frac{dt}{d\tau}\right)^2 \left( \Bu^2 - c^2 \right) \\
\end{align*}

Shuffling and taking roots produces a $\gamma$ factor by virtue of the invariant

\begin{align*}
%\gamma 
%&= 
\frac{dt}{d\tau} \\
&= \inv{\sqrt{ 1 - \Bu^2/c^2 }}
\end{align*}

This is enough to write the proper velocity in terms of a space time split 

\begin{align*}
\dot{X} 
&= \left(\frac{dx^\mu}{d\tau}\right) \\
&= \inv{\sqrt{ 1 - \Bu^2/c^2 }} (\Bu, c)
\end{align*}

As a four vector this can be Lorentz boosted.  For an 
x-axis boost we have

\begin{align*}
{\begin{bmatrix}
u^1 \\
u^2 \\
u^3 \\
u^4 \\
\end{bmatrix}}'
&=
\begin{bmatrix}
\gamma & 0 & 0 & - \gamma \beta \\
0 & 1 & 0 & 0 \\
0 & 0 & 1 & 0 \\
- \gamma \beta & 0 & 0 & \gamma \\
\end{bmatrix}
{\begin{bmatrix}
u^1 \\
u^2 \\
u^3 \\
u^4 \\
\end{bmatrix}} 
\\
\gamma &= \inv{\sqrt{ 1 - \beta^2 }} \\
\end{align*}

Expanding this we have

\begin{align}\label{eqn:realRepresentationFourVector}
{u^1}' &= \gamma ( u^1 - \beta u^4) \\
{u^2}' &= {u^2} \\
{u^3}' &= {u^3} \\
{u^4}' &= \gamma ( u^4 - \beta u^1)
\end{align}

In the imaginary representation the Lorentz transform takes the form

\begin{align*}
{\begin{bmatrix}
u^1 \\
u^2 \\
u^3 \\
u^4 \\
\end{bmatrix}}'
&=
\begin{bmatrix}
\gamma & 0 & 0 & i \gamma \beta \\
0 & 1 & 0 & 0 \\
0 & 0 & 1 & 0 \\
- i \gamma \beta & 0 & 0 & \gamma \\
\end{bmatrix}
{\begin{bmatrix}
u^1 \\
u^2 \\
u^3 \\
u^4 \\
\end{bmatrix}} 
\end{align*}

Let's verify that this produces the same result by expansion

\begin{align*}
{u^1}' &= \gamma ( u^1 + i \beta u^4) \\
{u^2}' &= {u^2} \\
{u^3}' &= {u^3} \\
{u^4}' &= \gamma ( u^4 - \beta i u^1)
\end{align*}

with $u^4 \rightarrow i u^4$ to switch to a real representation this is

\begin{align*}
{u^1}' &= \gamma ( u^1 - \beta u^4) \\
{u^2}' &= {u^2} \\
{u^3}' &= {u^3} \\
{u^4}' &= \gamma ( u^4 - \beta u^1)
\end{align*}

Good.  This matches equations \ref{eqn:realRepresentationFourVector}.  Now, we want to put these in an explicit space time representation
to compare against \ref{eqn:eqn10}.  Since those are in real form, work with the real representation instead of the imaginary Minkowski
representation for such a comparision.

\subsection{ Non-covariant representation of the transformed velocity. }

Expanding out the proper time derivatives (assuming that $dx'/dt' = v$ is a correct interpretation of the math), we have

\begin{align*}
\inv{\sqrt{1 - v^2/c^2}} \frac{{dx'}^1}{dt'} &= \inv{\sqrt{1 - v^2/c^2}} \inv{\sqrt{1 - \Bu^2/c^2}} \left( \frac{dx^1}{dt} - \beta c \right) \\
\inv{\sqrt{1 - v^2/c^2}} \frac{{dx'}^2}{dt'} &= \inv{\sqrt{1 - \Bu^2/c^2}} \frac{dx^2}{dt} \\
\inv{\sqrt{1 - v^2/c^2}} \frac{{dx'}^3}{dt'} &= \inv{\sqrt{1 - \Bu^2/c^2}} \frac{dx^3}{dt} \\
\inv{\sqrt{1 - v^2/c^2}} \frac{{dx'}^4}{dt'} &= \inv{\sqrt{1 - v^2/c^2}} \inv{\sqrt{1 - \Bu^2/c^2}} \left( c - \beta \frac{dx^1}{dt} \right)
\end{align*}

Hmm.  That doesn't appear to match.

\section{ Try again from scratch. }

\subsection{ Boost a stationary particle. }

Instead of starting with a proper velocity with a spatial component, let's cut the complexity and consider the simplest case, a particle at rest.  The worldline (in two dimensions) for a particle in its rest frame is

\begin{align*}
X = (0, ct) 
\end{align*}

The proper velocity for this particle is 

\begin{align*}
u = \frac{dX}{d\tau} = \left(0, c\frac{dt}{d\tau} \right) 
\end{align*}

But since this is a particle in its rest frame $dt/d\tau = 1$, this proper velocity is

\begin{align*}
u = \left(0, c \right) 
\end{align*}

Observe that the norm of this vector (still using the time negative metric signature) is

\begin{align*}
u \cdot u = 0^2 - c^2 = -c^2
\end{align*}

Now, what happens when we apply a Lorentz boost to this?

\begin{align*}
u' &= 
\begin{bmatrix}
\gamma & - \gamma \beta \\
- \gamma \beta & \gamma \\
\end{bmatrix}
\begin{bmatrix}
0 \\
c
\end{bmatrix} \\
\end{align*}

This is
\begin{align}\label{eqn:uPrime}
u' &= 
\gamma
\begin{bmatrix}
- \beta \\
1 \\
\end{bmatrix}
c
\end{align}

What's the norm of this vector.  It should be unchanged, so let's verify.

\begin{align*}
u' \cdot u' 
&= \gamma^2 \left( (- \beta)^2 - 1^2 \right) c^2 \\
&= - \gamma^2 \left( 1 - \beta^2 \right) c^2 \\
&= - c^2 \\
\end{align*}

Good, still have the expected $-c^2$ value.  For this boosted vector, what is $dt'/d\tau'$?

Note that in general for the components of $u'$ we have

\begin{align*}
\frac{{dx'}^\mu}{d\tau'}
&=
\frac{{dx'}^\mu}{dt'} \frac{{dt'}}{d\tau'}
\end{align*}

and in particular we have ${u'}^4 = c dt'/d\tau$ %, since the proper time $\tau'$ in the primed frame measures the time for the particle at rest
%in that frame.  This gives

\begin{align*}
{u'}^4
&=
\frac{{dx'}^4}{dt'} \frac{{dt'}}{d\tau'} \\
&= c \frac{{dt'}}{d\tau'} \\
\end{align*}

Comparing to \ref{eqn:uPrime} we have

\begin{align*}
{u'}^4 
&= \gamma c \\
&= c \frac{{dt'}}{d\tau'} \\
\end{align*}

and therefore can write

\begin{align*}
\frac{{dt'}}{d\tau'} 
&= \gamma 
\end{align*}

Similarily the spatial velocity of the particle in the boosted frame is

\begin{align*}
{u'}^1
&=
\frac{{dx'}^1}{dt'} \frac{{dt'}}{d\tau'} \\
&= u_x' \frac{{dt'}}{d\tau'} \\
&= - \gamma v
\end{align*}

So we have 

\begin{align*}
u_x' = -v 
\end{align*}

This seems to make sense.  We move the frame along the positive x-axis, so a particle at rest at the origin of the stationary frame has a velocity $v$ in the opposite direction from the viewpoint of something at rest in the moving frame.

\subsection{ Apply a second boost transformation. }

Okay, treating the almost too simple case in detail was helpful to see where to go next.  Now that we have a view of a particle at rest
from a moving frame, let's apply another boost so we have a second frame moving with relative velocity $\beta'$ with respect to the moving
frame.  Our transformation is

\begin{align*}
L' =
\begin{bmatrix}
\gamma' & - \gamma' \beta' \\
- \gamma' \beta' & \gamma' \\
\end{bmatrix}
\end{align*}

this second transformation takes the original proper velocity to
\begin{align*}
u'' &=
\gamma \gamma'
\begin{bmatrix}
1 & - \beta' \\
- \beta' & 1 \\
\end{bmatrix}
\begin{bmatrix}
- \beta \\
1 \\
\end{bmatrix}
c \\
&=
\gamma \gamma'
\begin{bmatrix}
-(\beta + \beta') \\
1 + \beta\beta'
\end{bmatrix}
c \\
\end{align*}

Let's verify that we still have our invarient norm.

\begin{align*}
u'' \cdot u'' 
&=
\gamma^2 {\gamma'}^2
\left(
(\beta + \beta')^2 
-(1 + \beta\beta')^2
\right)
c^2 \\
&=
\gamma^2 {\gamma'}^2
\left(
\beta^2
+{\beta'}^2
+2 \beta\beta'
-1
-2 \beta\beta'
-\beta^2 {\beta'}^2
\right)
c^2 \\
&=
\gamma^2 {\gamma'}^2
\left(
\beta^2 (1 - {\beta'}^2)
-(1 -{\beta'}^2)
\right)
c^2 \\
&=
-\gamma^2 {\gamma'}^2 (1 -{\beta'}^2)(1 -\beta^2) c^2 \\
&=
- c^2 \\
\end{align*}

\bibliographystyle{plainnat}
\bibliography{myrefs}

\end{document}
