%\documentclass{article}

%\input{../peeters_macros.tex}

%\usepackage[bookmarks=true]{hyperref}

\chapter{Taylor's theorem deviation.}
%\author{Peeter Joot \quad peeter.joot@gmail.com}
%\date{ Feb. 2, 2008. Last Revision: $Date: 2009/06/03 22:13:06 $ } % Deleting this command produces today's date.

%\begin{document}

%\maketitle{}

\cite{hestenes1999nfc} presents a very simple derivation of Taylor's Theorem,
but I feel a
slightly different (dumber, but longer) presentation would be more effective.

In the same fashion, form the integral

\[
I = \int_{t}^{t+s} F'(u) du
\]

Now, observe that the this first order derivative can be written in
terms of it's second order derivative

\[
(u F'(u))' = F'(u) + u F''(u)
\]

So we could write

\begin{align*}
I &= \int_{t}^{t+s} ((u F'(u))' - u F''(u)) du \\
  &= {u F'(u)} \vert_{u=t}^{t+s} - \int_{t}^{t+s} u F''(u)) du \\
  &= (t+s) F'(t+s) - t F'(t) - \int_{t}^{t+s} u F''(u)) du \\
\end{align*}

This is true, but not the Taylor expansion we are used to.  Adjusting things slightly leaves a zero term at $u=t+s$, as follows:

\[
\left((t + s - u) F'(u)\right)' = -F'(u) + (t+s-u) F''(u)
\]

\begin{align*}
I &= F(t+s) - F(t) \\
 &= \int_{t}^{t+s} ( - ((t + s - u) F'(u))' + (t+s-u) F''(u) ) du \\
 &= - {(t + s - u) F'(u)} \vert_{u=t}^{t+s} + \int_{t}^{t+s} (t+s-u) F''(u) du \\
 &= s F'(t) + \int_{t}^{t+s} (t+s-u) F''(u) du \\
\end{align*}

This results in the first two order terms of the Tailor series, with an explicit remainder term

\[
F(t+s) = F(t) + s F'(t) + \int_{t}^{t+s} (t+s-u) F''(u) du
\]

This process can be continued for as many terms as desired.  Doing the calculation for the second order term yields

\[
\left(\frac{(t + s - u)^2}{2} F''(u)\right)' = -( t + s - u ) F''(u) + \frac{(t+s-u)}{2} F'''(u)
\]

And substituting that into the first order expansion above we have

\[
F(t+s) = F(t) + s F'(t) + \frac{s^2}{2} F''(t) + \int_{t}^{t+s} \frac{1}{2}(t+s-u)^2 F'''(u) du
\]

Induction produces n terms of Taylor's series with an explicit remainder

\[
F(t+s) = \sum_{k=0}^{n} \frac{s^k}{k!} \frac{d^k}{dt^k} F(t) +
                        \int_{t}^{t+s} \frac{1}{n!}(t+s-u)^n \frac{d^{n+1}}{dt^{n+1}} F(u) du
\]

To truly prove the infinite series result one would have to show that the remainder term tends to zero.

%\bibliographystyle{plainnat} % supposed to allow for \url use.
%\bibliography{myrefs}      % expects file "myrefs.bib"

%\end{document}               % End of document.
