\documentclass{article}

\input{../peeters_macros.tex}
\input{../peeters_macros2.tex}

\usepackage[bookmarks=true]{hyperref}

\usepackage{color,cite,graphicx}
   % use colour in the document, put your citations as [1-4]
   % rather than [1,2,3,4] (it looks nicer, and the extended LaTeX2e
   % graphics package. 
\usepackage{latexsym,amssymb,epsf} % don't remember if these are
   % needed, but their inclusion can't do any damage


\title{ Some notes on Pauli Relativity Velocity addition. }
\author{Peeter Joot}
\date{ Dec 25, 2008.  Last Revision: $Date: 2008/12/26 04:22:41 $ }

\begin{document}
\maketitle{}
%
%\tableofcontents

\section{ Motivation. }

Fill out some details from part 1.6, velocity additon of \cite{pauli1981tr}.

\section{ }

Given a path $x^i(t')$ i n the moving (primed) frame $S'$, the aim is to 
express the observed velocities for this path from the rest frame $S$.

From the Lorentz transformation of the coordinates we have for a point in the moving frame

\begin{align*}
x' &= \gamma ( x - vt) \\
t' &= \gamma ( t - vx)
\end{align*}

Or reversed (inverting velocities)

\begin{align*}
x &= \gamma ( x' + vt') \\
t &= \gamma ( t' + vx')
\end{align*}

taking differentials we have

\begin{align*}
dx &= \gamma ( dx' + v dt') \\
dy &= dy' \\
dz &= dz' \\
dt &= \gamma ( dt' + v dx')
\end{align*}

Dividing by $dt'$, this is

\begin{align*}
\frac{dx}{dt} &= \frac{ dx' + v dt' }{ dt' + v dx'} \\
\frac{dy}{dt} &= \frac{dy'}{\gamma (dt' + v dx')} \\
\frac{dz}{dt} &= \frac{dz'}{\gamma (dt' + v dx')} \\
\end{align*}

FIXME: don't like this dividing by differentials.  Try to reexpress this 
using the chain rule.

Or in terms of velocity coordinates we have Pauli's equation 10.

\begin{align*}
u_x &= \frac{ {u_x}' + v  }{ 1 + v {u_x}'} \\
u_y &= \frac{{u_y}'}{\gamma (1 + v {u_x}')} \\
u_z &= \frac{{u_z}'}{\gamma (1 + v {u_x}')} \\
\end{align*}

Next he writes $u^2 = \sum_i {u_i}^2$, in terms of the primed velocities

\begin{align*}
{u_x}^2 +{u_y}^2 +{u_z}^2 
&=
\inv{( 1 + v {u_x}' )^2 } \left(
( {u_x}' + v  )^2
+(1-v^2){{u_y}'}^2
+(1-v^2){{u_z}'}^2
\right) \\
&=
\inv{( 1 + v {u_x}' )^2 } \left(
{{u_x}'}^2
+ 2 {u_x}' v
+ v^2
+(1-v^2){{u_y}'}^2
+(1-v^2){{u_z}'}^2
+v^2 {{u_x}'}^2
-v^2 {{u_x}'}^2
\right) \\
&=
\inv{( 1 + v {u_x}' )^2 } \left(
{{u}'}^2
+ 2 {u_x}' v
+ v^2
+v^2 {{u_x}'}^2
-v^2 {{u}'}^2
\right) \\
&=
\inv{( 1 + v {u_x}' )^2 } \left(
{{u}'}^2(1-v^2)
+ 2 {u_x}' v
+v^2 (1 + {{u_x}'}^2)
\right) \\
\end{align*}

\bibliographystyle{plainnat}
\bibliography{myrefs}

\end{document}
