%
% Copyright © 2012 Peeter Joot.  All Rights Reserved.
% Licenced as described in the file LICENSE under the root directory of this GIT repository.
%

% 
% 
\input{../peeter_prologue.tex}

\chapter{scratch}

%\beginArtWithToc
\beginArtNoToc

By process of elimination.

1.  Suppose $P$ is a vector, $P = \gamma^k P_k$, with $P_k$ scalars, then we'd have

\begin{align*}
\inv{2} \antisymmetric{\gamma_a \wedge \gamma_b}{P} 
&= 
(\gamma_a \wedge \gamma_b) \cdot (\gamma^k P_k) \\
&=
(\gamma_a {\delta_b}^k - \gamma_b {\delta_a}^k ) P_k \\
&=
\gamma_a P_b - \gamma_b P_a
\end{align*}

This is a vector, whereas your expression would be a scalar, so it doesn't look like what you are after.

2.  Suppose $P$ is a bivector, $P = (\gamma^k \wedge \gamma^m) P_{km}$, then the commutator will be a bivector not a vector.  This is a messier expansion (perhaps there's a clever way to do it, but I don't know what it is).

\begin{align*}
\inv{2} \antisymmetric{\gamma_a \wedge \gamma_b}{P} 
&= 
\gpgradetwo{ (\gamma_a \wedge \gamma_b) (\gamma^k \wedge \gamma^m) } P_{km} \\
&= 
\gpgradetwo{ (\gamma_a \gamma_b - \gamma_a \cdot \gamma_b) (\gamma^k \wedge \gamma^m) } P_{km} \\
&= 
\gpgradetwo{ \gamma_a (\gamma_b \cdot (\gamma^k \wedge \gamma^m)) } P_{km} 
+ \gpgradetwo{ \gamma_a (\gamma_b \wedge (\gamma^k \wedge \gamma^m)) } P_{km} 
- (\gamma_a \cdot \gamma_b) (\gamma^k \wedge \gamma^m) P_{km} \\
&= 
(\gamma_a \wedge \gamma^m) P_{b m} -(\gamma_a \wedge \gamma^k) P_{k b} - (\gamma_a \cdot \gamma_b) (\gamma^k \wedge \gamma^m) P_{km} \\
&+ (\gamma_a \cdot \gamma_b) (\gamma^k \wedge \gamma^m) P_{km} 
- (\gamma_b \wedge \gamma^m) P_{a m} 
+ (\gamma_b \wedge \gamma^k) P_{k a} 
\\
&= 
(\gamma_a \wedge \gamma^c) (P_{b c} -P_{c b})
+ (\gamma_b \wedge \gamma^c) (P_{c a} -P_{a c} )
\\
&= 
\eta_{ad}(\gamma^d \wedge \gamma^c) (P_{b c} -P_{c b})
- \eta_{bd} (\gamma^d \wedge \gamma^c) ( P_{a c} -P_{c a} )
\\
\end{align*}

If you let 

\begin{align*}
{P_m}^d = 2 (\gamma^d \wedge \gamma^c) (P_{m c} -P_{c m})
\end{align*}

you have

\begin{align*}
\antisymmetric{\gamma_a \wedge \gamma_b}{P} = \eta_{ad} {P_b}^d - \eta_{bd} {P_a}^d
\end{align*}

This looks something like what you are after, but has one too many non-free indexes.  That leaves just a trivector bivector product to consider ... but I'd rather go for a hot tub right now then consider that case;)



%\EndArticle
\EndNoBibArticle
