\documentclass{article}

\input{../peeters_macros.tex}
\input{../peeters_macros2.tex}

\usepackage[bookmarks=true]{hyperref}

\usepackage{color,cite,graphicx}
   % use colour in the document, put your citations as [1-4]
   % rather than [1,2,3,4] (it looks nicer, and the extended LaTeX2e
   % graphics package. 
\usepackage{latexsym,amssymb,epsf} % don't remember if these are
   % needed, but their inclusion can't do any damage


\title{ Energy momentum tensor }
\author{Peeter Joot}
\date{ Jan 01, 2009.  Last Revision: $Date: 2009/01/02 02:52:27 $ }

\begin{document}
\maketitle{}

%\tableofcontents
%\section{}

\cite{doran2003gap} defines (with $\epsilon_0$ ommitted),
the energy momentum stress tensor as a vector to
vector mapping of the following form:

\begin{align*}
T(a) 
&= \frac{\epsilon_0}{2} F a \tilde{F}
= - \frac{\epsilon_0}{2} F a F
\end{align*}


This quantity can only have vector, trivector, and five vector grades.Â  The 
grade five term must be zero

\begin{align*}
\gpgrade{T(a)}{5}
&= \frac{\epsilon_0}{2} F \wedge a \wedge \tilde{F} \\
&= \frac{\epsilon_0}{2} a \wedge (F \wedge \tilde{F}) \\
&= 0
\end{align*}

Since $\tilde{T(a)} = T(a)$, the grade three term is also zero (trivectors invert on reversion), so this must therefore be a vector.

As a vector this can be expanded in coordinates

\begin{align*}
T(a) 
&= \left(T(a) \cdot \gamma^\beta \right) \gamma_\beta \\
&= \left(T(a^\alpha \gamma_\alpha) \cdot \gamma^\beta \right) \gamma_\beta \\
&= a^\alpha \gamma^\beta \left(T(\gamma_\alpha) \cdot \gamma^\beta \right) \\
\end{align*}

It's this last bit that has the form of a traditional tensor, so we can write

\begin{align*}
T(a) &= a^\alpha \gamma^\beta {T_\alpha}^{\beta} \\
{T_\alpha}^{\beta} &= T(\gamma_\alpha) \cdot \gamma^\beta 
\end{align*}

Let's expand this tensor ${T_\alpha}^{\beta}$ explicitly to verify its form.

We want to expand, and dot with $\gamma^\beta$, the following

\begin{align*}
-2 \inv{\epsilon_0} \left(T(\gamma_\alpha) \cdot \gamma^\beta \right) \gamma_\beta 
&= \gpgradeone{(\grad \wedge A) \gamma_\alpha (\grad \wedge A)} \\
&= \gpgradeone{
(\grad \wedge A) \cdot \gamma_\alpha (\grad \wedge A)
+ (\grad \wedge A) \wedge \gamma^\alpha (\grad \wedge A)
} \\
&=
((\grad \wedge A) \cdot \gamma_\alpha) \cdot (\grad \wedge A)
+ ((\grad \wedge A) \wedge \gamma_\alpha) \cdot (\grad \wedge A)
\\
\end{align*}

Both of these will get temporarily messy, so let's do them in parts.Â  Starting
with

\begin{align*}
(\grad \wedge A) \cdot \gamma_\alpha
&= (\gamma^{a} \wedge \gamma^{b}) \cdot \gamma_{\alpha} \partial_{a} A_{b} \\
&= (\gamma^{a} {\delta^{b}}_{\alpha} -\gamma^{b} {\delta^{a}}_{\alpha} ) \partial_{a} A_{b} \\
&=
\gamma^{a} \partial_{a} A_{\alpha} 
-\gamma^{b} \partial_{\alpha} A_{b} \\
&= \gamma^{a} (\partial_{a} A_{\alpha} -\partial_{\alpha} A_{a} ) \\
&= \gamma^{a} F_{a \alpha} \\
\end{align*}


\begin{align*}
((\grad \wedge A) \cdot \gamma_\alpha) \cdot (\grad \wedge A) 
&= (\gamma^{a} F_{a \alpha}) \cdot (\gamma_{b} \wedge \gamma_{c}) \partial^{b} A^{c} \\
%&= 
%\partial^{b} A^{c} F_{a \alpha} 
%\gamma^{a} \cdot (\gamma_{b} \wedge \gamma_{c}) 
%\\
&= 
\partial^{b} A^{c} F_{a \alpha} 
(
{\delta^{a}}_{b} \gamma_{c}
-{\delta^{a}}_{c} \gamma_{b}
)
\\
&= 
(\partial^{a} A^{b} F_{a \alpha} -\partial^{b} A^{a} F_{a \alpha} )\gamma_{b}
\\
&= F^{a b} F_{a \alpha} \gamma_{b} \\
\end{align*}

So, by dotting with $\gamma^\beta$ we have

\begin{align}\label{eqn:firstPartDone}
((\grad \wedge A) \cdot \gamma_\alpha) \cdot (\grad \wedge A) \cdot \gamma^{\beta} 
&= F^{a \beta} F_{a \alpha} 
\end{align}

Moving on to the next bit,
$(((\grad \wedge A) \wedge \gamma^\alpha) \cdot (\grad \wedge A)) \cdot \gamma^\beta$.  By inspection the first part of this is

\begin{align*}
(\grad \wedge A) \wedge \gamma_\alpha
&= (\gamma_\alpha)^2 (\gamma^{a} \wedge \gamma^{b}) \wedge \gamma^{\alpha} \partial_{a} A_{b} \\
\end{align*}

so dotting with $\grad \wedge A$, we have

\begin{align*}
((\grad \wedge A) \wedge \gamma_\alpha) \cdot (\grad \wedge A)
&= 
(\gamma_\alpha)^2 
\partial_{a} A_{b} 
\partial^{c} A^{d} 
(\gamma^{a} \wedge \gamma^{b} \wedge \gamma^{\alpha}) \cdot 
(\gamma_{c} \wedge \gamma_{d})
\\
&= 
(\gamma_\alpha)^2 
\partial_{a} A_{b} 
\partial^{c} A^{d} 
((\gamma^{a} \wedge \gamma^{b} \wedge \gamma^{\alpha}) \cdot \gamma_{c} ) \cdot \gamma_{d}
\\
&= 
(\gamma_\alpha)^2 
\partial_{a} A_{b} 
\partial^{c} A^{d} 
(
%((\gamma^{a} \wedge \gamma^{b}) \wedge \gamma^{\alpha}) \cdot \gamma_{c} 
(\gamma^{a} \wedge \gamma^{b}) {\delta^{\alpha}}_{c}
-(\gamma^{a} \wedge \gamma^{\alpha}) {\delta^{b}}_{c}
+(\gamma^{b} \wedge \gamma^{\alpha}) {\delta^{a}}_{c}
) \cdot \gamma_{d}
\\
&= 
(\gamma_\alpha)^2 (
\partial_{a} A_{b} \partial^{\alpha} A^{d} (\gamma^{a} \wedge \gamma^{b}) 
-\partial_{a} A_{b} \partial^{b} A^{d} (\gamma^{a} \wedge \gamma^{\alpha}) 
+\partial_{a} A_{b} \partial^{a} A^{d} (\gamma^{b} \wedge \gamma^{\alpha}) 
) \cdot \gamma_{d}
\\
&= 
(\gamma_\alpha)^2 
\partial_{a} A_{b}
( \partial^{\alpha} A^{c} 
(\gamma^{a} \wedge \gamma^{b}) 
- \partial^{b} A^{c} (\gamma^{a} \wedge \gamma^{\alpha}) 
+ \partial^{a} A^{c} (\gamma^{b} \wedge \gamma^{\alpha}) 
) \cdot \gamma_{c}
\\
&= 
(\gamma_\alpha)^2 
\partial_{a} A_{b}
( 
+ \partial^{\alpha} A^{c}
%(\gamma^{a} \wedge \gamma^{b}) \cdot \gamma_c
(\gamma^{a} {\delta^{b}}_{c} -\gamma^{b} {\delta^{a}}_{c})
- \partial^{b} A^{c} 
%(\gamma^{a} \wedge \gamma^{\alpha}) \cdot \gamma_{c}
(\gamma^{a} {\delta^{\alpha}}_{c} -\gamma^{\alpha} {\delta^{a}}_{c})
+ \partial^{a} A^{c} 
%(\gamma^{b} \wedge \gamma^{\alpha}) \cdot \gamma_{c}
(\gamma^{b} {\delta^{\alpha}}_{c} -\gamma^{\alpha} {\delta^{b}}_{c})
) 
\\
&= 
 (\gamma_\alpha)^2 \partial_{a} A_{b} \partial^{\alpha} A^{c} (\gamma^{a} {\delta^{b}}_{c} -\gamma^{b} {\delta^{a}}_{c})
-(\gamma_\alpha)^2 \partial_{a} A_{b} \partial^{b} A^{c} (\gamma^{a} {\delta^{\alpha}}_{c} -\gamma^{\alpha} {\delta^{a}}_{c})
+(\gamma_\alpha)^2 \partial_{a} A_{b} \partial^{a} A^{c} (\gamma^{b} {\delta^{\alpha}}_{c} -\gamma^{\alpha} {\delta^{b}}_{c})
\\
&= 
(\gamma_\alpha)^2 \partial_{a} A_{b} \partial^{\alpha} A^{c} \gamma^{a} {\delta^{b}}_{c}
-(\gamma_\alpha)^2 \partial_{a} A_{b} \partial^{\alpha} A^{c} \gamma^{b} {\delta^{a}}_{c})
%
-(\gamma_\alpha)^2 \partial_{a} A_{b} \partial^{b} A^{c} \gamma^{a} {\delta^{\alpha}}_{c}
+(\gamma_\alpha)^2 \partial_{a} A_{b} \partial^{b} A^{c} \gamma^{\alpha} {\delta^{a}}_{c}
%
+(\gamma_\alpha)^2 \partial_{a} A_{b} \partial^{a} A^{c} \gamma^{b} {\delta^{\alpha}}_{c}
-(\gamma_\alpha)^2 \partial_{a} A_{b} \partial^{a} A^{c} \gamma^{\alpha} {\delta^{b}}_{c}
\\
&= 
(\gamma_\alpha)^2 \partial_{a} A_{b} \partial^{\alpha} A^{b} \gamma^{a} 
-(\gamma_\alpha)^2 \partial_{a} A_{b} \partial^{b} A^{\alpha} \gamma^{a} 
%
+(\gamma_\alpha)^2 \partial_{a} A_{b} \partial^{a} A^{\alpha} \gamma^{b}
-(\gamma_\alpha)^2 \partial_{a} A_{b} \partial^{\alpha} A^{a} \gamma^{b} 
%
+(\gamma_\alpha)^2 \partial_{a} A_{b} \partial^{b} A^{a} \gamma^{\alpha} 
-(\gamma_\alpha)^2 \partial_{a} A_{b} \partial^{a} A^{b} \gamma^{\alpha} 
\\
&= 
(\gamma_\alpha)^2 \partial_{a} A_{b} F^{\alpha b} \gamma^{a} 
+(\gamma_\alpha)^2 \partial_{a} A_{b} F^{a \alpha} \gamma^{b}
+\partial_{a} A_{b} F^{b a} \gamma_{\alpha} 
\\
&= 
\partial^{a} A^{b} F_{\alpha b} \gamma_{a} 
%+\partial^{a} A_{b} F_{a \alpha} \gamma^{b}
+\partial^{b} A_{a} F_{b \alpha} \gamma^{a}
+\partial_{a} A_{b} F^{b a} \gamma_{\alpha} 
\\
&= 
F^{a b} F_{\alpha b} \gamma_{a} 
+\partial_{a} A_{b} F^{b a} \gamma_{\alpha} 
\\
\end{align*}

So finally

\begin{align*}
((\grad \wedge A) \wedge \gamma_\alpha) \cdot (\grad \wedge A) \cdot \gamma^\beta
&= 
( F^{a b} F_{\alpha b} \gamma_{a} 
+\partial_{a} A_{b} F^{b a} \gamma_{\alpha} ) \cdot \gamma^\beta
\\
&= 
F^{\beta b} F_{\alpha b} 
+\partial_{a} A_{b} F^{b a} {\delta_{\alpha}}^\beta
\\
&= 
F^{\beta b} F_{\alpha b} 
+\inv{2}(
\partial_{a} A_{b} F^{b a} {\delta_{\alpha}}^\beta
+\partial_{b} A_{a} F^{a b} {\delta_{\alpha}}^\beta
)
\\
\end{align*}

\begin{align}\label{eqn:secondPart}
((\grad \wedge A) \wedge \gamma_\alpha) \cdot (\grad \wedge A) \cdot \gamma^\beta
&=
F^{\beta b} F_{\alpha b} 
+\inv{2} F_{a b} F^{b a} {\delta_{\alpha}}^\beta
\end{align}

The final combination of results \ref{eqn:firstPartDone}, and 
\ref{eqn:secondPart} gives

\begin{align*}
F \gamma_\alpha F 
&= 
2 F^{a \beta} F_{a \alpha} ) 
+\inv{2} F_{a b} F^{b a} {\delta_{\alpha}}^\beta
\end{align*}

Yielding the tensor

\begin{align*}
{T_\alpha}^{\beta}
&=
\epsilon_0 (
\inv{4} F_{a b} F^{a b} {\delta_{\alpha}}^\beta 
-
F_{a \alpha} 
F^{a \beta}
) 
\end{align*}

\bibliographystyle{plainnat}
\bibliography{myrefs}

\end{document}
