%
% Copyright © 2012 Peeter Joot.  All Rights Reserved.
% Licenced as described in the file LICENSE under the root directory of this GIT repository.
%

% 
% 
\chapter{Energy momentum tensor relation to Lorentz force. }\label{chap:PJenMtensor}
\date{Feb 17, 2009.  enMTensor.tex}

\section{Motivation. }

In \chapcite{PJstressEnergyLorentz} the energy momentum tensor was related
to the Lorentz force in STA form.  Work the same calculation strictly in
tensor form, to
%compare the difficulty of the algebra and
develop more comfort with tensor manipulation.  This should also serve
as a translation aid to compare signs due to metric tensor differences 
in other reading.

\subsection{Definitions. }

The energy momentum ``tensor'', really a four vector, is defined
in \citep{doran2003gap}
as

\begin{align}
T(a) &= 
\frac{\epsilon_0}{2} F a \tilde{F} = -\frac{\epsilon_0}{2} F a {F} 
\end{align}

We've seen that the divergence of the $T(\gamma^\mu)$ vectors generate
the Lorentz force relations.

Let's expand this with respect to index lower basis vectors for use in the
divergence calculation.

\begin{align}
T(\gamma^\mu) &= (T(\gamma^\mu) \cdot \gamma^\nu) \gamma_\nu 
\end{align}

So we define
\begin{align}
T^{\mu \nu} 
&= T(\gamma^\mu) \cdot \gamma^\nu
\end{align}

and can write these four vectors in tensor form as
\begin{align}
T(\gamma^\mu) &= T^{\mu \nu} \gamma_\nu 
\end{align}

\subsection{Expanding out the tensor. }

An expansion of $T^{\mu\nu}$ was done in \chapcite{PJemstresstensor}, but looking
back that seems a peculiar way, using the four vector potential.

Let's try again in terms of $F^{\mu\nu}$ instead.  Our field is

\begin{align}
F 
&= \inv{2} F^{\mu\nu} \gamma_{\mu} \wedge \gamma_\nu 
%\\
%&= \inv{2} F_{\mu\nu} \gamma^{\mu} \wedge \gamma^\nu
\end{align}

So our tensor components are
\begin{align*}
T^{\mu\nu}
&= T(\gamma^\mu) \cdot \gamma^\nu \\
&= -\frac{\epsilon_0}{8} F^{\lambda\sigma} F^{\alpha\beta} 
\gpgradezero{ (\gamma_\lambda \wedge \gamma_\sigma) \gamma^\mu (\gamma_\alpha \wedge \gamma_\beta) \gamma^\nu } \\
\end{align*}

Or
\begin{align*}
-8{\inv{\epsilon_0}} T^{\mu\nu}
&= 
F^{\lambda\sigma} F^{\alpha\beta} 
\gpgradezero{ 
(\gamma_\lambda {\delta_\sigma}^\mu 
-\gamma_\sigma {\delta_\lambda}^\mu)
(\gamma_\alpha {\delta_\beta}^\nu 
-\gamma_\beta {\delta_\alpha}^\nu)
} \\
&+
F^{\lambda\sigma} F^{\alpha\beta} 
\gpgradezero{ (\gamma_\lambda \wedge \gamma_\sigma \wedge \gamma^\mu) (\gamma_\alpha \wedge \gamma_\beta \wedge \gamma^\nu) } \\
\end{align*}

Expanding only the first term to start with
\begin{align*}
&
F^{\lambda\sigma} F^{\alpha\beta} (\gamma_\lambda {\delta_\sigma}^\mu) \cdot  (\gamma_\alpha {\delta_\beta}^\nu)  
+F^{\lambda\sigma} F^{\alpha\beta} (\gamma_\sigma {\delta_\lambda}^\mu) \cdot (\gamma_\beta {\delta_\alpha}^\nu)  \\
&-F^{\lambda\sigma} F^{\alpha\beta} (\gamma_\lambda {\delta_\sigma}^\mu) \cdot (\gamma_\beta {\delta_\alpha}^\nu) 
-F^{\lambda\sigma} F^{\alpha\beta} (\gamma_\sigma {\delta_\lambda}^\mu) \cdot (\gamma_\alpha {\delta_\beta}^\nu)  \\
&=
F^{\lambda\mu} F^{\alpha\nu} \gamma_\lambda \cdot \gamma_\alpha  
+F^{\mu\sigma} F^{\nu\beta} \gamma_\sigma \cdot \gamma_\beta  
-F^{\lambda\mu} F^{\nu\beta} \gamma_\lambda \cdot \gamma_\beta  
-F^{\mu\sigma} F^{\alpha\nu} \gamma_\sigma \cdot \gamma_\alpha \\
&=
\eta_{\alpha\beta} 
(
F^{\lambda\mu} F^{\alpha\nu} \gamma_\lambda \cdot \gamma^\beta  
+
%\eta_{\alpha\beta} 
F^{\mu\sigma} F^{\nu\alpha} \gamma_\sigma \cdot \gamma^\beta  
-
%\eta_{\alpha\beta} 
F^{\lambda\mu} F^{\nu\alpha} \gamma_\lambda \cdot \gamma^\beta  
-
%\eta_{\alpha\beta} 
F^{\mu\sigma} F^{\alpha\nu} \gamma_\sigma \cdot \gamma^\beta )
\\
&=
\eta_{\alpha\lambda} F^{\lambda\mu} F^{\alpha\nu} + \eta_{\alpha\sigma} F^{\mu\sigma} F^{\nu\alpha} 
- \eta_{\alpha\lambda} F^{\lambda\mu} F^{\nu\alpha} - \eta_{\alpha\sigma} F^{\mu\sigma} F^{\alpha\nu}  \\
&=
2( \eta_{\alpha\lambda} F^{\lambda\mu} F^{\alpha\nu} + \eta_{\alpha\sigma} F^{\mu\sigma} F^{\nu\alpha} ) \\
&=
2( \eta_{\alpha\beta} F^{\beta\mu} F^{\alpha\nu} + 
\eta_{\alpha\beta} F^{\mu\beta} F^{\nu\alpha} ) \\
&=
4 \eta_{\alpha\beta} F^{\beta\mu} F^{\alpha\nu}  \\
&= 4 F^{\beta\mu} {F_{\beta}}^{\nu} \\
&= 4 F^{\alpha\mu} {F_{\alpha}}^{\nu} \\
\end{align*}

For the second term after a shuffle of indexes we have
\begin{align*}
F^{\lambda\sigma} F_{\alpha\beta} 
\eta^{\mu\mu'} \gpgradezero{ (\gamma_\lambda \wedge \gamma_\sigma \wedge \gamma_\mu) (\gamma^\alpha \wedge \gamma^\beta \wedge \gamma^\nu) } \\
\end{align*}

This dot product is reducible with the identity
\begin{align*}
(a \wedge b \wedge c) \cdot (d \wedge e \wedge f) &= 
(((a \wedge b \wedge c) \cdot d) \cdot e) \cdot f 
\end{align*}

leaving a completely antisymmetized sum

\begin{align*}
&
F^{\lambda\sigma} F_{\alpha\beta} 
\eta^{\mu\mu'} 
(
{\delta_\lambda}^\nu {\delta_\sigma}^\beta {\delta_{\mu'}}^\alpha
-{\delta_\lambda}^\nu {\delta_\sigma}^\alpha {\delta_{\mu'}}^\beta
-{\delta_\lambda}^\beta {\delta_\sigma}^\nu {\delta_{\mu'}}^\alpha
+{\delta_\lambda}^\alpha {\delta_\sigma}^\nu {\delta_{\mu'}}^\beta
+{\delta_\lambda}^\beta {\delta_\sigma}^\alpha {\delta_{\mu'}}^\nu
-{\delta_\lambda}^\alpha {\delta_\sigma}^\beta {\delta_{\mu'}}^\nu
) \\
&=
  F^{\nu\beta} F_{{\mu'}\beta} \eta^{\mu\mu'} 
- F^{\nu\alpha} F_{\alpha{\mu'}} \eta^{\mu\mu'}
- F^{\beta\nu} F_{{\mu'}\beta} \eta^{\mu\mu'} 
+ F^{\alpha\nu} F_{\alpha{\mu'}} \eta^{\mu\mu'} 
+ F^{\beta\alpha} F_{\alpha\beta} \eta^{\mu\mu'} {\delta_{\mu'}}^\nu
- F^{\alpha\beta} F_{\alpha\beta} \eta^{\mu\mu'} {\delta_{\mu'}}^\nu
 \\
&=
4 F^{\nu\alpha} F_{{\mu'}\alpha} \eta^{\mu\mu'} 
+ 2 F^{\beta\alpha} F_{\alpha\beta} \eta^{\mu\mu'} {\delta_{\mu'}}^\nu
 \\
&=
4 F^{\nu\alpha} {F^{\mu}}_{\alpha} 
+ 2 F^{\beta\alpha} F_{\alpha\beta} \eta^{\mu\nu} 
 \\
\end{align*}

Combining these we have
\begin{align*}
T^{\mu\nu}
&= 
-\frac{\epsilon_0}{8} \left(
 4 F^{\alpha\mu} {F_{\alpha}}^{\nu} 
+ 4 F^{\nu\alpha} {F^{\mu}}_{\alpha} 
+ 2 F^{\beta\alpha} F_{\alpha\beta} \eta^{\mu\nu} 
\right) \\
&= 
\frac{\epsilon_0}{8} \left(
- 4 F^{\alpha\mu} {F_{\alpha}}^{\nu} 
+ 4 F^{\alpha\mu} {F^{\nu}}_{\alpha}
+ 2 F^{\alpha\beta} F_{\alpha\beta} \eta^{\mu\nu} 
\right) \\
\end{align*}


If by some miracle all the index manipulation worked out, we have
\begin{align}\label{eqn:stressEnTen:miracle}
T^{\mu\nu} &= {\epsilon_0} \left( F^{\alpha\mu} {F^{\nu}}_{\alpha} + \inv{4} F^{\alpha\beta} F_{\alpha\beta} \eta^{\mu\nu} \right)
\end{align}

\subsubsection{Justifying some of the steps. }

For justification of some of the 
index manipulations of the $F$ tensor components it is 
helpful to think back to the definitions in terms of four vector potentials

\begin{align*}
F &= \grad \wedge A \\
&= \partial^\mu A^\nu \gamma_\mu \wedge \gamma_\nu \\
&= \partial_\mu A_\nu \gamma^\mu \wedge \gamma^\nu \\
&= \partial_\mu A^\nu \gamma^\mu \wedge \gamma_\nu \\ 
&= \partial^\mu A_\nu \gamma_\mu \wedge \gamma^\nu \\
&= \inv{2}(\partial^\mu A^\nu -\partial^\nu A^\mu ) \gamma_\mu \wedge \gamma_\nu \\
&= \inv{2}(\partial_\mu A_\nu -\partial_\nu A_\mu ) \gamma^\mu \wedge \gamma^\nu \\
&= \inv{2}(\partial_\mu A^\nu -\partial^\nu A_\mu ) \gamma^\mu \wedge \gamma_\nu \\ 
&= \inv{2}(\partial^\mu A_\nu -\partial_\nu A^\mu ) \gamma_\mu \wedge \gamma^\nu
\end{align*}

So with the shorthand
\begin{align*}
F^{\mu\nu} &= \partial^\mu A^\nu -\partial^\nu A^\mu \\
F_{\mu\nu} &= \partial_\mu A_\nu -\partial_\nu A_\mu \\
{F_{\mu}}^{\nu} &= \partial_\mu A^\nu -\partial^\nu A_\mu \\
{F^{\mu}}_{\nu} &= \partial^\mu A_\nu -\partial_\nu A^\mu
\end{align*}

We have
\begin{align*}
F 
&= \inv{2}F^{\mu\nu} \gamma_\mu \wedge \gamma_\nu \\
&= \inv{2}F_{\mu\nu} \gamma^\mu \wedge \gamma^\nu \\
&= \inv{2}{F_\mu}^\nu \gamma^\mu \wedge \gamma_\nu \\ 
&= \inv{2}{F^\mu}_\nu \gamma_\mu \wedge \gamma^\nu
\end{align*}

In particular, and perhaps not obvious without the definitions handy, the following was used above

\begin{align*}
{F^{\mu}}_{\nu} &= -{F_{\nu}}^{\mu}
\end{align*}

\subsection{The divergence. }

What's our divergence in tensor form?  This would be

\begin{align*}
\grad \cdot T(\gamma^\mu)
&= (\gamma^\alpha \partial_\alpha ) \cdot (T^{\mu\nu} \gamma_\nu) \\
\end{align*}

So we have
\begin{align}
\grad \cdot T(\gamma^\mu)
&= \partial_\nu T^{\mu\nu}
\end{align}

Ignoring the $\epsilon_0$ factor for now, chain rule gives us

\begin{align*}
(\partial_\nu &F^{\alpha\mu}) {F^{\nu}}_{\alpha} + 
F^{\alpha\mu} (\partial_\nu {F^{\nu}}_{\alpha}) + 
\inv{2} (\partial_\nu F^{\alpha\beta}) F_{\alpha\beta} \eta^{\mu\nu} \\
&=
(\partial_\nu F^{\alpha\mu}) {F^{\nu}}_{\alpha} + 
{F_{\alpha}}^{\mu} 
(\partial_\nu F^{\nu\alpha}) + 
\inv{2} (\partial_\nu F^{\alpha\beta}) F_{\alpha\beta} \eta^{\mu\nu} 
\end{align*}

Only this center term is recognizable in terms of current since we
have
\begin{align*}
\grad \cdot F &= J/\epsilon_0 c
\end{align*}

Where the LHS is
\begin{align*}
\grad \cdot F 
&= \gamma^\alpha \partial_\alpha \cdot \left( \inv{2} F^{\mu\nu} \gamma_\mu \wedge \gamma_\nu \right) \\
&= \inv{2} \partial_\alpha F^{\mu\nu} ( {\delta^\alpha}_\mu \gamma_\nu -{\delta^\alpha}_\nu \gamma_\mu ) \\
&= \partial_\mu F^{\mu\nu} \gamma_\nu
\end{align*}

So we have

\begin{align*}
\partial_\mu F^{\mu\nu} 
&= (J \cdot \gamma^\nu)/\epsilon_0 c \\
&= ((J^\alpha \gamma_\alpha) \cdot \gamma^\nu)/\epsilon_0 c \\
&= J^\nu/\epsilon_0 c
\end{align*}

Or
\begin{align}
\partial_\mu F^{\mu\nu} &= J^\nu/\epsilon_0 c
\end{align}
%\partial_\nu F^{\nu\alpha} &= J^\alpha/\epsilon_0 c

So we have

\begin{align*}
\grad \cdot T(\gamma^\mu) 
&= \epsilon_0\left(
(\partial_\nu F^{\alpha\mu}) {F^{\nu}}_{\alpha} + 
\inv{2} (\partial_\nu F^{\alpha\beta}) F_{\alpha\beta} \eta^{\mu\nu} 
\right)
+
{F_{\alpha}}^{\mu} J^\alpha/c
\end{align*}

So, to get the expected result the remaining two derivative terms must somehow cancel.  How to reduce these?  Let's look at twice that

\begin{align*}
2 (\partial_\nu &F^{\alpha\mu}) {F^{\nu}}_{\alpha} + (\partial_\nu F^{\alpha\beta}) F_{\alpha\beta} \eta^{\mu\nu} \\
&= 2 (\partial^\nu F^{\alpha\mu}) F_{\nu\alpha} + (\partial^\mu F^{\alpha\beta}) F_{\alpha\beta} \\
&= (\partial^\nu F^{\alpha\mu}) (F_{\nu\alpha} -F_{\alpha\nu}) + (\partial^\mu F^{\alpha\beta}) F_{\alpha\beta} \\
&= 
(\partial^\alpha F^{\beta\mu}) F_{\alpha\beta} 
+(\partial^\beta F^{\mu\alpha}) F_{\alpha\beta}
+ (\partial^\mu F^{\alpha\beta}) F_{\alpha\beta} \\
&= 
(\partial^\alpha F^{\beta\mu} +\partial^\beta F^{\mu\alpha} + \partial^\mu F^{\alpha\beta}) F_{\alpha\beta} \\
\end{align*}

Ah, there's the trivector term of Maxwell's equation hiding in there.

\begin{align*}
0
&= \grad \wedge F \\
&= \gamma_\mu \partial^\mu \wedge \left(\inv{2} F^{\alpha\beta} (\gamma_\alpha \wedge \gamma_\beta) \right) \\
&= \inv{2} (\partial^\mu F^{\alpha\beta}) (\gamma_\mu \wedge \gamma_\alpha \wedge \gamma_\beta) \\
&= \inv{3!} 
\left(
\partial^\mu F^{\alpha\beta}
+\partial^\alpha F^{\beta\mu} 
+\partial^\beta F^{\mu\alpha}
\right)
(\gamma_\mu \wedge \gamma_\alpha \wedge \gamma_\beta)
\end{align*}

Since this is zero, each component of this trivector must separately equal zero, and we have

\begin{align}
\partial^\mu F^{\alpha\beta} +\partial^\alpha F^{\beta\mu} +\partial^\beta F^{\mu\alpha} = 0
\end{align}

So, where $T^{\mu\nu}$ is defined by \ref{eqn:stressEnTen:miracle}, the final result is

\begin{align}\label{eqn:stressEnTen:covariantTensor}
\partial_\nu T^{\mu\nu} &= F^{\alpha\mu} J_\alpha/c
\end{align}
