\documentclass{article}

\input{../peeters_macros.tex}
\input{../peeters_macros2.tex}

%\usepackage{listings}
%\usepackage{txfonts} % for ointctr... (also appears to make "prettier" \int and \sum's)
% makes \grad look funny though (almost like spacegrad, but narrower)
\usepackage[bookmarks=true]{hyperref}

\usepackage{color,cite,graphicx}
   % use colour in the document, put your citations as [1-4]
   % rather than [1,2,3,4] (it looks nicer, and the extended LaTeX2e
   % graphics package. 
\usepackage{latexsym,amssymb,epsf} % don't remember if these are
   % needed, but their inclusion can't do any damage


\title{ Lorentz boost of Lorentz force equations. }
\author{Peeter Joot \quad peeter.joot@gmail.com }
\date{ May 23, 2009.  Last Revision: $Date: 2009/05/24 03:56:22 $ }

\begin{document}

\maketitle{}
\tableofcontents
\section{ Motivation. }

Reading of \cite{bohm1996str} is a treatment of the Lorentz transform
properties of the Lorentz force equation.  This isn't clear to me
without working through it myself, but in doing so I have the urge to
try it with the GA formulation of the Lorentz transformation.

\section{ GA Lorentz tx. }

I've got the coordinate and Geometric Algebra versions of the Lorentz
transform all mixed up in my head.  Let's work through the relations 
between these once more.

Write the Lorentz boost of a four vector $x = x^\mu \gamma_\mu = ct \gamma_0 + x^k \gamma_k$ as

\begin{align}\label{eqn:LorentzBoost}
L(x) &= 
e^{-\alpha \vcap/2}
x
e^{\alpha \vcap/2}
\end{align}

\subsection{ Invariance property. }

A Lorentz transformation (boost or rotation) can be defined as those transformation that leave the four vector square unchanged.

Following \cite{doran2003gap}, work with a $+---$ metric signature ($1 = \gamma_0^2 = -\gamma_k^2$), and $\sigma_k = \gamma_k \gamma_0$.  Our four vector square in this representation has the familiar invariant form

\begin{align*}
x^2 
&= (ct \gamma_0 + x^m \gamma_m) (ct \gamma_0 + x^k \gamma_k) \\
&= (ct \gamma_0 + x^m \gamma_m) \gamma_0^2 (ct \gamma_0 + x^k \gamma_k) \\
&= (ct + x^m \sigma_m) (ct - x^k \sigma_k) \\
&= (ct + \Bx) (ct - \Bx) \\
&= (ct)^2 - \Bx^2
\end{align*}

and we expect this of the Lorentz boost of equation \ref{eqn:LorentzBoost}.  To verify we have

\begin{align*}
L(x)^2 
&=
e^{-\alpha \vcap/2}
x
e^{\alpha \vcap/2}
e^{-\alpha \vcap/2}
x
e^{\alpha \vcap/2} \\
&=
e^{-\alpha \vcap/2}
x
x
e^{\alpha \vcap/2} \\
&=
x^2
e^{-\alpha \vcap/2}
e^{\alpha \vcap/2} \\
&=
x^2
\end{align*}

\subsection{ Sign of the rapidity angle. }

The factor $\alpha$ will be the rapidity angle, but what sign do we want for a boost along the positive $\vcap$ direction?

Dropping to coordinates is an easy way to determine the sign convention in effect.  Write $\vcap = \sigma_1$

\begin{align*}
L(x) &= 
e^{-\alpha \vcap/2}
x
e^{\alpha \vcap/2} \\
&=
(\cosh(\alpha/2) - \sigma_1 \sinh(\alpha/2))
(
x^0 \gamma_0
+x^1 \gamma_1
+x^2 \gamma_2
+x^3 \gamma_3
)
(\cosh(\alpha/2) + \sigma_1 \sinh(\alpha/2))
\end{align*}

$\sigma_1$ commutes with $\gamma_2$ and $\gamma_3$ and anticommutes otherwise, so we have

\begin{align*}
L(x) &= 
(
x^2 \gamma_2
+x^3 \gamma_3
) 
e^{-\alpha \vcap/2}
e^{\alpha \vcap/2}
+
(
x^0 \gamma_0
+x^1 \gamma_1
)
e^{\alpha \vcap} \\
&=
x^2 \gamma_2
+x^3 \gamma_3
+(
x^0 \gamma_0
+x^1 \gamma_1
)
e^{\alpha \vcap} \\
&=
x^2 \gamma_2
+x^3 \gamma_3
+(
x^0 \gamma_0
+x^1 \gamma_1
)
(\cosh(\alpha) + \sigma_1 \sinh(\alpha))
\end{align*}

Expanding out just the $0,1$ terms changed by the transformation we have

\begin{align*}
(
&x^0 \gamma_0
+x^1 \gamma_1
)
(\cosh(\alpha) + \sigma_1 \sinh(\alpha)) \\
&=
x^0 \gamma_0 \cosh(\alpha) 
+x^1 \gamma_1 \cosh(\alpha) 
+x^0 \gamma_0 \sigma_1 \sinh(\alpha)
+x^1 \gamma_1 \sigma_1 \sinh(\alpha) \\
&=
x^0 \gamma_0 \cosh(\alpha) 
+x^1 \gamma_1 \cosh(\alpha) 
+x^0 \gamma_0 \gamma_1 \gamma_0 \sinh(\alpha)
+x^1 \gamma_1 \gamma_1 \gamma_0 \sinh(\alpha) \\
&=
x^0 \gamma_0 \cosh(\alpha) 
+x^1 \gamma_1 \cosh(\alpha) 
-x^0 \gamma_1 \sinh(\alpha)
-x^1 \gamma_0 \sinh(\alpha) \\
&=
\gamma_0 (x^0 \cosh(\alpha) -x^1 \sinh(\alpha) )
+\gamma_1 (x^1 \cosh(\alpha) -x^0 \sinh(\alpha) )
\\
\end{align*}

Writing ${x^\mu}' = L(x) \cdot \gamma^\mu$, and $x^\mu = x \cdot \gamma^\mu$,
and a substitution of $\cosh(\alpha) = 1/\sqrt{1 - \Bv^2/c^2}$, and $\alpha \vcap = \tanh^{-1}(\Bv/c)$,
we have the traditional coordinate
expression for the one directional Lorentz boost

\begin{align}
\begin{bmatrix}
{x^0}' \\
{x^1}' \\
{x^2}' \\
{x^3}'
\end{bmatrix}
&=
\begin{bmatrix}
\cosh\alpha & -\sinh\alpha & 0 & 0 \\
-\sinh\alpha & \cosh\alpha & 0 & 0 \\
0 & 0 & 1 & 0 \\
0 & 0 & 0 & 1 \\
\end{bmatrix}
\begin{bmatrix}
x^0 \\
x^1 \\
x^2 \\
x^3
\end{bmatrix}
\end{align}

Performing this expansion showed initially showed that I had the wrong sign for $\alpha$ in the exponentials and I went back and
adjusted it all accordingly.

\subsection{ Expanding out the Lorentz boost for projective and rejective directions. }

Two forms of Lorentz boost representations have been compared above.  An additional one is used in the Bohm text (a 
vector form of the Lorentz transformation not using coordinates).  Let's see
if we can derive that from the exponential form.

Start with computation of components of a four vector relative to an observer timelike unit vector $\gamma_0$.

\begin{align*}
x 
&= x \gamma_0 \gamma_0 \\
&= (x \gamma_0) \gamma_0 \\
&= (x \cdot \gamma_0 + x \wedge \gamma_0) \gamma_0 \\
\end{align*}

For the spatial vector factor above write $\Bx = x \wedge \gamma_0$, for

\begin{align*}
x 
&= (x \cdot \gamma_0) \gamma_0 + \Bx \gamma_0 \\
&= (x \cdot \gamma_0) \gamma_0 + \Bx \vcap \vcap \gamma_0 \\
&= (x \cdot \gamma_0) \gamma_0 + (\Bx \cdot \vcap) \vcap \gamma_0 + (\Bx \wedge \vcap) \vcap \gamma_0 \\
\end{align*}

We have the following commutation relations for the various components
\begin{align*}
\vcap (\gamma_0) &= - \gamma_0 \vcap \\
\vcap (\vcap \gamma_0) &= - (\vcap \gamma_0) \vcap \\
\vcap ((\Bx \wedge \vcap) \vcap \gamma_0 ) 
%&= -(\Bx \wedge \vcap) \vcap \vcap \gamma_0 
&= ((\Bx \wedge \vcap) \vcap \gamma_0) \vcap
\end{align*}

For a four vector $u$ that commutes with $\vcap$ we have $e^{-\alpha \vcap/2} u = u e^{-\alpha \vcap/2}$, and if it anticommutes
we have the conjugate relation
$e^{-\alpha \vcap/2} u = u e^{\alpha \vcap/2}$.  This gives us

\begin{align*}
L(x) 
&= 
(\Bx \wedge \vcap) \vcap \gamma_0 +
\left( (x \cdot \gamma_0) \gamma_0 + (\Bx \cdot \vcap) \vcap \gamma_0 \right) e^{\alpha \vcap} \\
\end{align*}

Now write the exponential as a scalar and spatial vector sum
\begin{align*}
e^{\alpha \vcap}
&= 
\cosh\alpha 
+\vcap \sinh\alpha 
\\
&= 
\gamma (1 +\vcap \tanh\alpha )
\\
&= 
\gamma (1 +\vcap \beta)
\\
&= 
\gamma (1 + \Bv/c )
\\
\end{align*}

Expanding out the exponential product above, also writing $x^0 = ct = x \cdot \gamma_0$, we have

\begin{align*}
( &x^0 \gamma_0 + (\Bx \cdot \vcap) \vcap \gamma_0 ) e^{\alpha \vcap} \\
&=
\gamma ( x^0 \gamma_0 + (\Bx \cdot \vcap) \vcap \gamma_0 ) ( 1 + \Bv/c ) \\
&=
\gamma ( 
x^0 \gamma_0 
+ (\Bx \cdot \vcap) \vcap \gamma_0 
+x^0 \gamma_0 \Bv/c  
+ (\Bx \cdot \vcap) \vcap \gamma_0 \Bv/c
) \\
\end{align*}

So for the total Lorentz boost in vector form we have

\begin{align}
L(x)
&=
(\Bx \wedge \vcap) \vcap \gamma_0 +
\gamma \left(x^0 - \Bx \cdot \frac{\Bv}{c} \right) \gamma_0
+ \gamma \left( \Bx \cdot \inv{\Bv/c} - x^0 \right) \frac{\Bv}{c} \gamma_0
\end{align}

Equation (15-12) from the text was

\begin{align*}
\Bx' 
&= \Bx - (\vcap \cdot \Bx) \vcap + \frac{ (\vcap \cdot \Bx )\vcap - \Bv t }{ \sqrt{1 - (v^2/c^2)} } \\
t' 
&= \frac{ t - (\vcap \cdot \Bx )/c^2 }{ \sqrt{1 - (v^2/c^2)} } \\
\end{align*}

and a visual inspection shows that this does match as desired.

\bibliographystyle{plainnat}
\bibliography{myrefs}

\end{document}
