\documentclass{article}

\input{../peeters_macros.tex}
\input{../peeters_macros2.tex}

\usepackage[bookmarks=true]{hyperref}

\usepackage{color,cite,graphicx}
   % use colour in the document, put your citations as [1-4]
   % rather than [1,2,3,4] (it looks nicer, and the extended LaTeX2e
   % graphics package. 
\usepackage{latexsym,amssymb,epsf} % don't remember if these are
   % needed, but their inclusion can't do any damage


\title{ Poynting vector and Electromagnetic Energy conservation. }
\author{Peeter Joot}
\date{ Dec 29, 2008.  Last Revision: $Date: 2008/12/31 01:06:10 $ }

\begin{document}

\maketitle{}

\tableofcontents

\section{ Motivation. }

Clarify Poynting discussion from \cite{doran2003gap}.

Equation 7.59 and 7.60 derives a $\BE \cross \BB$ quantity, the Poynting vector, as a sort of energy flux through the surface of the containing volume.

There are a couple of magic steps here that were not at all obvious to me.  Go through this in enough detail that it makes sense to me.

\section{ Charge free case. }

In SI units the Energy density is given as

\begin{align*}
U = \frac{\epsilon_0}{2}\left( \BE^2 + c^2 \BB^2 \right)
\end{align*}

FIXME: Don't truely understand where this part comes from.  The article \href{http://farside.ph.utexas.edu/teaching/em/lectures/node89.html}{Energy Conservation} looks promising to study this.

Given this energy density the rate of change of energy in a volume is then

\begin{align*}
\frac{dU}{dt} 
&= 
\frac{d}{dt} 
\frac{\epsilon_0}{2} \int dV \left( \BE^2 + c^2 \BB^2 \right) \\
&= 
\epsilon_0 \int dV \left( \BE \cdot \PD{t}{\BE} + c^2 \BB \cdot \PD{t}{\BB} \right) \\
\end{align*}

The next (omitted in the text) step is to utilize Maxwell's equation to eliminate the time derivatives.  Since this is the
charge and current free case, we can write Maxwell's as

\begin{align*}
0
&= \gamma_0 \grad F \\
&= \gamma_0 (\gamma^0 \partial_0 + \gamma^k \partial_k) F \\
&= (\partial_0 + \gamma_k\gamma_0 \partial_k) F \\
&= (\partial_0 + \sigma_k \partial_k) F \\
&= (\partial_0 + \spacegrad)F \\
&= (\partial_0 + \spacegrad)(\BE + ic \BB) \\
&= \partial_0 \BE + ic \partial_0 \BB + \spacegrad \BE + ic \spacegrad \BB \\
\end{align*}

In the spatial ($\sigma$) basis we can separate this into even and odd grades, which are separately equal to zero

\begin{align*}
0 &= \partial_0 \BE + ic \spacegrad \BB \\
%   1                  3,1 
0 &= ic \partial_0 \BB + \spacegrad \BE 
%  2                    0,2
\end{align*}

A selection of just the vector parts is

\begin{align*}
\partial_t \BE &= - ic^2 \spacegrad \wedge \BB \\
\partial_t \BB &= i\spacegrad \wedge \BE 
\end{align*}

Which can be back substituited into the energy flux
\begin{align*}
\frac{dU}{dt} 
&= \epsilon_0 \int dV \left( \BE \cdot (-i c^2 \spacegrad \wedge \BB) + c^2 \BB \cdot (i \spacegrad \wedge \BE) \right) \\
&= \epsilon_0 c^2 \int dV \gpgradezero{ \BB i \spacegrad \wedge \BE -\BE i \spacegrad \wedge \BB } \\
\end{align*}

Since the two divergence terms are zero we can drop the wedges here for

\begin{align*}
\frac{dU}{dt} 
&= \epsilon_0 c^2 \int dV \gpgradezero{ \BB i \spacegrad \BE -\BE i \spacegrad \BB } \\
&= \epsilon_0 c^2 \int dV \gpgradezero{ (i \BB) \spacegrad \BE -\BE \spacegrad (i\BB) } \\
&= \epsilon_0 c^2 \int dV \spacegrad \cdot ( (i \BB) \cdot \BE ) \\
\end{align*}

Justification for this last step can be found below in the derivation of equation \ref{eqn:poyntingDivergence}.

We can now use Stokes theorem to change this into a surface integral for a final energy flux 

\begin{align*}
\frac{dU}{dt} 
&= \epsilon_0 c^2 \int d\BA \cdot ( (i \BB) \cdot \BE ) \\
\end{align*}

This last bivector/vector dot product is the Poynting vector

\begin{align*}
(i \BB) \cdot \BE 
&= \gpgradeone{ (i \BB) \cdot \BE } \\
&= \gpgradeone{ i \BB \BE } \\
&= \gpgradeone{ i (\BB \wedge \BE) } \\
&= i (\BB \wedge \BE) \\
&= i^2(\BB \cross \BE) \\
&= \BE \cross \BB \\
\end{align*}

So, we can identity the quantity 

\begin{align}\label{eqn:poynting}
\epsilon_0 c^2 \BE \cross \BB = \epsilon_0 c (i c \BB) \cdot \BE 
\end{align}

As a directed energy density flux through the surface of a containing volume.


\section{ With charges and currents }
 
To calculate time derivatives we want to take Maxwell's equation and put into a form with explicit time derivatives, as was done before, but this time be more careful with the handling of the four vector current term.  Starting with left factoring out of a $\gamma_0$ from the spacetime gradient. 
 
\begin{align*}
\grad &= \gamma^0 \partial_0 + \gamma^k \partial_k \\
&= \gamma^0 (\partial_0 - \gamma^k \gamma_0 \partial_k) \\
&= \gamma^0 (\partial_0 + \sigma_k \partial_k) \\
\end{align*}

Similarily, the $\gamma_0$ can be factored from the current density

\begin{align*}
J 
&= \gamma_0 c \rho + \gamma_k J^k \\
&= \gamma_0 (c \rho - \gamma_k \gamma_0 J^k) \\
&= \gamma_0 (c \rho - \sigma_k J^k) \\
&= \gamma_0 (c \rho - \Bj )
\end{align*}

With this Maxwell's equation becomes
 
\begin{align*}
\gamma_0 \grad F &= \gamma_0 J / \epsilon_0 c \\
(\partial_0 + \spacegrad) ( \BE + i c \BB ) &= \rho/\epsilon_0 - \Bj/\epsilon_0 c \\
\end{align*}
 
A split into even and odd grades including current and charge density is thus
 
\begin{align*}
\spacegrad \BE + \partial_t (i \BB) &= \rho/\epsilon_0 \\
\spacegrad (i \BB) c^2 + \partial_t \BE &= -\Bj/\epsilon_0
\end{align*}
 
Now, taking time derivatives of the energy density gives

\begin{align*}
\PD{t}{U} 
&= \PD{t}{}\inv{2} \epsilon_0 \left( \BE^2 - (ic \BB)^2 \right) \\
&= \epsilon_0 \left( \BE \cdot \partial_t \BE - c^2 (i\BB) \cdot \partial_t (i\BB) \right) \\
&= \epsilon_0 \gpgradezero{ \BE ( -\Bj/\epsilon_0 -\spacegrad (i \BB) c^2 ) - c^2 (i\BB) ( -\spacegrad \BE + \rho/\epsilon_0 ) } \\
&= -\BE \cdot \Bj + c^2 \epsilon_0 \gpgradezero{ i\BB \spacegrad \BE -\BE \spacegrad (i \BB) } \\
&= -\BE \cdot \Bj + c^2 \epsilon_0 \left( (i\BB) \cdot (\spacegrad \wedge \BE) - \BE \cdot (\spacegrad \cdot (i \BB)) \right) \\
\end{align*}

Using equation \ref{eqn:poyntingDivergence}, we now have the rate of change of
field energy for the general case including currents.  That is

\begin{align}
\PD{t}{U} &= -\BE \cdot \Bj + c^2 \epsilon_0 \spacegrad \cdot (\BE \cdot (i\BB)) 
\end{align}

Written out in full, and in terms of the Poynting vector this is

\begin{align}
\PD{t}{}\frac{\epsilon_0}{2} \left(\BE^2 + c^2 \BB^2\right) + c^2 \epsilon_0 \spacegrad \cdot (\BE \cross \BB) &= -\BE \cdot \Bj 
\end{align}

\section{ Poynting vector in terms of complete field. }

In equation \ref{eqn:poynting} the individual parts of the complete Faraday
bivector $F = \BE + i c \BB$ stand out.  How would the Poynting vector be
expressed in terms of $F$ or in tensor form?

Since
\begin{align*}
F \gamma_0 = - \gamma_0(\BE - i c \BB)
\end{align*}

we have
\begin{align*}
\gamma^0 F \gamma_0 = - (\BE - i c \BB)
\end{align*}

and
\begin{align*}
i c \BB &= \inv{2}(F + \gamma^0 F \gamma_0) \\
\BE &= \inv{2}(F - \gamma^0 F \gamma_0) \\
\end{align*}

FIXME: tried using these but messed up.

%Without justifying all the steps I think that the following is valid
%
%\begin{align*}
%(i c \BB) \cdot \BE 
%&= \gpgradeone{(i c \BB) \cdot \BE } \\
%&= \gpgradeone{i c \BB \BE } \\
%&= \inv{4} (F + \gamma_0 F \gamma_0) \cdot (F - \gamma_0 F \gamma_0) \\
%&= \inv{4} (F^2 - \gamma_0 F \gamma_0 \gamma_0 F \gamma_0 + (\gamma_0 F \gamma_0) \cdot F - F \cdot (\gamma_0 F \gamma_0) ) \\
%&= \inv{4} ( (\gamma_0 F \gamma_0) \cdot F - F \cdot (\gamma_0 F \gamma_0) ) \\
%&= \inv{2} (\gamma_0 F \gamma_0) \cdot F 
%\end{align*}
%
%  The above is wrong.  This is - <F^\dagger F>/2, which is c^2 B^2 - E^2, which isn't even vector.

\section{ Energy Density from Lagrangian. }

I didn't get too far trying to calculate the electrodynamic Hamiltonian density for the general case, so I tried it for a very 
simple special case, with just an electric field component in one direction:

\begin{align*}
\mathcal{L}
&= \frac{1}{2}(E_x)^2 \\
&= \frac{1}{2}(F_{01})^2 \\
&= \frac{1}{2}(\partial_0 A_1 - \partial_1 A_0)^2 \\
\end{align*}

Goldstein gives the Hamiltonian density as

\begin{align*}
\pi &= \frac{\partial \mathcal{L}}{\partial \dot{n}} \\
\mathcal{H} &= \dot{n} \pi - \mathcal{L}
\end{align*}

If I try calculating this I get

\begin{align*}
\pi 
&= \frac{\partial}{\partial (\partial_0 A_1)} \left( \frac{1}{2}(\partial_0 A_1 - \partial_1 A_0)^2 \right) \\
&= \partial_0 A_1 - \partial_1 A_0 \\
&= F_{01} \\
\end{align*}

So this gives a Hamiltonian of
\begin{align*}
\mathcal{H}
&= \partial_0 A_1 F_{01} - \frac{1}{2}(\partial_0 A_1 - \partial_1 A_0)F_{01} \\
&= \frac{1}{2} (\partial_0 A_1 + \partial_1 A_0 )F_{01} 
&= \frac{1}{2} ((\partial_0 A_1)^2 - (\partial_1 A_0)^2 )
\end{align*}

For a Lagrangian density of $E^2 - B^2$ we have an energy density of $E^2 + B^2$, so I'd have expected the Hamiltonian density here to stay equal to $E_x^2/2$, but it 
doesn't look like that's what I get (what I calculated isn't at all familiar seeming).

If I haven't made a mistake here, perhaps I'm incorrect in assuming that the Hamiltonian density of the electrodynamic Lagrangian should be the energy density?

\section{ Appendix.  Messy details. }

For both the charge and the charge free case, we need a proof of 

\begin{align*}
(i\BB) \cdot (\spacegrad \wedge \BE) - \BE \cdot (\spacegrad \cdot (i \BB)) 
&= \spacegrad \cdot (\BE \cdot (i\BB)) 
\end{align*}

This is relativity straightforward, albeit tedious, to do backwards.

\begin{align*}
\spacegrad \cdot ((i \BB) \cdot \BE)
&= \gpgradezero{ \spacegrad ((i \BB) \cdot \BE)} \\
&= \inv{2} \gpgradezero{ \spacegrad ( i \BB \BE - \BE i \BB ) } \\
&= \inv{2} \gpgradezero{ 
  \dot{\spacegrad} i \dot{\BB} \BE 
+ \dot{\spacegrad} i \BB \dot{\BE}
- \dot{\spacegrad} \dot{\BE} i \BB 
- \dot{\spacegrad} \BE i \dot{\BB}
} \\
&= \inv{2} \gpgradezero{ 
  \BE \spacegrad (i \BB) - (i\dot{\BB}) \dot{\spacegrad} \BE
+ \dot{\BE} \dot{\spacegrad} i \BB - i \BB \spacegrad \BE
} \\
&= \inv{2} \left(
  \BE \cdot (\spacegrad \cdot (i \BB)) - ((i\dot{\BB}) \cdot \dot{\spacegrad}) \cdot \BE
+ (\dot{\BE} \wedge \dot{\spacegrad}) \cdot (i \BB) - (i \BB) \cdot (\spacegrad \wedge \BE) 
\right)
\\
\end{align*}

Grouping the two sets of repeated terms after reordering and the associated sign adjustments we have

\begin{align}\label{eqn:poyntingDivergence}
\spacegrad \cdot ((i \BB) \cdot \BE) &= \BE \cdot (\spacegrad \cdot (i \BB)) - (i \BB) \cdot (\spacegrad \wedge \BE)
\end{align}

which is the desired identity (in negated form) that was to be proved.

There is likely some theorem that could be used to avoid some of this algebra.

\bibliographystyle{plainnat}
\bibliography{myrefs}

\end{document}
