\chapter{Radial components of vector derivatives}\label{chap:PJRadialDer}
\date{ Oct 22, 2007.  $RCSfile: radialVectorDerivatives.tex,v $ Last $Revision: 1.7 $ $Date: 2009/06/11 16:45:58 $ }

\section{first derivative of a radially expressed vector.}

Having calculated the derivative of a unit vector, the total 
derivative of a radially expressed vector can be calculated

\begin{align*}
(r\rcap)'  
   &= r'\rcap  + r\rcap' \\
   &= r'\rcap  + \BrPrimeRej \\
\end{align*}

There are two components.  One is in the $\rcap$ direction (linear component)
and the other perpendicular to that (a rotational component) in the direction of the rejection
of $\rcap$ from $\Br'$.

\section{Second derivative of a vector}

Taking second derivatives of a radially expressed vector, we have

\begin{align*}
(r\rcap)'' 
   &= (r'\rcap + r{\rcap}')' \\
   &= r''\rcap + r'\rcap' + (r\rcap')' \\
   &= r''\rcap + (r'/r)\BrPrimeRej + (r\rcap')' \\
\end{align*}

Expanding the last term takes a bit more work
\begin{align*}
(r\rcap')' 
   &= (\BrPrimeRej)' \\
   &= 
\rcap'(\rcap \wedge \Br') +
\rcap(\rcap' \wedge \Br') +
\rcap(\rcap \wedge \Br'') \\
   &= 
(1/r)(\BrPrimeRej)(\rcap \wedge \Br') +
\rcap(\rcap' \wedge \Br') +
\rcap(\rcap \wedge \Br'') \\
   &= 
(1/r)\rcap(\rcap \wedge \Br')^2 +
\rcap(\rcap' \wedge \Br') +
\rcap(\rcap \wedge \Br'') \\
\end{align*}

There are three terms to this.  One a scalar (negative) multiple of $\rcap$, and another, the rejection of $\rcap$ from $\Br''$.  The middle term here remains to be expanded.  In particular,

\begin{align*}
\rcap' \wedge \Br' 
   &= \rcap' \wedge (r\rcap' + r'\rcap) \\
   &= r' \rcap' \wedge \rcap \\
   &= r'/2 (\rcap'\rcap - \rcap\rcap') \\
   &= r'/2r ((\Br' \wedge \rcap)\rcap\rcap - \rcap\rcap(\rcap \wedge \Br')) \\
   &= r'/2r (\Br' \wedge \rcap - \rcap \wedge \Br') \\
   &= -(r'/r) \rcap \wedge \Br' \\
\end{align*}

\begin{align*}
\implies
(r\rcap')' 
   &= 
(1/r)\rcap(\rcap \wedge \Br')^2 
-(r'/r)\BrPrimeRej 
+\rcap(\rcap \wedge \Br'') \\
\end{align*}

\begin{align*}
\implies
(r\rcap)'' 
   &= r''\rcap 
+(r'/r)\BrPrimeRej
+(1/r)\rcap(\rcap \wedge \Br')^2 
-(r'/r)\BrPrimeRej
+\rcap(\rcap \wedge \Br'') \\
   &= r''\rcap 
    +(1/r)\rcap(\rcap \wedge \Br')^2 
    +\rcap(\rcap \wedge \Br'') \\
   &= 
\rcap \left(  r'' +(1/r)(\rcap \wedge \Br')^2\right) +    \rcap(\rcap \wedge \Br'') \\
\end{align*}

There are two terms here that are in the $\rcap$ direction (the bivector square is a negative scalar), and
one rejective term in the direction of the component perpendicular to $\rcap$ relative to $\Br''$.

