\documentclass{article}

\input{../peeters_macros.tex}
\input{../peeters_macros2.tex}

\usepackage[bookmarks=true]{hyperref}

\usepackage{color,cite,graphicx}
   % use colour in the document, put your citations as [1-4]
   % rather than [1,2,3,4] (it looks nicer, and the extended LaTeX2e
   % graphics package. 
\usepackage{latexsym,amssymb,epsf} % don't remember if these are
   % needed, but their inclusion can't do any damage


\title{ Expressing wave equation exponential solutions using four vectors. }
\author{Peeter Joot}
\date{ Nov 30, 2008.  Last Revision: $Date: 2008/12/01 05:08:35 $ }

\begin{document}

\maketitle{}

%\tableofcontents
%\section{}

For the unforced wave equation in 3D one wants solutions to

\begin{align}\label{eqn:waveEquation}
\left( \inv{\Bv^2} \partial_{tt} - \sum_{j=1}^3 \partial_{jj}\right) \phi = 0
\end{align}

For the single spatial variable case one can verify that 
$\phi = f( \Bx \pm \Abs{\Bv} t)$ is a solution for any function $f$.  In particular $\phi = \exp(i (\pm \Abs{\Bv} t + x))$ is a solution.  Similarily
$\phi = \exp(i (\pm \Abs{\Bv} t + \kcap \cdot \Bx))$ is a solution in the 3D case.

Can the relativistic four vector notation be used to put this in a more symmetric form with respect to time and position?  For the four
vector

\begin{align*}
x = x^\mu \gamma_\mu
\end{align*}

Lets try the following as a possible solution to \ref{eqn:waveEquation}

\begin{align*}
\phi = \exp(i k \cdot x)
\end{align*}

verifying that this can be a solution, and determining the constraints required on the four vector $k$.

Observe that

\begin{align*}
x \cdot k = x^\mu k_\mu
\end{align*}

so

\begin{align*}
\phi_\mu &= i k_\mu \\
\phi_{\mu\mu} &= (i k_\mu)^2 \phi = -(k_\mu)^2 \phi
\end{align*}

Since $\partial_t = c\partial_0$, we have $\phi_tt = c^2 \phi_{00}$, and

\begin{align*}
\left( \inv{\Bv^2} \partial_{tt} - \sum_{j=1}^3 \partial_{jj}\right) \phi &= 
\left( -\inv{\Bv^2} c^2 {k_0}^2 - \sum_{j=1}^3 -(k_j)^2\right) \phi \\ 
\end{align*}

For equality with zero, and $\Bbeta = \Bv/c$, we require 

\begin{align*}
\Bbeta^2 = \frac{(k_0)^2}{\sum_j (k_j)^2}
\end{align*}

Now want the components of $k = k_\mu \gamma^\mu$ in terms of $k$ directly.  First

\begin{align*}
k_0 = k \cdot \gamma_0
\end{align*}

The spacetime relative vector for $k$ is

\begin{align*}
\Bk &= k \wedge \gamma_0 = \sum k_\mu \gamma^\mu \wedge \gamma_0 = (\gamma_1)^2 \sum_j k_j \sigma_j \\
\Bk^2 &= (\pm 1)^2 \sum_j (k_j)^2 
\end{align*}

So the constraint on the four vector parameter $k$ is 
\begin{align*}
\Bbeta^2
&= \frac{(k_0)^2}{\sum_j (k_j)^2} \\
&= \frac{(k \cdot \gamma_0)^2}{(k \wedge \gamma_0)^2} \\
\end{align*}

It is interesting to compare this to the relative spacetime bivector for $x$

\begin{align*}
v &= \frac{dx}{d\tau} = c \frac{dt}{d\tau} \gamma_0 + \frac{dx^i}{d\tau} \gamma_i \\
v \cdot \gamma^0 &= \frac{dx}{d\tau} \cdot \gamma^0 = c \frac{dt}{d\tau} \\
v \wedge \gamma_0 &= \frac{dx}{d\tau} \wedge \gamma_0 \\
&= \frac{dx^i}{d\tau} \sigma_i \\
&= \frac{dx^i}{dt} \frac{dt}{d\tau} \sigma_i \\
\end{align*}

\begin{align*}
\Bv/c
&= \frac{d (x^i \sigma_i) }{dt} \\
&= \frac{v \wedge \gamma_0}{ v \cdot \gamma^0 }
\end{align*}

So, for $\phi = \exp(i k \cdot x)$ to be a solution to the wave equation for a wave travelling with velocity $\Abs{\Bv}$, the constraint on k
in terms of proper velocity $v$ is

\begin{align*}
\Abs{\frac{k \wedge \gamma_0}{ k \cdot \gamma^0 }}^{-1} &=
\Abs{\frac{v \wedge \gamma_0}{ v \cdot \gamma^0 }}
\end{align*}

So we see the relative spacetime vector of $k$ has an inverse relationship with the relative spacetime velocity vector of $x$.

%\bibliographystyle{plainnat}
%\bibliography{myrefs}

\end{document}
