%
% Copyright © 2015 Peeter Joot.  All Rights Reserved.
% Licenced as described in the file LICENSE under the root directory of this GIT repository.
%
\input{../latex/blogpost.tex}
\renewcommand{\basename}{dualFarField}
\renewcommand{\dirname}{notes/ece1229/}
%\newcommand{\dateintitle}{}
%\newcommand{\keywords}{}

\input{../latex/peeter_prologue_print2.tex}

\usepackage{macros_bm}

\beginArtNoToc

\generatetitle{Duality transformation of the far field fields.}
%\section{Duality transformation of the far field fields.}
%\label{chap:dualFarField}

@Ted Shifrin mentioned in the comments that this translation is possible using Geometric Algebra.

With

\begin{equation}\label{eqn:t:n}
I = \Be_1 \Be_2 \Be_3,
\end{equation}

and the identity $ \Bx \cross \By = I (\Bx \wedge \By) $, the pair of identities becomes

\begin{equation}\label{eqn:t:n}
I \BA = \inv{2} \BB \wedge \Br
\end{equation}
\begin{equation}\label{eqn:t:n}
\spacegrad \wedge \BA = I \BB.
\end{equation}

Introducing a bivector dual $ \bcB = -I \BB $, these can be written

\begin{equation}\label{eqn:t:n}
\BA = \inv{2} \bcB \cdot \Br
\end{equation}
\begin{equation}\label{eqn:t:n}
\spacegrad \wedge \BA = -\bcB, \qquad (1)
\end{equation}

As with the coordinate expansion of the original 3D vector result, this can be verified by direct expansion.  Assuming an antisymmetric scalar $ B_{ab} = -B_{ba} $, the bivector coordinate expansion is

\begin{equation}\label{eqn:t:n}
\bcB = \inv{2} B_{ab} \Be_a \wedge \Be_b.
\end{equation}

Expanding out (1) gives

\begin{equation}\label{eqn:t:n}
\begin{aligned}
\spacegrad \wedge \BA
&=
\Be_i \partial_i \wedge \left(
\inv{4} B_{ab} (\Be_a \wedge \Be_b) \cdot (\Be_s x_s)
\right)
\\
&=
\inv{4}
B_{ab}
\Be_i \wedge \left(
 (\Be_a \wedge \Be_b) \cdot (\Be_s \delta_{i s})
\right)  \\
&=
\inv{4}
B_{ab}
\Be_i \wedge \left(
 (\Be_a \wedge \Be_b) \cdot \Be_i
\right)  \\
&=
\inv{4}
B_{ab}
\Be_i \wedge \left(
 \Be_a \delta_{b i} - \Be_b \delta_{a i}
\right)  \\
&=
\inv{4}
B_{ab}
\left(
\Be_b \wedge \Be_a - \Be_a \wedge \Be_b
\right)  \\
&=
-\inv{2} B_{ab} \Be_a \wedge \Be_b \\
&=
-\bcB
\end{aligned}
\end{equation}

Mapping the Geometric Algebra form to differential forms should (I believe) just require using differentials as the basis, and using the $ d $ operator in place of the bivector curl $ \spacegrad \wedge $.  With

\begin{equation}\label{eqn:t:n}
\begin{aligned}
\bcB &= \inv{2} B_{ab} dx_a \wedge dx_b \\
\Br &= x_a dx_a,
\end{aligned}
\end{equation}

that is

\begin{equation}\label{eqn:t:n}
d \BA = -\bcB.
\end{equation}

Presuming that is the right notation, then

\begin{equation}\label{eqn:t:n}
\begin{aligned}
\BA
&= \inv{2} \bcB \cdot \Br \\
&=
\inv{4} B_{ab} (dx_a \wedge dx_b) \cdot (dx_s x_s) \\
&=
\inv{4} B_{ab} x_s ( dx_a \delta_{bs} - dx_b \delta_{as} ) \\
&=
\inv{4} B_{ab} (x_b dx_a - x_a dx_b).
\end{aligned}
\end{equation}

Application of the differential operator gives

\begin{equation}\label{eqn:t:n}
\begin{aligned}
d\BA
&=
\inv{4} B_{ab} d(x_b dx_a - x_a dx_b) \\
&=
\inv{4} B_{ab} (dx_b \wedge dx_a - dx_a \wedge dx_b) \\
&=
-
\inv{2} B_{ab} dx_a \wedge dx_b \\
&=
-\bcB.
\end{aligned}
\end{equation}

\EndArticle
