%
% Copyright © 2013 Peeter Joot.  All Rights Reserved.
% Licenced as described in the file LICENSE under the root directory of this GIT repository.
%
\input{../latex/blogpost.tex}
\renewcommand{\basename}{curvilinearCoordinates}
\renewcommand{\dirname}{notes/gabook/}
%\newcommand{\dateintitle}{}
\newcommand{\keywords}{curvilinear coordinates, geometric algebra, dual basis, reciprocal coordinates}

\input{../latex/peeter_prologue_print2.tex}

% for post to:
% http://math.stackexchange.com/questions/766146/inner-product-of-trivector-and-bivector-in-geometric-algebra
\beginArtNoToc

Hestenes's New Foundations book \citep{hestenes1999nfc} sets a problem to show:

\begin{dmath}\label{eqn:trivectorBivectorInnerProduct:20}
\left( \Ba \wedge \Bb \wedge \Bc \right) \cdot B
=
\Ba \left( \left( \Bb \wedge \Bc \right) \cdot B \right)
+
\Bb \left( \left( \Bc \wedge \Ba \right) \cdot B \right)
+
\Bc \left( \left( \Ba \wedge \Bb \right) \cdot B \right).
\end{dmath}

I'm having trouble proving this.  Using an antisymmetric expansion of the wedge within a grade one selection, we have

\begin{equation}\label{eqn:trivectorBivectorInnerProduct:40}
\begin{aligned}
\left( \Ba \wedge \Bb \wedge \Bc \right) \cdot B
&=
\inv{6}
{\left\langle
\left(
\Ba \Bb \Bc
+\Bb \Bc \Ba
+\Bc \Ba \Bb
-\Ba \Bc \Ba
-\Bb \Ba \Bc
-\Bc \Bb \Ba
\right)
B
\right\rangle}_1 \\
&=
\inv{3}
{\left\langle
\Ba \left( \Bb \wedge \Bc \right) B
+\Bb \left( \Bc \wedge \Ba\right) B
+\Bc \left( \Ba \wedge \Bb\right) B
\right\rangle}_1 \\
&=
\inv{3}
\left(
\Ba \left( \left( \Bb \wedge \Bc \right) \cdot B \right)
+\Bb \left( \left( \Bc \wedge \Ba\right) \cdot B \right)
+\Bc \left( \left( \Ba \wedge \Bb\right) \cdot B \right)
\right) \\
&\quad +
\inv{3}
\left(
\Ba \cdot {\left\langle \left( \Bb \wedge \Bc \right) B \right\rangle}_2
+\Bb \cdot {\left\langle \left( \Bc \wedge \Ba\right) B \right\rangle}_2
+\Bc \cdot {\left\langle \left( \Ba \wedge \Bb\right) B \right\rangle}_2
\right).
\end{aligned}
\end{equation}

My attempts to reduce the latter terms have all gone in circles.  Any tips?

\section{Answer}

I figured it out.  The key is trying not to be so clever, instead expand in successive dot products and regroup.  With $B = \Bu \wedge \Bv$

\begin{equation}\label{eqn:trivectorBivectorInnerProduct:60}
\begin{aligned}
\left(  \Ba \wedge \Bb \wedge \Bc  \right)
\cdot B
&=
\gpgradeone{
\left(  \Ba \wedge \Bb \wedge \Bc \right)
 \left( \Bu \wedge \Bv \right) } \\
&=
\gpgradeone{
\left(  \Ba \wedge \Bb \wedge \Bc  \right)
\left(
\Bu \Bv
- \Bu \cdot \Bv
\right) } \\
&=
\left(
\left(  \Ba \wedge \Bb \wedge \Bc  \right)
 \cdot \Bu \right) \cdot \Bv \\
&=
\left( \Ba \wedge \Bb \right) \cdot \Bv \left( \Bc \cdot \Bu \right)
+
\left( \Bc \wedge \Ba \right) \cdot \Bv \left( \Bb \cdot \Bu \right)
+
\left( \Bb \wedge \Bc \right) \cdot \Bv \left( \Ba \cdot \Bu \right) \\
&=
\Ba
\left(  \Bb \cdot \Bv  \right)
\left( \Bc \cdot \Bu \right)
-\Bb
\left(  \Ba \cdot \Bv  \right)
\left( \Bc \cdot \Bu \right) \\
&\quad +
\Bc
\left(  \Ba \cdot \Bv  \right)
\left( \Bb \cdot \Bu \right)
-
\Ba
\left(  \Bc \cdot \Bv  \right)
\left( \Bb \cdot \Bu \right) \\
&\quad +
\Bb
\left(  \Bc \cdot \Bv  \right)
\left( \Ba \cdot \Bu \right)
-
\Bc
\left(  \Bb \cdot \Bv  \right)
\left( \Ba \cdot \Bu \right) \\
&=
\Ba
\left(  \left(  \Bb \cdot \Bv  \right) \left( \Bc \cdot \Bu \right) - \left(  \Bc \cdot \Bv  \right) \left( \Bb \cdot \Bu \right)  \right)
\\
&\quad +
\Bb
\left(  \left(  \Bc \cdot \Bv  \right) \left( \Ba \cdot \Bu \right) - \left(  \Ba \cdot \Bv  \right) \left( \Bc \cdot \Bu \right)  \right)
\\
&\quad +
\Bc
\left(  \left(  \Ba \cdot \Bv  \right) \left( \Bb \cdot \Bu \right) - \left(  \Bb \cdot \Bv  \right) \left( \Ba \cdot \Bu \right)  \right)
 \\
&=
\Ba
\left(  \Bb \wedge \Bc  \right)
\cdot
\left(  \Bu \wedge \Bv  \right)
\\
&\quad +
\Bb
\left(  \Bc \wedge \Ba  \right)
\cdot
\left(  \Bu \wedge \Bv  \right)
\\
&\quad +
\Bc
\left(  \Ba \wedge \Bb  \right)
 \cdot
\left(  \Bu \wedge \Bv  \right)
\\
&=
\Ba
\left(  \Bb \wedge \Bc  \right)
\cdot B
+
\Bb
\left(  \Bc \wedge \Ba  \right)
 \cdot B
+
\Bc
\left(  \Ba \wedge \Bb  \right)
\cdot B.
\end{aligned}
\end{equation}

\EndArticle
