%\paragraph{Useful identities.}

%\begin{equation}\label{eqn:emtLecture3:540}
\begin{equation}\label{eqn:usefulFormulas:620}
\spacegrad' \inv{R} = \frac{\rcap}{R^2} = -\spacegrad \inv{R}
\end{equation}
%\begin{equation}\label{eqn:emtLecture3:560}
\begin{equation}\label{eqn:usefulFormulas:640}
\spacegrad R = \rcap = \frac{\BR}{R}
\end{equation}
%\begin{equation}\label{eqn:emtLecture3:580}
\begin{equation}\label{eqn:usefulFormulas:660}
\spacegrad f(R) = \rcap \PD{R}{f}
\end{equation}
%\begin{equation}\label{eqn:emtLecture3:600}
\begin{equation}\label{eqn:usefulFormulas:680}
-\spacegrad^2 \inv{R} = 4\pi \delta(\BR)
\end{equation}

\begin{equation}\label{eqn:usefulFormulas:700}
\spacegrad \cross \lr{ \spacegrad \cross \BA } = \spacegrad \lr{ \spacegrad \cdot \BA } - \spacegrad^2 \BA.
\end{equation}

\paragraph{Proofs.}

This result was used in ps1 problem 3,5, and 6.

\begin{dmath}\label{eqn:emtProblemSet1Appendix:460}
\spacegrad \cross \lr{ \spacegrad \cross \BA }
=
\epsilon_{a b c} \Be_a \partial_b \lr{ \epsilon_{r s t} \Be_r \partial_s A_t }_c
=
\epsilon_{a b c} \Be_a \partial_b \epsilon_{c s t} \partial_s A_t
=
\delta_{ab}^{[st]}
\Be_a \partial_b \partial_s A_t
=
\Be_a \partial_b \lr{ \partial_a A_b - \partial_b A_a }
=
\spacegrad \lr{ \spacegrad \cdot \BA } - \spacegrad^2 \BA.
\end{dmath}
